dot12_wip becomes dot12 since file type checks

dev2015/dot12.v
@@ -1,11 +1,10 @@
 (* Full safety for DOT (WIP) *)
 
 (* this version is based on dot10.v *)
-(* based on that, it adds intersection types from dot3.v *)
+(* based on that, it adds intersection types *)
 
 (*
-TODO:
-- stp2 trans + narrowing 
+- stp2 trans + narrowing
 - stp/stp2 weakening and regularity
 *)
 
@@ -20,8 +19,8 @@ Definition id := nat.
 
 Inductive ty : Type :=
   | TBool  : ty
-  | TBot   : ty           
-  | TTop   : ty    
+  | TBot   : ty
+  | TTop   : ty
   | TFun   : ty -> ty -> ty
   | TMem   : ty -> ty -> ty
   | TSel   : id -> ty
@@ -117,16 +116,16 @@ Inductive closed_rec: nat -> nat -> ty -> Prop :=
     closed_rec k l (TBind T2)
 | cl_sel: forall k l x,
     closed_rec k l (TSel x)
+| cl_and: forall k l T1 T2,
+    closed_rec k l T1 ->
+    closed_rec k l T2 ->
+    closed_rec k l (TAnd T1 T2)
 | cl_selh: forall k l x,
     l > x ->
     closed_rec k l (TSelH x)
 | cl_selb: forall k l i,
     k > i ->
     closed_rec k l (TSelB i)
-| cl_and: forall k l T1 T2,
-    closed_rec k l T1 ->
-    closed_rec k l T2 ->
-    closed_rec k l (TAnd T1 T2)
 .
 
 Hint Constructors closed_rec.
@@ -184,7 +183,7 @@ Fixpoint nosubst (T : ty) {struct T} : Prop :=
     | TSelH i      => i <> 0
     | TAll T1 T2   => nosubst T1 /\ nosubst T2
     | TBind T2     => nosubst T2
-    | TAnd T1 T2 => nosubst T1 /\ nosubst T2
+    | TAnd T1 T2   => nosubst T1 /\ nosubst T2
   end.
 
 
@@ -192,96 +191,110 @@ Hint Unfold open.
 Hint Unfold closed.
 
 
-Inductive stp: tenv -> tenv -> option (bool * id) -> ty -> ty -> Prop :=
-| stp_topx: forall G1 GH S,
-    stp G1 GH S TTop TTop
-| stp_botx: forall G1 GH S,
-    stp G1 GH S TBot TBot
-| stp_top: forall G1 GH S T1,
-    stp G1 GH S T1 T1 ->
-    stp G1 GH S T1 TTop
-| stp_bot: forall G1 GH S T2,
-    stp G1 GH S T2 T2 ->
-    stp G1 GH S TBot T2
-| stp_bool: forall G1 GH S,
-    stp G1 GH S TBool TBool
-| stp_fun: forall G1 GH S T1 T2 T3 T4,
-    stp G1 GH None T3 T1 ->
-    stp G1 GH None T2 T4 ->
-    stp G1 GH S (TFun T1 T2) (TFun T3 T4)             
-| stp_mem: forall G1 GH S T1 T2 T3 T4,
-    stp G1 GH None T3 T1 ->
-    stp G1 GH None T2 T4 ->
-    stp G1 GH S (TMem T1 T2) (TMem T3 T4)
-| stp_sel1: forall G1 GH S TX T2 x,
+Inductive stp: tenv -> tenv -> ty -> ty -> Prop :=
+| stp_topx: forall G1 GH,
+    stp G1 GH TTop TTop
+| stp_botx: forall G1 GH,
+    stp G1 GH TBot TBot
+| stp_top: forall G1 GH T1,
+    stp G1 GH T1 T1 -> (* regularity *)
+    stp G1 GH T1 TTop
+| stp_bot: forall G1 GH T2,
+    stp G1 GH T2 T2 -> (* regularity *)
+    stp G1 GH TBot T2
+| stp_bool: forall G1 GH,
+    stp G1 GH TBool TBool
+| stp_fun: forall G1 GH T1 T2 T3 T4,
+    stp G1 GH T3 T1 ->
+    stp G1 GH T2 T4 ->
+    stp G1 GH (TFun T1 T2) (TFun T3 T4)
+| stp_mem: forall G1 GH T1 T2 T3 T4,
+    stp G1 GH T3 T1 ->
+    stp G1 GH T2 T4 ->
+    stp G1 GH (TMem T1 T2) (TMem T3 T4)
+| stp_sel1: forall G1 GH TX T2 x,
     index x G1 = Some TX ->
-    stp G1 GH S TX (TMem TBot T2) ->   
-    stp G1 GH S (TSel x) T2
-| stp_sel2: forall G1 GH S TX T1 x,
+    closed 0 0 TX ->
+    stp G1 GH TX (TMem TBot T2) ->
+    stp G1 GH T2 T2 -> (* regularity of stp2 *)
+    stp G1 GH (TSel x) T2
+| stp_sel2: forall G1 GH TX T1 x,
     index x G1 = Some TX ->
-    stp G1 GH S TX (TMem T1 TTop) ->
-    stp G1 GH S T1 (TSel x)
-| stp_selb1: forall G1 GH S TX T2 x,
-    index x G1 = Some TX -> 
-    stp G1 [] S TX (TBind (TMem TBot T2)) ->   (* Note GH = [] *)
-    stp G1 GH S (TSel x) (open (TSel x) T2)
-| stp_selb2: forall G1 GH S TX T1 x,
+    closed 0 0 TX ->
+    stp G1 GH TX (TMem T1 TTop) ->
+    stp G1 GH T1 T1 -> (* regularity of stp2 *)
+    stp G1 GH T1 (TSel x)
+| stp_selb1: forall G1 GH TX T2 x,
     index x G1 = Some TX ->
-    stp G1 [] S TX (TBind (TMem T1 TTop)) ->   (* Note GH = [] *)
-    stp G1 GH S (open (TSel x) T1) (TSel x)
-| stp_selx: forall G1 GH S TX x,
+    stp G1 [] TX (TBind (TMem TBot T2)) ->   (* Note GH = [] *)
+    stp G1 GH (open (TSel x) T2) (open (TSel x) T2) -> (* regularity *)
+    stp G1 GH (TSel x) (open (TSel x) T2)
+| stp_selb2: forall G1 GH TX T1 x,
     index x G1 = Some TX ->
-    stp G1 GH S (TSel x) (TSel x)
-| stp_sela1: forall G1 GH S TX T2 x,
-    indexr x GH = Some TX -> 
-    stp G1 GH S TX (TMem TBot T2) ->   (* not using self name for now *)
-    stp G1 GH S (TSelH x) T2
-| stp_sela2: forall G1 GH S TX T1 x,
+    stp G1 [] TX (TBind (TMem T1 TTop)) ->   (* Note GH = [] *)
+    stp G1 GH (open (TSel x) T1) (open (TSel x) T1) -> (* regularity *)
+    stp G1 GH (open (TSel x) T1) (TSel x)
+| stp_selx: forall G1 GH TX x,
+    index x G1 = Some TX ->
+    stp G1 GH (TSel x) (TSel x)
+| stp_sela1: forall G1 GH TX T2 x,
     indexr x GH = Some TX ->
-    stp G1 GH S TX (TMem T1 TTop) ->   (* not using self name for now *)
-    stp G1 GH S T1 (TSelH x)
-| stp_selab1: forall G1 GH S TX T2 T2' x,
-    indexr x GH = Some TX -> 
-    stp G1 [] S TX (TBind (TMem TBot T2)) ->   (* XXX Note GH = [] *)
+    closed 0 x TX ->
+    stp G1 GH TX (TMem TBot T2) ->   (* not using self name for now *)
+    stp G1 GH T2 T2 -> (* regularity of stp2 *)
+    stp G1 GH (TSelH x) T2
+| stp_sela2: forall G1 GH TX T1 x,
+    indexr x GH = Some TX ->
+    closed 0 x TX ->
+    stp G1 GH TX (TMem T1 TTop) ->   (* not using self name for now *)
+    stp G1 GH T1 T1 -> (* regularity of stp2 *)
+    stp G1 GH T1 (TSelH x)
+| stp_selab1: forall G1 GH TX T2 T2' x,
+    indexr x GH = Some TX ->
+    stp G1 [] TX (TBind (TMem TBot T2)) ->   (* XXX Note GH = [] *)
     T2' = (open (TSelH x) T2) ->
-    stp G1 GH S (TSelH x) T2'
-| stp_selab2: forall G1 GH S TX T1 T1' x,
+    stp G1 GH T2' T2' -> (* regularity *)
+    stp G1 GH (TSelH x) T2'
+| stp_selab2: forall G1 GH TX T1 T1' x,
     indexr x GH = Some TX ->
-    stp G1 [] S TX (TBind (TMem T1 TTop)) ->   (* XXX Note GH = [] *)
+    stp G1 [] TX (TBind (TMem T1 TTop)) ->   (* XXX Note GH = [] *)
     T1' = (open (TSelH x) T1) ->
-    stp G1 GH S T1' (TSelH x)
-| stp_selax: forall G1 GH S TX x,
+    stp G1 GH T1' T1' -> (* regularity *)
+    stp G1 GH T1' (TSelH x)
+| stp_selax: forall G1 GH TX x,
     indexr x GH = Some TX  ->
-    stp G1 GH S (TSelH x) (TSelH x)
-| stp_all: forall G1 GH S T1 T2 T3 T4 x,
-    stp G1 GH None T3 T1 ->
+    stp G1 GH (TSelH x) (TSelH x)
+| stp_all: forall G1 GH T1 T2 T3 T4 x,
+    stp G1 GH T3 T1 ->
     x = length GH ->
     closed 1 (length GH) T2 -> (* must not accidentally bind x *)
-    closed 1 (length GH) T4 -> 
-    stp G1 ((0,T3)::GH) None (open (TSelH x) T2) (open (TSelH x) T4) ->
-    stp G1 GH S (TAll T1 T2) (TAll T3 T4)
-| stp_bindx: forall G1 GH S T1 T2 x,
+    closed 1 (length GH) T4 ->
+    stp G1 ((0,T1)::GH) (open (TSelH x) T2) (open (TSelH x) T2) -> (* regularity *)
+    stp G1 ((0,T3)::GH) (open (TSelH x) T2) (open (TSelH x) T4) ->
+    stp G1 GH (TAll T1 T2) (TAll T3 T4)
+| stp_bindx: forall G1 GH T1 T2 x,
     x = length GH ->
     closed 1 (length GH) T1 -> (* must not accidentally bind x *)
-    closed 1 (length GH) T2 -> 
-    stp G1 ((0,open (TSelH x) T1)::GH) S (open (TSelH x) T1) (open (TSelH x) T2) ->
-    stp G1 GH S (TBind T1) (TBind T2)
-| stp_and11: forall G1 G2 S T1 T2 T,
-    stp G1 G2 S T1 T ->
-    stp G1 G1 S T2 T2 -> (* regularity *)
-    stp G1 G2 S (TAnd T1 T2) T
-| stp_and12: forall G1 G2 S T1 T2 T,
-    stp G1 G2 S T2 T ->
-    stp G1 G1 S T1 T1 -> (* regularity *)
-    stp G1 G2 S (TAnd T1 T2) T
-| stp_and2: forall G1 G2 S T1 T2 T,
-    stp G1 G2 S T T1 ->
-    stp G1 G2 S T T2 ->
-    stp G1 G2 S T (TAnd T1 T2)
+    closed 1 (length GH) T2 ->
+    stp G1 ((0,open (TSelH x) T2)::GH) (open (TSelH x) T2) (open (TSelH x) T2) -> (* regularity *)
+    stp G1 ((0,open (TSelH x) T1)::GH) (open (TSelH x) T1) (open (TSelH x) T2) ->
+    stp G1 GH (TBind T1) (TBind T2)
+| stp_and11: forall G GH T1 T2 T,
+    stp G GH T1 T ->
+    stp G GH T2 T2 -> (* regularity *)
+    stp G GH (TAnd T1 T2) T
+| stp_and12: forall G GH T1 T2 T,
+    stp G GH T2 T ->
+    stp G GH T1 T1 -> (* regularity *)
+    stp G GH (TAnd T1 T2) T
+| stp_and2: forall G GH T1 T2 T,
+    stp G GH T T1 ->
+    stp G GH T T2 ->
+    stp G GH T (TAnd T1 T2)
 .
 
 
-(*        
+(*
 with path_type: tenv -> tenv -> id -> ty -> Prop :=
 | pt_var: forall G1 GH TX x,
     index x G1 = Some TX ->
@@ -294,7 +307,7 @@ with path_type: tenv -> tenv -> id -> ty -> Prop :=
 with pathH_type: tenv -> tenv -> id -> ty -> Prop :=
 | pth_var: forall G1 GH TX T x,
     indexr x GH = Some TX ->
-    stp G1 GH TX T ->        
+    stp G1 GH TX T ->
     pathH_type G1 GH x T
 *)
 
@@ -320,7 +333,7 @@ Inductive has_type : tenv -> tm -> ty -> Prop :=
 | t_typ: forall env x T1 T1X,
            fresh env = x ->
            open (TSel x) T1 = T1X ->
-           stp ((x,TMem T1X T1X)::env) [] None T1X T1X ->
+           stp ((x,TMem T1X T1X)::env) [] T1X T1X ->
            has_type env (ttyp T1) (TBind (TMem T1 T1))
 | t_app: forall env f x T1 T2,
            has_type env f (TFun T1 T2) ->
@@ -328,14 +341,14 @@ Inductive has_type : tenv -> tm -> ty -> Prop :=
            has_type env (tapp f x) T2
 | t_abs: forall env f x y T1 T2,
            has_type ((x,T1)::(f,TFun T1 T2)::env) y T2 ->
-           stp env [] None (TFun T1 T2) (TFun T1 T2) ->
+           stp env [] (TFun T1 T2) (TFun T1 T2) ->
            fresh env <= f ->
            1+f <= x ->
            has_type env (tabs f x y) (TFun T1 T2)
 | t_tapp: forall env f x T11 T12,
            has_type env f (TAll T11 T12) ->
            has_type env x T11 ->
-           stp env [] None T12 T12 ->
+           stp env [] T12 T12 ->
            has_type env (ttapp f x) T12
 (*
 NOTE: both the POPLmark paper and Cardelli's paper use this rule:
@@ -346,16 +359,16 @@ Does it make a difference? It seems like we can always widen f?
            stp env T2 T11 ->
            has_type env (ttapp f T2) (open T2 T12)
 
-*)                    
+*)
 | t_tabs: forall env x y T1 T2,
-           has_type ((x,T1)::env) y (open (TSel x) T2) -> 
-           stp env [] None (TAll T1 T2) (TAll T1 T2) ->
+           has_type ((x,T1)::env) y (open (TSel x) T2) ->
+           stp env [] (TAll T1 T2) (TAll T1 T2) ->
            fresh env = x ->
            has_type env (ttabs x T1 y) (TAll T1 T2)
 
 | t_sub: forall env e T1 T2,
            has_type env e T1 ->
-           stp env [] None T1 T2 ->
+           stp env [] T1 T2 ->
            has_type env e T2
 .
 
@@ -373,23 +386,23 @@ Definition MAX := 2.
 
 Inductive stp2: nat -> bool -> venv -> ty -> venv -> ty -> list (id*(venv*ty)) -> nat -> Prop :=
 | stp2_topx: forall m G1 G2 GH n1,
-    stp2 m true G1 TTop G2 TTop GH n1
+    stp2 m true G1 TTop G2 TTop GH (S n1)
 | stp2_botx: forall m G1 G2 GH n1,
-    stp2 m true G1 TBot G2 TBot GH n1
+    stp2 m true G1 TBot G2 TBot GH (S n1)
 | stp2_top: forall m G1 G2 GH T n1,
-    stp2 MAX false G1 T G1 T GH n1 ->
+    stp2 m true G1 T G1 T GH n1 -> (* regularity *)
     stp2 m true G1 T G2 TTop GH (S n1)
 | stp2_bot: forall m G1 G2 GH T n1,
-    stp2 MAX false G2 T G2 T GH n1 ->
+    stp2 m true G2 T G2 T GH n1 -> (* regularity *)
     stp2 m true G1 TBot G2 T GH (S n1)
 | stp2_bool: forall m G1 G2 GH n1,
-    stp2 m true G1 TBool G2 TBool GH n1
+    stp2 m true G1 TBool G2 TBool GH (S n1)
 | stp2_fun: forall m G1 G2 T1 T2 T3 T4 GH n1 n2,
     stp2 MAX false G2 T3 G1 T1 GH n1 ->
     stp2 MAX false G1 T2 G2 T4 GH n2 ->
     stp2 m true G1 (TFun T1 T2) G2 (TFun T3 T4) GH (S (n1+n2))
 | stp2_mem: forall G1 G2 T1 T2 T3 T4 GH n1 n2,
-    stp2 1 false G2 T3 G1 T1 GH n1 ->
+    stp2 0 false G2 T3 G1 T1 GH n1 ->
     stp2 0 true G1 T2 G2 T4 GH n2 ->
     stp2 0 true G1 (TMem T1 T2) G2 (TMem T3 T4) GH (S (n1+n2))
 
@@ -402,12 +415,14 @@ Inductive stp2: nat -> bool -> venv -> ty -> venv -> ty -> list (id*(venv*ty)) -
 (* strong version, with precise/invertible bounds *)
 | stp2_strong_sel1: forall G1 G2 GX TX x T2 GH n1,
     index x G1 = Some (vty GX TX) ->
+(*  val_type GX (vty GX TX) (TMem TX TX) -> (* for downgrade *)*)
     closed 0 0 TX ->
     stp2 0 true GX TX G2 T2 GH n1 ->
     stp2 0 true G1 (TSel x) G2 T2 GH (S n1)
 
 | stp2_strong_sel2: forall G1 G2 GX TX x T1 GH n1,
     index x G2 = Some (vty GX TX) ->
+(*  val_type GX (vty GX TX) (TMem TX TX) -> (* for downgrade *)*)
     closed 0 0 TX ->
     stp2 0 false G1 T1 GX TX GH n1 ->
     stp2 0 true G1 T1 G2 (TSel x) GH (S n1)
@@ -416,81 +431,90 @@ Inductive stp2: nat -> bool -> venv -> ty -> venv -> ty -> list (id*(venv*ty)) -
     index x1 G1 = Some v ->
     index x2 G2 = Some v ->
     stp2 0 true G1 (TSel x1) G2 (TSel x2) GH n1
-         
-         
+
+
 (* existing object, but imprecise type *)
-| stp2_sel1: forall m G1 G2 GX TX x T2 GH n1 v,
+| stp2_sel1: forall m G1 G2 GX TX x T2 GH n1 n2 v,
     index x G1 = Some v ->
     val_type GX v TX ->
     closed 0 0 TX ->
     stp2 (S m) false GX TX G2 (TMem TBot T2) GH n1 ->
-    stp2 (S m) true G1 (TSel x) G2 T2 GH (S n1)
+    stp2 (S m) true G2 T2 G2 T2 GH n2 -> (* regularity *)
+    stp2 (S m) true G1 (TSel x) G2 T2 GH (S (n1+n2))
 
-| stp2_sel1b: forall m G1 G2 GX TX x T2 GH n1 v,
+| stp2_selb1: forall m G1 G2 GX TX x T2 GH n1 n2 v,
     index x G1 = Some v ->
     val_type GX v TX ->
     closed 0 0 TX ->
     stp2 (S (S m)) false GX TX G2 (TBind (TMem TBot T2)) [] n1 -> (* Note GH = [] *)
-    stp2 (S (S m)) true G1 (TSel x) G2 (open (TSel x) T2) GH (S n1)
+    stp2 (S (S m)) true G2 (open (TSel x) T2) G2 (open (TSel x) T2) GH n2 -> (* regularity *)
+    stp2 (S (S m)) true G1 (TSel x) G2 (open (TSel x) T2) GH (S (n1+n2))
 
-         
-| stp2_sel2: forall m G1 G2 GX TX x T1 GH n1 v,
+
+| stp2_sel2: forall m G1 G2 GX TX x T1 GH n1 n2 v,
     index x G2 = Some v ->
-    val_type GX v TX ->           
+    val_type GX v TX ->
     closed 0 0 TX ->
     stp2 (S m) false GX TX G1 (TMem T1 TTop) GH n1 ->
-    stp2 (S m) true G1 T1 G2 (TSel x) GH (S n1)
-         
+    stp2 (S m) true G1 T1 G1 T1 GH n2 -> (* regularity *)
+    stp2 (S m) true G1 T1 G2 (TSel x) GH (S (n1+n2))
+
 | stp2_selx: forall m G1 G2 v x1 x2 GH n1,
     index x1 G1 = Some v ->
     index x2 G2 = Some v ->
-    stp2 (S m) true G1 (TSel x1) G2 (TSel x2) GH n1
-         
-(* hypothetical object *)
-| stp2_sela1: forall m G1 G2 GX TX x T2 GH n1,
-    indexr x GH = Some (GX, TX) ->
-    (* closed 0 x TX -> *)
-    stp2 (S m) false GX TX G2 (TMem TBot T2) GH n1 ->
-    stp2 (S m) true G1 (TSelH x) G2 T2 GH (S n1)
+    stp2 (S m) true G1 (TSel x1) G2 (TSel x2) GH (S n1)
 
-| stp2_selab1: forall m G1 G2 GX TX x T2 GH n1, (* XXX TODO *)
+(* hypothetical object *)
+| stp2_sela1: forall m G1 G2 GX TX x T2 GH n1 n2,
+    indexr x GH = Some (GX, TX) ->
+    closed 0 x TX ->
+    stp2 (S m) false GX TX G2 (TMem TBot T2) GH n1 ->
+    stp2 (S m) true G2 T2 G2 T2 GH n2 -> (* regularity *)
+    stp2 (S m) true G1 (TSelH x) G2 T2 GH (S (n1+n2))
+
+| stp2_selab1: forall m G1 G2 GX TX x T2 T2' GH n1 n2, (* XXX TODO *)
     indexr x GH = Some (GX, TX) ->
     (* closed 0 x TX -> *)
     stp2 (S m) false GX TX G2 (TBind (TMem TBot T2)) [] n1 ->
-    stp2 (S m) true G1 (TSelH x) G2 (open (TSelH x) T2) GH (S n1)
+    T2' = (open (TSelH x) T2) ->
+    stp2 (S m) true G2 T2' G2 T2' GH n2 -> (* regularity *)
+    stp2 (S m) true G1 (TSelH x) G2 T2' GH (S (n1+n2))
 
-| stp2_sela2: forall m G1 G2 GX TX x T1 GH n1,
+| stp2_sela2: forall m G1 G2 GX TX x T1 GH n1 n2,
     indexr x GH = Some (GX, TX) ->
-    (* closed 0 x TX -> *)
+    closed 0 x TX ->
     stp2 (S m) false GX TX G2 (TMem T1 TTop) GH n1 ->
-    stp2 (S m) true G1 T1 G2 (TSelH x) GH (S n1)
+    stp2 (S m) true G1 T1 G1 T1 GH n2 -> (* regularity *)
+    stp2 (S m) true G1 T1 G2 (TSelH x) GH (S (n1+n2))
 
-         
+
 | stp2_selax: forall m G1 G2 GX TX x GH n1,
     indexr x GH = Some (GX, TX) ->
-    indexr x GH = Some (GX, TX) ->
-    stp2 (S m) true G1 (TSelH x) G2 (TSelH x) GH n1
+    stp2 (S m) true G1 (TSelH x) G2 (TSelH x) GH (S n1)
 
 
-| stp2_all: forall m G1 G2 T1 T2 T3 T4 GH n1 n2, 
+| stp2_all: forall m G1 G2 T1 T2 T3 T4 GH n1 n1' n2,
     stp2 MAX false G2 T3 G1 T1 GH n1 ->
     closed 1 (length GH) T2 -> (* must not accidentally bind x *)
-    closed 1 (length GH) T4 -> 
+    closed 1 (length GH) T4 ->
+    stp2 MAX false G1 (open (TSelH (length GH)) T2) G1 (open (TSelH (length GH)) T2) ((0,(G1, T1))::GH) n1' -> (* regularity *)
     stp2 MAX false G1 (open (TSelH (length GH)) T2) G2 (open (TSelH (length GH)) T4) ((0,(G2, T3))::GH) n2 ->
-    stp2 m true G1 (TAll T1 T2) G2 (TAll T3 T4) GH (S (n1+n2))
+    stp2 m true G1 (TAll T1 T2) G2 (TAll T3 T4) GH (S (n1+n1'+n2))
 
-| stp2_bind: forall G1 G2 T1 T2 GH n1, 
+| stp2_bind: forall G1 G2 T1 T2 GH n1 n2,
     closed 1 (length GH) T1 -> (* must not accidentally bind x *)
-    closed 1 (length GH) T2 -> 
+    closed 1 (length GH) T2 ->
+    stp2 1 false G2 (open (TSelH (length GH)) T2) G2 (open (TSelH (length GH)) T2) ((0,(G2, open (TSelH (length GH)) T2))::GH) n2 -> (* regularity *)
     stp2 1 false G1 (open (TSelH (length GH)) T1) G2 (open (TSelH (length GH)) T2) ((0,(G1, open (TSelH (length GH)) T1))::GH) n1 ->
-    stp2 0 true G1 (TBind T1) G2 (TBind T2) GH (S n1)
+    stp2 0 true G1 (TBind T1) G2 (TBind T2) GH (S (n1+n2))
 
-| stp2_bindb: forall m G1 G2 T1 T2 GH n1, 
+| stp2_bindb: forall m G1 G2 T1 T2 GH n1 n2,
     closed 1 (length GH) T1 -> (* must not accidentally bind x *)
-    closed 1 (length GH) T2 -> 
+    closed 1 (length GH) T2 ->
+    stp2 (S m) false G2 (open (TSelH (length GH)) T2) G2 (open (TSelH (length GH)) T2) ((0,(G2, open (TSelH (length GH)) T2))::GH) n2 -> (* regularity *)
     stp2 (S m) false G1 (open (TSelH (length GH)) T1) G2 (open (TSelH (length GH)) T2) ((0,(G1, open (TSelH (length GH)) T1))::GH) n1 ->
-    stp2 (S m) true G1 (TBind T1) G2 (TBind T2) GH (S n1)
-         
+    stp2 (S m) true G1 (TBind T1) G2 (TBind T2) GH (S (n1+n2))
+
 | stp2_and11: forall m n1 n2 G1 G2 GH T1 T2 T,
     stp2 m true G1 T1 G2 T GH n1 ->
     stp2 m true G1 T2 G1 T2 GH n2 -> (* regularity *)
@@ -500,22 +524,21 @@ Inductive stp2: nat -> bool -> venv -> ty -> venv -> ty -> list (id*(venv*ty)) -
     stp2 m true G1 T1 G1 T1 GH n2 -> (* regularity *)
     stp2 m true G1 (TAnd T1 T2) G2 T GH (S (n1+n2))
 | stp2_and2: forall m n1 n2 G1 G2 GH T1 T2 T,
-    stp2 MAX false G1 T G2 T1 GH n1 ->
-    stp2 MAX false G1 T G2 T2 GH n2 ->
-    stp2 m true G1 T G2 (TAnd T1 T2) GH (S (n1+n2)) 
-
+    stp2 m false G1 T G2 T1 GH n1 ->
+    stp2 m false G1 T G2 T2 GH n2 ->
+    stp2 m true G1 T G2 (TAnd T1 T2) GH (S (n1+n2))
 
 | stp2_wrapf: forall m G1 G2 T1 T2 GH n1,
     stp2 m true G1 T1 G2 T2 GH n1 ->
     stp2 m false G1 T1 G2 T2 GH (S n1)
 | stp2_transf: forall m G1 G2 G3 T1 T2 T3 GH n1 n2,
     stp2 m true G1 T1 G2 T2 GH n1 ->
-    stp2 m false G2 T2 G3 T3 GH n2 ->           
+    stp2 m false G2 T2 G3 T3 GH n2 ->
     stp2 m false G1 T1 G3 T3 GH (S (n1+n2))
 
 
 
-with wf_env : venv -> tenv -> Prop := 
+with wf_env : venv -> tenv -> Prop :=
 | wfe_nil : wf_env nil nil
 | wfe_cons : forall n v t vs ts,
     val_type ((n,v)::vs) v t ->
@@ -535,7 +558,7 @@ with val_type : venv -> vl -> ty -> Prop :=
     has_type ((x,T1)::(f,TFun T1 T2)::tenv) y T2 ->
     fresh venv <= f ->
     1 + f <= x ->
-    (exists n, stp2 0 true venv (TFun T1 T2) env TE [] n)-> 
+    (exists n, stp2 0 true venv (TFun T1 T2) env TE [] n)->
     val_type env (vabs venv f x y) TE
 | v_tabs: forall env venv tenv x y T1 T2 TE,
     wf_env venv tenv ->
@@ -552,13 +575,13 @@ with val_type : venv -> vl -> ty -> Prop :=
 .
 
 
-Inductive wf_envh : venv -> aenv -> tenv -> Prop := 
+Inductive wf_envh : venv -> aenv -> tenv -> Prop :=
 | wfeh_nil : forall vvs, wf_envh vvs nil nil
 | wfeh_cons : forall n t vs vvs ts,
     wf_envh vvs vs ts ->
     wf_envh vvs (cons (n,(vvs,t)) vs) (cons (n,t) ts)
 .
-                 
+
 Inductive valh_type : venv -> aenv -> (venv*ty) -> ty -> Prop :=
 | v_tya: forall aenv venv T1,
     valh_type venv aenv (venv, T1) T1
@@ -592,21 +615,21 @@ Hint Unfold stpd2.
 
 Lemma stpd2_topx: forall G1 G2 GH,
     stpd2 true G1 TTop G2 TTop GH.
-Proof. intros. repeat exists 0. eauto. Qed.
+Proof. intros. repeat exists (S 0). eauto. Qed.
 Lemma stpd2_botx: forall G1 G2 GH,
     stpd2 true G1 TBot G2 TBot GH.
-Proof. intros. repeat exists 0. eauto. Qed.
+Proof. intros. repeat exists (S 0). eauto. Qed.
 Lemma stpd2_top: forall G1 G2 GH T,
-    stpd2 false G1 T G1 T GH ->
+    stpd2 true G1 T G1 T GH ->
     stpd2 true G1 T G2 TTop GH.
 Proof. intros. repeat eu. eauto. Qed.
 Lemma stpd2_bot: forall G1 G2 GH T,
-    stpd2 false G2 T G2 T GH ->
+    stpd2 true G2 T G2 T GH ->
     stpd2 true G1 TBot G2 T GH.
 Proof. intros. repeat eu. eauto. Qed.
 Lemma stpd2_bool: forall G1 G2 GH,
     stpd2 true G1 TBool G2 TBool GH.
-Proof. intros. repeat exists 0. eauto. Qed.
+Proof. intros. repeat exists (S 0). eauto. Qed.
 Lemma stpd2_fun: forall G1 G2 GH T11 T12 T21 T22,
     stpd2 false G2 T21 G1 T11 GH ->
     stpd2 false G1 T12 G2 T22 GH ->
@@ -620,25 +643,28 @@ Proof. intros. repeat eu. eauto. unfold stpd2. eexists. eapply stp2_mem2; eauto.
 
 Lemma stpd2_sel1: forall G1 G2 GX TX x T2 GH v,
     index x G1 = Some v ->
-    val_type GX v TX ->                
+    val_type GX v TX ->
     closed 0 0 TX ->
     stpd2 false GX TX G2 (TMem TBot T2) GH ->
+    stpd2 true G2 T2 G2 T2 GH ->
     stpd2 true G1 (TSel x) G2 T2 GH.
 Proof. intros. repeat eu. eexists. eapply stp2_sel1; eauto. Qed.
 
-Lemma stpd2_sel1b: forall G1 G2 GX TX x T2 GH v,
+Lemma stpd2_selb1: forall G1 G2 GX TX x T2 GH v,
     index x G1 = Some v ->
-    val_type GX v TX ->                
+    val_type GX v TX ->
     closed 0 0 TX ->
     stpd2 false GX TX G2 (TBind (TMem TBot T2)) [] -> (* Note GH = [] *)
+    stpd2 true G2 (open (TSel x) T2) G2 (open (TSel x) T2) GH ->
     stpd2 true G1 (TSel x) G2 (open (TSel x) T2) GH.
-Proof. intros. repeat eu. eexists. eapply stp2_sel1b; eauto. Qed.
+Proof. intros. repeat eu. eexists. eapply stp2_selb1; eauto. Qed.
 
 Lemma stpd2_sel2: forall G1 G2 GX TX x T1 GH v,
     index x G2 = Some v ->
-    val_type GX v TX ->                
+    val_type GX v TX ->
     closed 0 0 TX ->
     stpd2 false GX TX G1 (TMem T1 TTop) GH ->
+    stpd2 true G1 T1 G1 T1 GH ->
     stpd2 true G1 T1 G2 (TSel x) GH.
 Proof. intros. repeat eu. eexists. eapply stp2_sel2; eauto. Qed.
 
@@ -646,61 +672,56 @@ Lemma stpd2_selx: forall G1 G2 x1 x2 GH v,
     index x1 G1 = Some v ->
     index x2 G2 = Some v ->
     stpd2 true G1 (TSel x1) G2 (TSel x2) GH.
-Proof. intros. eauto. exists 0. eapply stp2_selx; eauto. Qed.
+Proof. intros. eauto. exists (S 0). eapply stp2_selx; eauto. Qed.
 
 Lemma stpd2_selab1: forall G1 G2 GX TX x T2 GH,
     indexr x GH = Some (GX, TX) ->
     (* closed 0 x TX -> *)
     stpd2 false GX TX G2 (TBind (TMem TBot T2)) [] -> (* Note GH = [] *)
+    stpd2 true G2 (open (TSelH x) T2) G2 (open (TSelH x) T2) GH ->
     stpd2 true G1 (TSelH x) G2 (open (TSelH x) T2) GH.
 Proof. intros. repeat eu. eauto. eexists. eapply stp2_selab1; eauto. Qed.
 
 Lemma stpd2_sela1: forall G1 G2 GX TX x T2 GH,
     indexr x GH = Some (GX, TX) ->
-    (* closed 0 x TX -> *)
+    closed 0 x TX ->
     stpd2 false GX TX G2 (TMem TBot T2) GH ->
+    stpd2 true G2 T2 G2 T2 GH ->
     stpd2 true G1 (TSelH x) G2 T2 GH.
 Proof. intros. repeat eu. eauto. eexists. eapply stp2_sela1; eauto. Qed.
 
 Lemma stpd2_sela2: forall G1 G2 GX TX x T1 GH,
     indexr x GH = Some (GX, TX) ->
-    (* closed 0 x TX -> *)
+    closed 0 x TX ->
     stpd2 false GX TX G2 (TMem T1 TTop) GH ->
+    stpd2 true G1 T1 G1 T1 GH ->
     stpd2 true G1 T1 G2 (TSelH x) GH.
 Proof. intros. repeat eu. eauto. eexists. eapply stp2_sela2; eauto. Qed.
 
-         
+
 Lemma stpd2_selax: forall G1 G2 GX TX x GH,
     indexr x GH = Some (GX, TX) ->
-    indexr x GH = Some (GX, TX) ->
     stpd2 true G1 (TSelH x) G2 (TSelH x) GH.
-Proof. intros. exists 1. eauto. eapply stp2_selax; eauto. Qed.
+Proof. intros. exists (S 0). eauto. eapply stp2_selax; eauto. Qed.
 
 
-Lemma stpd2_all: forall G1 G2 T1 T2 T3 T4 GH, 
+Lemma stpd2_all: forall G1 G2 T1 T2 T3 T4 GH,
     stpd2 false G2 T3 G1 T1 GH ->
-    closed 1 (length GH) T2 -> 
-    closed 1 (length GH) T4 -> 
+    closed 1 (length GH) T2 ->
+    closed 1 (length GH) T4 ->
+    stpd2 false G1 (open (TSelH (length GH)) T2) G1 (open (TSelH (length GH)) T2) ((0,(G1, T1))::GH) ->
     stpd2 false G1 (open (TSelH (length GH)) T2) G2 (open (TSelH (length GH)) T4) ((0,(G2, T3))::GH) ->
     stpd2 true G1 (TAll T1 T2) G2 (TAll T3 T4) GH.
 Proof. intros. repeat eu. eauto. Qed.
 
-Lemma stpd2_bind: forall G1 G2 T1 T2 GH, 
-    closed 1 (length GH) T1 -> 
-    closed 1 (length GH) T2 -> 
+Lemma stpd2_bind: forall G1 G2 T1 T2 GH,
+    closed 1 (length GH) T1 ->
+    closed 1 (length GH) T2 ->
+    stpd2 false G2 (open (TSelH (length GH)) T2) G2 (open (TSelH (length GH)) T2) ((0,(G2, open (TSelH (length GH)) T2))::GH) ->
     stpd2 false G1 (open (TSelH (length GH)) T1) G2 (open (TSelH (length GH)) T2) ((0,(G1, open (TSelH (length GH)) T1))::GH) ->
     stpd2 true G1 (TBind T1) G2 (TBind T2) GH.
 Proof. intros. repeat eu. eauto. unfold stpd2. eexists. eapply stp2_bindb; eauto. Qed.
 
-Lemma stpd2_wrapf: forall G1 G2 T1 T2 GH,
-    stpd2 true G1 T1 G2 T2 GH ->
-    stpd2 false G1 T1 G2 T2 GH.
-Proof. intros. repeat eu. eauto. Qed.
-Lemma stpd2_transf: forall G1 G2 G3 T1 T2 T3 GH,
-    stpd2 true G1 T1 G2 T2 GH ->
-    stpd2 false G2 T2 G3 T3 GH ->           
-    stpd2 false G1 T1 G3 T3 GH.
-Proof. intros. repeat eu. eauto. Qed.
 Lemma stpd2_and11: forall G1 G2 GH T1 T2 T,
     stpd2 true G1 T1 G2 T GH ->
     stpd2 true G1 T2 G1 T2 GH ->
@@ -716,6 +737,35 @@ Lemma stpd2_and2: forall G1 G2 GH T1 T2 T,
     stpd2 false G1 T G2 T2 GH ->
     stpd2 true G1 T G2 (TAnd T1 T2) GH.
 Proof. intros. repeat eu. eauto. Qed.
+
+Lemma stpd2_wrapf: forall G1 G2 T1 T2 GH,
+    stpd2 true G1 T1 G2 T2 GH ->
+    stpd2 false G1 T1 G2 T2 GH.
+Proof. intros. repeat eu. eauto. Qed.
+Lemma stpd2_transf: forall G1 G2 G3 T1 T2 T3 GH,
+    stpd2 true G1 T1 G2 T2 GH ->
+    stpd2 false G2 T2 G3 T3 GH ->
+    stpd2 false G1 T1 G3 T3 GH.
+Proof. intros. repeat eu. eauto. Qed.
+
+
+Lemma sstpd2_wrapf: forall G1 G2 T1 T2 GH,
+    sstpd2 true G1 T1 G2 T2 GH ->
+    sstpd2 false G1 T1 G2 T2 GH.
+Proof. intros. repeat eu. eexists. eapply stp2_wrapf. eauto. Qed.
+Lemma sstpd2_transf: forall G1 G2 G3 T1 T2 T3 GH,
+    sstpd2 true G1 T1 G2 T2 GH ->
+    sstpd2 false G2 T2 G3 T3 GH ->
+    sstpd2 false G1 T1 G3 T3 GH.
+Proof. intros. repeat eu. eexists. eapply stp2_transf; eauto. Qed.
+
+
+Lemma atpd2_transf: forall G1 G2 G3 T1 T2 T3 GH,
+    atpd2 true G1 T1 G2 T2 GH ->
+    atpd2 false G2 T2 G3 T3 GH ->
+    atpd2 false G1 T1 G3 T3 GH.
+Proof. intros. repeat eu. eexists. eapply stp2_transf; eauto. Qed.
+
 (*
 None             means timeout
 Some None        means stuck
@@ -840,11 +890,17 @@ Proof.
     { eapply t_sub.
       { eapply t_var. simpl. eauto. }
       { eapply stp_all; eauto. { eapply stp_bindx; crush2. } compute. eapply cl_fun; eauto.
-        eapply stp_fun. compute. eapply stp_selab2. crush2. crush2. instantiate (1:=TBool). crush2. crush2. compute. eapply stp_selab1; crush2. instantiate(1:=TBool). crush2. crush2. } }
+        eapply stp_fun. compute. eapply stp_selax; crush2. crush2.
+        eapply stp_fun. compute. eapply stp_selab2. crush2.
+        instantiate (1:=TBool). crush2. crush2. crush2.
+        simpl. eapply stp_selab1. crush2.
+        instantiate (1:=TBool). crush2. crush2. crush2.
+      }
+    }
     { eapply t_typ; crush2. }
     crush2.
 Qed.
-       
+
 
 
 (* define brand / unbrand client function *)
@@ -875,9 +931,11 @@ Example ex4:
   has_type [(1,TFun TBool TBool);(0,brandUnbrand)]
            (tvar 0) (TAll (TBind (TMem TBool TBool)) (TFun (TFun TBool TBool) (TFun (TFun TBool TBool) TBool))).
 Proof.
-  eapply t_sub. crush2. crush2. eapply stp_all; crush2. compute. eapply stp_fun. eapply stp_fun. crush2. eapply stp_selab2; crush2. instantiate(1:=TBool). crush2. crush2.
-  eapply stp_fun. crush2. eapply stp_fun. eapply stp_selab1; crush2. instantiate(1:=TBool). crush2. crush2. crush2.
-  crush2.
+  eapply t_sub. crush2. crush2. eapply stp_all; crush2. compute. eapply stp_fun. eapply stp_fun. crush2.
+  eapply stp_selab2. crush2. instantiate(1:=TBool). crush2. crush2. crush2.
+  eapply stp_fun. crush2. eapply stp_fun.
+  eapply stp_selab1. crush2. instantiate(1:=TBool). crush2. crush2. crush2.
+  crush2. crush2.
 Qed.
 
 Hint Resolve ex4.
@@ -906,7 +964,7 @@ Qed.
 
 
 Example ex7:
-  stp [(1,TSel 0);(0,TMem TBot (TBind (TMem TBot (TFun TBool (TSelB 0)))))] [] None
+  stp [(1,TSel 0);(0,TMem TBot (TBind (TMem TBot (TFun TBool (TSelB 0)))))] []
            (TSel 1) (TFun TBool(TSel 1)).
 Proof.
   remember (TFun TBool (TSel 1)) as T.
@@ -914,8 +972,11 @@ Proof.
   rewrite H.
   eapply stp_selb1. compute. eauto.
   eapply stp_sel1. compute. eauto.
+  crush2.
   eapply stp_mem. eauto.
-  eapply stp_bindx. eauto. crush2. crush2. crush2.
+  eapply stp_bindx; crush2.
+  eapply stp_bindx; crush2.
+  crush2.
 Qed.
 
 
@@ -987,7 +1048,7 @@ Proof.
     + SSCase "miss".
       rewrite E2 in H1.
       assert (n < length vs). eapply IHvs. apply H1.
-      compute. eauto. 
+      compute. eauto.
 Qed.
 
 
@@ -997,13 +1058,13 @@ Lemma le_xx : forall a b,
                        exists E, le_lt_dec a b = left E.
 Proof. intros.
   case_eq (le_lt_dec a b). intros. eauto.
-  intros. omega.     
+  intros. omega.
 Qed.
 Lemma le_yy : forall a b,
                        a > b ->
                        exists E, le_lt_dec a b = right E.
 Proof. intros.
-  case_eq (le_lt_dec a b). intros. omega. 
+  case_eq (le_lt_dec a b). intros. omega.
   intros. eauto.
 Qed.
 
@@ -1056,25 +1117,32 @@ Definition splicett n (V: (id*ty)) :=
     | (x,T) => (x,(splice n T))
   end.
 
-Lemma splice_open_permute: forall (G0:tenv) T2 n j,
-(open_rec j (TSelH (n + S (length G0))) (splice (length G0) T2)) = 
-(splice (length G0) (open_rec j (TSelH (n + length G0)) T2)).
+Definition spliceat n (V: (id*(venv*ty))) :=
+  match V with
+    | (x,(G,T)) => (x,(G,splice n T))
+  end.
+
+Lemma splice_open_permute: forall {X} (G:list (id*X)) T n j k,
+n + k >= length G ->
+(open_rec j (TSelH (n + S k)) (splice (length G) T)) =
+(splice (length G) (open_rec j (TSelH (n + k)) T)).
 Proof.
-  intros G T. induction T; intros; simpl; eauto;
+  intros X G T. induction T; intros; simpl; eauto;
   try rewrite IHT1; try rewrite IHT2; try rewrite IHT; eauto.
-  
+
   case_eq (le_lt_dec (length G) i); intros E LE; simpl; eauto.
   case_eq (beq_nat j i); intros E; simpl; eauto.
   case_eq (le_lt_dec (length G) (n + length G)); intros EL LE.
   assert (n + S (length G) = n + length G + 1). omega.
-  rewrite H. eauto.
-  omega.
+  case_eq (le_lt_dec (length G) (n+k)); intros E' LE'; simpl; eauto.
+  assert (n + S k=n + k + 1) as R by omega. rewrite R. reflexivity.
+  omega. omega.
 Qed.
 
 Lemma indexr_splice_hi: forall G0 G2 x0 x v1 T,
     indexr x0 (G2 ++ G0) = Some T ->
     length G0 <= x0 ->
-    indexr (x0 + 1) (map (splicett (length G0)) (G2 ++ (x, v1) :: G0)) = Some (splice (length G0) T).
+    indexr (x0 + 1) (map (splicett (length G0)) G2 ++ (x, v1) :: G0) = Some (splice (length G0) T).
 Proof.
   intros G0 G2. induction G2; intros.
   - eapply indexr_max in H. simpl in H. omega.
@@ -1082,112 +1150,1133 @@ Proof.
     case_eq (beq_nat x0 (length (G2 ++ G0))); intros E.
     + rewrite E in H. inversion H. subst. simpl.
       rewrite app_length in E.
-      rewrite map_length. rewrite app_length. simpl.
+      rewrite app_length. rewrite map_length. simpl.
       assert (beq_nat (x0 + 1) (length G2 + S (length G0)) = true). eapply beq_nat_true_iff. eapply beq_nat_true_iff in E. omega.
       rewrite H1. eauto.
     + rewrite E in H.  eapply IHG2 in H. eapply indexr_extend. eapply H. eauto.
 Qed.
 
-Lemma indexr_splice_lo0: forall G0 G2 x0 (T:ty),
+Lemma indexr_spliceat_hi: forall G0 G2 x0 x v1 G T,
+    indexr x0 (G2 ++ G0) = Some (G, T) ->
+    length G0 <= x0 ->
+    indexr (x0 + 1) (map (spliceat (length G0)) G2 ++ (x, v1) :: G0) = Some (G, splice (length G0) T).
+Proof.
+  intros G0 G2. induction G2; intros.
+  - eapply indexr_max in H. simpl in H. omega.
+  - simpl in H. destruct a.
+    case_eq (beq_nat x0 (length (G2 ++ G0))); intros E.
+    + rewrite E in H. inversion H. subst. simpl.
+      rewrite app_length in E.
+      rewrite app_length. rewrite map_length. simpl.
+      assert (beq_nat (x0 + 1) (length G2 + S (length G0)) = true). eapply beq_nat_true_iff. eapply beq_nat_true_iff in E. omega.
+      rewrite H1. eauto.
+    + rewrite E in H.  eapply IHG2 in H. destruct p. eapply indexr_extend. eapply H. eauto.
+Qed.
+
+Lemma plus_lt_contra: forall a b,
+  a + b < b -> False.
+Proof.
+  intros a b H. induction a.
+  - simpl in H. apply lt_irrefl in H. assumption.
+  - simpl in H. apply IHa. omega.
+Qed.
+
+Lemma indexr_splice_lo0: forall {X} G0 G2 x0 (T:X),
     indexr x0 (G2 ++ G0) = Some T ->
     x0 < length G0 ->
     indexr x0 G0 = Some T.
-Proof. admit. Qed.
+Proof.
+  intros X G0 G2. induction G2; intros.
+  - simpl in H. apply H.
+  - simpl in H. destruct a.
+    case_eq (beq_nat x0 (length (G2 ++ G0))); intros E.
+    + eapply beq_nat_true_iff in E. subst.
+      rewrite app_length in H0. apply plus_lt_contra in H0. inversion H0.
+    + rewrite E in H. apply IHG2. apply H. apply H0.
+Qed.
 
-Lemma indexr_splice_lo1: forall G0 x0 (T:ty) f,
-    indexr x0 G0 = Some T ->
-    map (splicett f) G0 = G0 ->
-    indexr x0 G0 = Some (splice f T).
-Proof. admit. Qed.
-
-Lemma indexr_extend_mult: forall G0 G2 x0 (T:ty),
+Lemma indexr_extend_mult: forall {X} G0 G2 x0 (T:X),
     indexr x0 G0 = Some T ->
     indexr x0 (G2++G0) = Some T.
-Proof. admit. Qed.
-
+Proof.
+  intros X G0 G2. induction G2; intros.
+  - simpl. assumption.
+  - destruct a. simpl.
+    case_eq (beq_nat x0 (length (G2 ++ G0))); intros E.
+    + eapply beq_nat_true_iff in E.
+      apply indexr_max in H. subst.
+      rewrite app_length in H. apply plus_lt_contra in H. inversion H.
+    + apply IHG2. assumption.
+Qed.
 
 Lemma indexr_splice_lo: forall G0 G2 x0 x v1 T f,
     indexr x0 (G2 ++ G0) = Some T ->
-    map (splicett f) G0 = G0 ->
     x0 < length G0 ->
-    indexr x0 (map (splicett f) (G2 ++ (x, v1) :: G0)) = Some (splice f T).
+    indexr x0 (map (splicett f) G2 ++ (x, v1) :: G0) = Some T.
 Proof.
   intros.
   assert (indexr x0 G0 = Some T). eapply indexr_splice_lo0; eauto.
-  assert (indexr x0 (map (splicett f) G0) = Some (splice f T)).
-  rewrite H0. eapply indexr_splice_lo1. eauto. eauto.
-  rewrite map_app. simpl.
   eapply indexr_extend_mult. eapply indexr_extend. eauto.
-Qed.  
+Qed.
 
-
-Lemma stp_splice : forall GX G0 G1 T1 T2 S x v1,
-   stp GX (G1++G0) S T1 T2 ->
-   map (splicett (length G0)) G0 = G0 ->                  
-   stp GX (map (splicett (length G0)) (G1++(x,v1)::G0)) S (splice (length G0) T1) (splice (length G0) T2).
+Lemma indexr_spliceat_lo: forall G0 G2 x0 x v1 G T f,
+    indexr x0 (G2 ++ G0) = Some (G, T) ->
+    x0 < length G0 ->
+    indexr x0 (map (spliceat f) G2 ++ (x, v1) :: G0) = Some (G, T).
 Proof.
-  admit. (*
-  intros GX G0 G1 T1 T2 S x v1 H. remember (G1++G0) as G. remember S as S'.
-  revert G0 G1 HeqG S HeqS'.
+  intros.
+  assert (indexr x0 G0 = Some (G, T)). eapply indexr_splice_lo0; eauto.
+  eapply indexr_extend_mult. eapply indexr_extend. eauto.
+Qed.
+
+
+Lemma fresh_splice_ctx: forall G n,
+  fresh G = fresh (map (splicett n) G).
+Proof.
+  intros. induction G.
+  - simpl. reflexivity.
+  - destruct a. simpl. reflexivity.
+Qed.
+
+Lemma index_splice_ctx: forall G x T n,
+  index x G = Some T ->
+  index x (map (splicett n) G) = Some (splice n T).
+Proof.
+  intros. induction G.
+  - simpl in H. inversion H.
+  - destruct a. simpl in H.
+    case_eq (le_lt_dec (fresh G) i); intros E LE; rewrite LE in H.
+    case_eq (beq_nat x i); intros Eq; rewrite Eq in H.
+    inversion H. simpl. erewrite <- (fresh_splice_ctx). rewrite LE.
+    rewrite Eq. reflexivity.
+    simpl. erewrite <- (fresh_splice_ctx). rewrite LE.
+    rewrite Eq. apply IHG. apply H.
+    inversion H.
+Qed.
+
+Lemma closed_splice: forall j l T n,
+  closed j l T ->
+  closed j (S l) (splice n T).
+Proof.
+  intros. induction H; simpl; eauto.
+  case_eq (le_lt_dec n x); intros E LE.
+  unfold closed. apply cl_selh. omega.
+  unfold closed. apply cl_selh. omega.
+Qed.
+
+Lemma map_splice_length_inc: forall G0 G2 x v1,
+   (length (map (splicett (length G0)) G2 ++ (x, v1) :: G0)) = (S (length (G2 ++ G0))).
+Proof.
+  intros. rewrite app_length. rewrite map_length. induction G2.
+  - simpl. reflexivity.
+  - simpl. eauto.
+Qed.
+
+Lemma map_spliceat_length_inc: forall G0 G2 x v1,
+   (length (map (spliceat (length G0)) G2 ++ (x, v1) :: G0)) = (S (length (G2 ++ G0))).
+Proof.
+  intros. rewrite app_length. rewrite map_length. induction G2.
+  - simpl. reflexivity.
+  - simpl. eauto.
+Qed.
+
+Lemma closed_inc: forall j l T,
+  closed j l T ->
+  closed j (S l) T.
+Proof.
+  intros. induction H; simpl; eauto.
+  unfold closed. apply cl_selh. omega.
+Qed.
+
+Lemma closed_inc_mult: forall j l l' T,
+  closed j l T ->
+  l' >= l ->
+  closed j l' T.
+Proof.
+  intros j l l' T H LE. induction LE.
+  - assumption.
+  - apply closed_inc. assumption.
+Qed.
+
+Ltac sp :=
+  match goal with
+    | A : ?P, H : ?P -> _ |- _ => specialize (H A)
+  end.
+
+Lemma closed_splice_idem: forall k l T n,
+                            closed k l T ->
+                            n >= l ->
+                            splice n T = T.
+Proof.
+  intros. induction H; simpl; repeat sp; repeat (match goal with
+    | H: splice ?N ?T = ?T |- _ => rewrite H
+  end); eauto.
+  case_eq (le_lt_dec n x); intros E LE. omega. reflexivity.
+Qed.
+
+Ltac ev := repeat match goal with
+                    | H: exists _, _ |- _ => destruct H
+                    | H: _ /\  _ |- _ => destruct H
+           end.
+
+Lemma closed_upgrade: forall i j l T,
+ closed_rec i l T ->
+ j >= i ->
+ closed_rec j l T.
+Proof.
+ intros. generalize dependent j. induction H; intros; eauto.
+ Case "TAll". econstructor. eapply IHclosed_rec1. omega. eapply IHclosed_rec2. omega.
+ Case "TBind". econstructor. eapply IHclosed_rec. omega.
+ Case "TSelB". econstructor. omega.
+Qed.
+
+Lemma closed_upgrade_free: forall i l k T,
+ closed_rec i l T ->
+ k >= l ->
+ closed_rec i k T.
+Proof.
+ intros. generalize dependent k. induction H; intros; eauto.
+ Case "TSelH". econstructor. omega.
+Qed.
+
+
+Lemma closed_open: forall j n TX T, closed (j+1) n T -> closed j n TX -> closed j n (open_rec j TX T).
+Proof.
+  intros. generalize dependent j. induction T; intros; inversion H; unfold closed; try econstructor; try eapply IHT1; eauto; try eapply IHT2; eauto; try eapply IHT; eauto. eapply closed_upgrade. eauto. eauto.
+
+  - Case "TSelB". simpl.
+    case_eq (beq_nat j i); intros E. eauto.
+
+    econstructor. eapply beq_nat_false_iff in E. omega.
+
+  - eauto.
+  - eapply closed_upgrade; eauto.
+  - eapply closed_upgrade; eauto.
+Qed.
+
+Lemma stp_closed : forall G GH T1 T2,
+                     stp G GH T1 T2 ->
+                     closed 0 (length GH) T1 /\ closed 0 (length GH) T2.
+Proof.
+  intros. induction H;
+    try solve [repeat ev; split; eauto using indexr_max];
+    try solve [try inversion IHstp; split; eauto; apply cl_selh; eapply indexr_max; eassumption];
+    try solve [inversion IHstp1 as [IH1 IH2]; inversion IH2; split; eauto; apply cl_selh; eapply indexr_max; eassumption].
+Qed.
+
+Lemma stp_closed2 : forall G1 GH T1 T2,
+                       stp G1 GH T1 T2 ->
+                       closed 0 (length GH) T2.
+Proof.
+  intros. apply (proj2 (stp_closed G1 GH T1 T2 H)).
+Qed.
+
+Lemma stp_closed1 : forall G1 GH T1 T2,
+                       stp G1 GH T1 T2 ->
+                       closed 0 (length GH) T1.
+Proof.
+  intros. apply (proj1 (stp_closed G1 GH T1 T2 H)).
+Qed.
+
+Lemma stp2_closed: forall G1 G2 T1 T2 GH s m n1,
+                     stp2 s m G1 T1 G2 T2 GH n1 ->
+                     closed 0 (length GH) T1 /\ closed 0 (length GH) T2.
+  intros. induction H;
+    try solve [repeat ev; split; eauto];
+    try solve [try inversion IHstp2_1; try inversion IHstp2_2; split; eauto; apply cl_selh; eapply indexr_max; eassumption];
+    try solve [inversion IHstp2 as [IH1 IH2]; inversion IH2; split; eauto; apply cl_selh; eapply indexr_max; eassumption].
+Qed.
+
+Lemma stp2_closed2 : forall G1 G2 T1 T2 GH s m n1,
+                       stp2 s m G1 T1 G2 T2 GH n1 ->
+                       closed 0 (length GH) T2.
+Proof.
+  intros. apply (proj2 (stp2_closed G1 G2 T1 T2 GH s m n1 H)).
+Qed.
+
+Lemma stp2_closed1 : forall G1 G2 T1 T2 GH s m n1,
+                       stp2 s m G1 T1 G2 T2 GH n1 ->
+                       closed 0 (length GH) T1.
+Proof.
+  intros. apply (proj1 (stp2_closed G1 G2 T1 T2 GH s m n1 H)).
+Qed.
+
+Lemma stp_splice : forall GX G0 G1 T1 T2 x v1,
+   stp GX (G1++G0) T1 T2 ->
+   stp GX ((map (splicett (length G0)) G1) ++ (x,v1)::G0) (splice (length G0) T1) (splice (length G0) T2).
+Proof.
+  intros GX G0 G1 T1 T2 x v1 H. remember (G1++G0) as G.
+  revert G0 G1 HeqG.
   induction H; intros; subst GH; simpl; eauto.
-  - admit.
-  - admit.
+  - Case "sel1".
+    eapply stp_sel1. apply H. assumption.
+    assert (splice (length G0) TX=TX) as A. {
+      eapply closed_splice_idem. eassumption. omega.
+    }
+    rewrite <- A. apply IHstp1. reflexivity.
+    apply IHstp2. reflexivity.
+  - Case "sel2".
+    eapply stp_sel2. apply H. assumption.
+    assert (splice (length G0) TX=TX) as A. {
+      eapply closed_splice_idem. eassumption. omega.
+    }
+    rewrite <- A. apply IHstp1. reflexivity.
+    apply IHstp2. reflexivity.
+  - Case "selb1".
+    assert (splice (length G0) (open (TSel x0) T2)=(open (TSel x0) T2)) as A. {
+      eapply closed_splice_idem. apply stp_closed2 in H0. inversion H0. subst.
+      simpl in H5. inversion H5. subst.
+      eapply closed_open. simpl. eassumption. eauto.
+      omega.
+    }
+    rewrite A. eapply stp_selb1; eauto.
+    rewrite <- A. apply IHstp2; eauto.
+  - Case "selb2".
+    assert (splice (length G0) (open (TSel x0) T1)=(open (TSel x0) T1)) as A. {
+      eapply closed_splice_idem. apply stp_closed2 in H0. inversion H0. subst.
+      simpl in H5. inversion H5. subst.
+      eapply closed_open. simpl. eassumption. eauto.
+      omega.
+    }
+    rewrite A. eapply stp_selb2; eauto.
+    rewrite <- A. apply IHstp2; eauto.
   - Case "sela1".
     case_eq (le_lt_dec (length G0) x0); intros E LE.
-    + eapply stp_sela1. eapply indexr_splice_hi with (T:=TX). eauto. eauto.
-      eapply IHstp. eauto. eauto. eauto.
-    + eapply stp_sela1. eapply indexr_splice_lo with (T:=TX). eauto. eauto. eauto.
-      eapply IHstp. eauto. eauto. eauto.
-  - Case "sela2". admit.
+    + eapply stp_sela1. eapply indexr_splice_hi. eauto. eauto.
+      eapply closed_splice in H0. assert (S x0 = x0 +1) as A by omega.
+      rewrite <- A. eapply H0.
+      eapply IHstp1. eauto.
+      eapply IHstp2. eauto.
+    + eapply stp_sela1. eapply indexr_splice_lo. eauto. eauto. eauto. eauto.
+      assert (splice (length G0) TX=TX) as A. {
+        eapply closed_splice_idem. eassumption. omega.
+      }
+      rewrite <- A. eapply IHstp1. eauto.
+      eapply IHstp2. eauto.
+  - Case "sela2".
+    case_eq (le_lt_dec (length G0) x0); intros E LE.
+    + eapply stp_sela2. eapply indexr_splice_hi. eauto. eauto.
+      eapply closed_splice in H0. assert (S x0 = x0 +1) as A by omega.
+      rewrite <- A. eapply H0.
+      eapply IHstp1. eauto.
+      eapply IHstp2. eauto.
+    + eapply stp_sela2. eapply indexr_splice_lo. eauto. eauto. eauto. eauto.
+      assert (splice (length G0) TX=TX) as A. {
+        eapply closed_splice_idem. eassumption. omega.
+      }
+      rewrite <- A. eapply IHstp1. eauto.
+      eapply IHstp2. eauto.
+  - Case "selab1".
+    case_eq (le_lt_dec (length G0) x0); intros E LE.
+    + eapply stp_selab1.
+      eapply indexr_splice_hi; eauto.
+      instantiate (1:=T2).
+      assert (splice (length G0) TX=TX) as A. {
+        apply stp_closed1 in H0. simpl in H0.
+        eapply closed_splice_idem.
+        apply H0.
+        omega.
+      }
+      rewrite A. apply H0.
+      rewrite H1.
+      unfold open.
+      assert (TSelH x0=TSelH (x0+0)) as B. {
+        rewrite <- plus_n_O. reflexivity.
+      }
+      rewrite B. rewrite <- splice_open_permute.
+      assert (splice (length G0) T2=T2) as C. {
+        apply stp_closed2 in H0. simpl in H0. inversion H0; subst.
+        inversion H6; subst.
+        eapply closed_splice_idem. eassumption. omega.
+      }
+      rewrite C. reflexivity. omega.
+      apply IHstp2; eauto.
+    + eapply stp_selab1.
+      eapply indexr_splice_lo; eauto.
+      eassumption.
+      rewrite H1.
+      apply stp_closed2 in H0. simpl in H0. inversion H0; subst.
+      inversion H6; subst.
+      apply closed_upgrade_free with (k:=(length G0)) in H8.
+      eapply closed_splice_idem. eapply closed_open. eassumption. apply cl_selh.
+      omega. omega. omega.
+      apply IHstp2; eauto.
+  - Case "selab2".
+    case_eq (le_lt_dec (length G0) x0); intros E LE.
+    + eapply stp_selab2.
+      eapply indexr_splice_hi; eauto.
+      instantiate (1:=T1).
+      assert (splice (length G0) TX=TX) as A. {
+        apply stp_closed1 in H0. simpl in H0.
+        eapply closed_splice_idem.
+        apply H0.
+        omega.
+      }
+      rewrite A. apply H0.
+      rewrite H1.
+      unfold open.
+      assert (TSelH x0=TSelH (x0+0)) as B. {
+        rewrite <- plus_n_O. reflexivity.
+      }
+      rewrite B. rewrite <- splice_open_permute.
+      assert (splice (length G0) T1=T1) as C. {
+        apply stp_closed2 in H0. simpl in H0. inversion H0; subst.
+        inversion H6; subst.
+        eapply closed_splice_idem. eassumption. omega.
+      }
+      rewrite C. reflexivity. omega.
+      apply IHstp2; eauto.
+    + eapply stp_selab2.
+      eapply indexr_splice_lo; eauto.
+      eassumption.
+      rewrite H1.
+      apply stp_closed2 in H0. simpl in H0. inversion H0; subst.
+      inversion H6; subst.
+      apply closed_upgrade_free with (k:=(length G0)) in H7.
+      eapply closed_splice_idem. eapply closed_open. eassumption. apply cl_selh.
+      omega. omega. omega.
+      apply IHstp2; eauto.
   - Case "selax".
     case_eq (le_lt_dec (length G0) x0); intros E LE.
-    + eapply stp_selax. eapply indexr_splice_hi with (T:=TX). eauto. eauto.
-    + eapply stp_selax. eapply indexr_splice_lo with (T:=TX). eauto. eauto. eauto.
+    + eapply stp_selax. eapply indexr_splice_hi. eauto. eauto.
+    + eapply stp_selax. eapply indexr_splice_lo. eauto. eauto.
   - Case "all".
     eapply stp_all.
-    eapply IHstp1. eauto. eauto. eauto. eauto.
-    admit. (* closed *) 
-    admit. (* closed *)
+    eapply IHstp1. eauto. eauto. eauto.
 
-    specialize IHstp2 with (G3:=G0) (G4:=(0, T3) :: G2).
-    simpl in IHstp2. rewrite map_length. rewrite app_length. simpl.
+    simpl. rewrite map_splice_length_inc. apply closed_splice. assumption.
+
+    simpl. rewrite map_splice_length_inc. apply closed_splice. assumption.
+
+    specialize IHstp2 with (G3:=G0) (G4:=(0, T1) :: G2).
+    simpl in IHstp2. rewrite app_length. rewrite map_length. simpl.
     repeat rewrite splice_open_permute with (j:=0). subst x0.
     rewrite app_length in IHstp2. simpl in IHstp2.
-    eapply IHstp2. eauto. eauto. eauto.
-  - Case "bind". admit.
-  - Case "bind1". admit.
-  - Case "bind2". admit.*)
+    eapply IHstp2. eauto. omega.
+
+    specialize IHstp3 with (G3:=G0) (G4:=(0, T3) :: G2).
+    simpl in IHstp2. rewrite app_length. rewrite map_length. simpl.
+    repeat rewrite splice_open_permute with (j:=0). subst x0.
+    rewrite app_length in IHstp3. simpl in IHstp3.
+    eapply IHstp3. eauto. omega. omega.
+
+  - Case "bind".
+    eapply stp_bindx.
+    eauto.
+
+    rewrite map_splice_length_inc. apply closed_splice. assumption.
+    rewrite map_splice_length_inc. apply closed_splice. assumption.
+
+    rewrite app_length. rewrite map_length. simpl.
+    repeat rewrite splice_open_permute with (j:=0). subst x0.
+    specialize IHstp1 with (G3:=G0) (G4:=(0, (open (TSelH (length G2 + length G0)) T2))::G2).
+    rewrite app_length in IHstp1. simpl in IHstp1. unfold open in IHstp1.
+    eapply IHstp1. eauto. omega.
+
+    rewrite app_length. rewrite map_length. simpl.
+    repeat rewrite splice_open_permute with (j:=0). subst x0.
+    specialize IHstp2 with (G3:=G0) (G4:=(0, (open (TSelH (length G2 + length G0)) T1))::G2).
+    rewrite app_length in IHstp2. simpl in IHstp2. unfold open in IHstp2.
+    eapply IHstp2. eauto. omega. omega.
 Qed.
 
-
-
-
-Lemma stp_extend : forall G1 GH S T1 T2 x v1,
-                       stp G1 GH S T1 T2 ->
-                       stp G1 ((x,v1)::GH) S T1 T2.
+Lemma stp2_splice : forall G1 T1 G2 T2 GH1 GH0 x v1 s m n1,
+   stp2 s m G1 T1 G2 T2 (GH1++GH0) n1 ->
+   stp2 s m G1 (splice (length GH0) T1) G2 (splice (length GH0) T2) ((map (spliceat (length GH0)) GH1) ++ (x,v1)::GH0) n1.
 Proof.
-  (* use stp_splice: we need to have that env and types are well-formed *)
-  admit.
+  intros G1 T1 G2 T2 GH1 GH0 x v1 s m n1 H. remember (GH1++GH0) as GH.
+  revert GH0 GH1 HeqGH.
+  induction H; intros; subst GH; simpl; eauto.
+  - Case "strong_sel1".
+    eapply stp2_strong_sel1. apply H. assumption. (*assumption.*)
+    assert (splice (length GH0) TX=TX) as A. {
+      eapply closed_splice_idem. eassumption. omega.
+    }
+    rewrite <- A. apply IHstp2.
+    reflexivity.
+  - Case "strong_sel2".
+    eapply stp2_strong_sel2. apply H. assumption. (*assumption.*)
+    assert (splice (length GH0) TX=TX) as A. {
+      eapply closed_splice_idem. eassumption. omega.
+    }
+    rewrite <- A. apply IHstp2.
+    reflexivity.
+  - Case "sel1".
+    eapply stp2_sel1. apply H. eassumption. assumption.
+    assert (splice (length GH0) TX=TX) as A. {
+      eapply closed_splice_idem. eassumption. omega.
+    }
+    rewrite <- A. apply IHstp2_1.
+    reflexivity.
+    apply IHstp2_2. reflexivity.
+
+  - Case "selb1".
+    assert (splice (length GH0) (open (TSel x0) T2)=(open (TSel x0) T2)) as A. {
+      eapply closed_splice_idem. apply stp2_closed2 in H2. inversion H2. subst.
+      simpl in H7. inversion H7. subst.
+      eapply closed_open. simpl. eassumption. eauto.
+      omega.
+    }
+    rewrite A. eapply stp2_selb1; eauto.
+    rewrite <- A. apply IHstp2_2; eauto.
+  - Case "sel2".
+    eapply stp2_sel2. apply H. eassumption. assumption.
+    assert (splice (length GH0) TX=TX) as A. {
+      eapply closed_splice_idem. eassumption. omega.
+    }
+    rewrite <- A. apply IHstp2_1.
+    reflexivity.
+    apply IHstp2_2. reflexivity.
+  - Case "sela1".
+    case_eq (le_lt_dec (length GH0) x0); intros E LE.
+    + eapply stp2_sela1. eapply indexr_spliceat_hi. apply H. eauto.
+      eapply closed_splice in H0. assert (S x0 = x0 +1) as EQ by omega. rewrite <- EQ.
+      eapply H0.
+      eapply IHstp2_1. eauto.
+      eapply IHstp2_2. eauto.
+    + eapply stp2_sela1. eapply indexr_spliceat_lo. apply H. eauto. eauto.
+      assert (splice (length GH0) TX=TX) as A. {
+        eapply closed_splice_idem. eassumption. omega.
+      }
+      rewrite <- A. eapply IHstp2_1. eauto. eapply IHstp2_2. eauto.
+
+  - Case "selab1".
+    case_eq (le_lt_dec (length GH0) x0); intros E LE.
+    + eapply stp2_selab1.
+      eapply indexr_spliceat_hi; eauto.
+      instantiate (1:=T2).
+      assert (splice (length GH0) TX=TX) as A. {
+        apply stp2_closed1 in H0. simpl in H0.
+        eapply closed_splice_idem.
+        apply H0.
+        omega.
+      }
+      rewrite A. apply H0.
+      rewrite H1.
+      unfold open.
+      assert (TSelH x0=TSelH (x0+0)) as B. {
+        rewrite <- plus_n_O. reflexivity.
+      }
+      rewrite B. rewrite <- splice_open_permute.
+      assert (splice (length GH0) T2=T2) as C. {
+        apply stp2_closed2 in H0. simpl in H0. inversion H0; subst.
+        inversion H6; subst.
+        eapply closed_splice_idem. eassumption. omega.
+      }
+      rewrite C. reflexivity. omega.
+      apply IHstp2_2; eauto.
+    + eapply stp2_selab1.
+      eapply indexr_spliceat_lo; eauto.
+      eassumption.
+      rewrite H1.
+      apply stp2_closed2 in H0. simpl in H0. inversion H0; subst.
+      inversion H6; subst.
+      apply closed_upgrade_free with (k:=(length GH0)) in H8.
+      eapply closed_splice_idem. eapply closed_open. eassumption. apply cl_selh.
+      omega. omega. omega.
+      apply IHstp2_2; eauto.
+  - Case "sela2".
+    case_eq (le_lt_dec (length GH0) x0); intros E LE.
+    + eapply stp2_sela2. eapply indexr_spliceat_hi. apply H. eauto.
+      eapply closed_splice in H0. assert (S x0 = x0 +1) as EQ by omega. rewrite <- EQ.
+      eapply H0.
+      eapply IHstp2_1. eauto.
+      eapply IHstp2_2. eauto.
+    + eapply stp2_sela2. eapply indexr_spliceat_lo. apply H. eauto. eauto.
+      assert (splice (length GH0) TX=TX) as A. {
+        eapply closed_splice_idem. eassumption. omega.
+      }
+      rewrite <- A. eapply IHstp2_1. eauto. eapply IHstp2_2. eauto.
+  - Case "selax".
+    case_eq (le_lt_dec (length GH0) x0); intros E LE.
+    + eapply stp2_selax.
+      eapply indexr_spliceat_hi. apply H. eauto.
+    + eapply stp2_selax.
+      eapply indexr_spliceat_lo. apply H. eauto.
+  - Case "all".
+    eapply stp2_all.
+    eapply IHstp2_1. reflexivity.
+
+    simpl. rewrite map_spliceat_length_inc. apply closed_splice. assumption.
+
+    simpl. rewrite map_spliceat_length_inc. apply closed_splice. assumption.
+
+    specialize IHstp2_2 with (GH2:=GH0) (GH3:=(0, (G1, T1)) :: GH1).
+    simpl in IHstp2_2. rewrite app_length. rewrite map_length. simpl.
+    repeat rewrite splice_open_permute with (j:=0).
+    rewrite app_length in IHstp2_2. simpl in IHstp2_2.
+    eapply IHstp2_2. reflexivity. omega.
+
+    specialize IHstp2_3 with (GH2:=GH0) (GH3:=(0, (G2, T3)) :: GH1).
+    simpl in IHstp2_3. rewrite app_length. rewrite map_length. simpl.
+    repeat rewrite splice_open_permute with (j:=0).
+    rewrite app_length in IHstp2_3. simpl in IHstp2_3.
+    eapply IHstp2_3. reflexivity. omega. omega.
+  - Case "bind".
+    eapply stp2_bind.
+
+    simpl. rewrite map_spliceat_length_inc. apply closed_splice. assumption.
+
+    simpl. rewrite map_spliceat_length_inc. apply closed_splice. assumption.
+
+    rewrite app_length. rewrite map_length. simpl.
+    repeat rewrite splice_open_permute with (j:=0).
+    specialize IHstp2_1 with (GH2:=GH0) (GH3:=(0, (G2,(open (TSelH (length GH1 + length GH0)) T2)))::GH1).
+    rewrite app_length in IHstp2_1. simpl in IHstp2_1. unfold open in IHstp2_1.
+    eapply IHstp2_1. eauto. omega.
+
+    rewrite app_length. rewrite map_length. simpl.
+    repeat rewrite splice_open_permute with (j:=0).
+    specialize IHstp2_2 with (GH2:=GH0) (GH3:=(0, (G1,(open (TSelH (length GH1 + length GH0)) T1)))::GH1).
+    rewrite app_length in IHstp2_2. simpl in IHstp2_2. unfold open in IHstp2_2.
+    eapply IHstp2_2. eauto. omega. omega.
+  - Case "bindb".
+    eapply stp2_bindb.
+
+    simpl. rewrite map_spliceat_length_inc. apply closed_splice. assumption.
+
+    simpl. rewrite map_spliceat_length_inc. apply closed_splice. assumption.
+
+    rewrite app_length. rewrite map_length. simpl.
+    repeat rewrite splice_open_permute with (j:=0).
+    specialize IHstp2_1 with (GH2:=GH0) (GH3:=(0, (G2,(open (TSelH (length GH1 + length GH0)) T2)))::GH1).
+    rewrite app_length in IHstp2_1. simpl in IHstp2_1. unfold open in IHstp2_1.
+    eapply IHstp2_1. eauto. omega.
+
+    rewrite app_length. rewrite map_length. simpl.
+    repeat rewrite splice_open_permute with (j:=0).
+    specialize IHstp2_2 with (GH2:=GH0) (GH3:=(0, (G1,(open (TSelH (length GH1 + length GH0)) T1)))::GH1).
+    rewrite app_length in IHstp2_2. simpl in IHstp2_2. unfold open in IHstp2_2.
+    eapply IHstp2_2. eauto. omega. omega.
 Qed.
 
+Lemma stp_extend : forall G1 GH T1 T2 x v1,
+                       stp G1 GH T1 T2 ->
+                       stp G1 ((x,v1)::GH) T1 T2.
+Proof.
+  intros. induction H; eauto using indexr_extend.
+  - Case "all".
+  assert (splice (length GH) T2 = T2) as A2. {
+    eapply closed_splice_idem. apply H1. omega.
+  }
+  assert (splice (length GH) T4 = T4) as A4. {
+    eapply closed_splice_idem. apply H2. omega.
+  }
+  assert (TSelH (S (length GH)) = splice (length GH) (TSelH (length GH))) as AH. {
+    simpl. case_eq (le_lt_dec (length GH) (length GH)); intros E LE.
+    simpl. rewrite NPeano.Nat.add_1_r. reflexivity.
+    clear LE. apply lt_irrefl in E. inversion E.
+  }
+  assert (closed 0 (length GH) T1).  eapply stp_closed2. eauto.
+  assert (splice (length GH) T1 = T1) as A1. {
+    eapply closed_splice_idem. eauto. omega.
+  }
+  assert (closed 0 (length GH) T3). eapply stp_closed1. eauto.
+  assert (splice (length GH) T3 = T3) as A3. {
+    eapply closed_splice_idem. eauto. omega.
+  }
+  assert (map (splicett (length GH)) [(0,T1)] ++(x,v1)::GH =((0,T1)::(x,v1)::GH)) as HGX1. {
+    simpl. rewrite A1. eauto.
+  }
+  assert (map (splicett (length GH)) [(0,T3)] ++(x,v1)::GH =((0,T3)::(x,v1)::GH)) as HGX3. {
+    simpl. rewrite A3. eauto.
+  }
+  apply stp_all with (x:=length ((x,v1) :: GH)).
+  apply IHstp1.
+  reflexivity.
+  apply closed_inc. apply H1.
+  apply closed_inc. apply H2.
+  simpl.
+  rewrite <- A2. rewrite <- A2.
+  unfold open.
+  change (TSelH (S (length GH))) with (TSelH (0 + (S (length GH)))).
+  rewrite -> splice_open_permute.
+  rewrite <- HGX1.
+  apply stp_splice.
+  rewrite A2. simpl. unfold open in H3. rewrite <- H0. apply H3.
+  omega.
+  simpl.
+  rewrite <- A2. rewrite <- A4.
+  unfold open.
+  change (TSelH (S (length GH))) with (TSelH (0 + (S (length GH)))).
+  rewrite -> splice_open_permute. rewrite -> splice_open_permute.
+  rewrite <- HGX3.
+  apply stp_splice.
+  simpl. unfold open in H4. rewrite <- H0. apply H4.
+  omega. omega.
+
+  - Case "bind".
+  assert (splice (length GH) T2 = T2) as A2. {
+    eapply closed_splice_idem. apply H1. omega.
+  }
+  assert (splice (length GH) T1 = T1) as A1. {
+    eapply closed_splice_idem. eauto. omega.
+  }
+  apply stp_bindx with (x:=length ((x,v1) :: GH)).
+  reflexivity.
+  apply closed_inc. apply H0.
+  apply closed_inc. apply H1.
+  simpl.
+  unfold open.
+  rewrite <- A2.
+  change (TSelH (S (length GH))) with (TSelH (0 + (S (length GH)))).
+  rewrite -> splice_open_permute. simpl.
+  assert (
+      stp G1
+     ((map (splicett (length GH)) [(0, (open_rec 0 (TSelH (length GH)) T2))])++(x, v1)::GH)
+     (splice (length GH) (open_rec 0 (TSelH (length GH)) T2))
+     (splice (length GH) (open_rec 0 (TSelH (length GH)) T2))
+     ->
+     stp G1
+     ((0, splice (length GH) (open_rec 0 (TSelH (length GH)) T2))
+      :: (x, v1) :: GH)
+     (splice (length GH) (open_rec 0 (TSelH (length GH)) T2))
+     (splice (length GH) (open_rec 0 (TSelH (length GH)) T2))
+    ) as HGX1. {
+    simpl. intros A. apply A.
+  }
+  apply HGX1.
+  apply stp_splice.
+  simpl. unfold open in H2. rewrite <- H. apply H2.
+  simpl. apply le_refl.
+  rewrite <- A1. rewrite <- A2.
+  unfold open. simpl.
+  change (TSelH (S (length GH))) with (TSelH (0 + (S (length GH)))).
+  rewrite -> splice_open_permute. rewrite -> splice_open_permute.
+  assert (
+     (stp G1
+     ((map (splicett (length GH)) [(0, (open_rec 0 (TSelH (length GH)) T1))])++(x, v1)::GH)
+     (splice (length GH) (open_rec 0 (TSelH (0 + length GH)) T1))
+     (splice (length GH) (open_rec 0 (TSelH (0 + length GH)) T2)))
+     ->
+     (stp G1
+     ((0, splice (length GH) (open_rec 0 (TSelH (0 + length GH)) T1))
+      :: (x, v1) :: GH)
+     (splice (length GH) (open_rec 0 (TSelH (0 + length GH)) T1))
+     (splice (length GH) (open_rec 0 (TSelH (0 + length GH)) T2)))
+    ) as HGX2. {
+    simpl. intros A. apply A.
+  }
+  apply HGX2.
+  apply stp_splice.
+  simpl. unfold open in H3. rewrite <- H. apply H3.
+  simpl. apply le_refl. simpl. apply le_refl.
+Qed.
+
+
+Lemma indexr_at_index: forall {A} x0 GH0 GH1 x (v:A),
+  beq_nat x0 (length GH1) = true ->
+  indexr x0 (GH0 ++ (x, v) :: GH1) = Some v.
+Proof.
+  intros. apply beq_nat_true in H. subst.
+  induction GH0.
+  - simpl. rewrite <- beq_nat_refl. reflexivity.
+  - destruct a. simpl.
+    rewrite app_length. simpl. rewrite <- plus_n_Sm. rewrite <- plus_Sn_m.
+    rewrite false_beq_nat. assumption. omega.
+Qed.
+
+Lemma indexr_same: forall {A} x0 (v0:A) GH0 GH1 x (v:A) (v':A),
+  beq_nat x0 (length GH1) = false ->
+  indexr x0 (GH0 ++ (x, v) :: GH1) = Some v0 ->
+  indexr x0 (GH0 ++ (x, v') :: GH1) = Some v0.
+Proof.
+  intros ? ? ? ? ? ? ? ? E H.
+  induction GH0.
+  - simpl. rewrite E. simpl in H. rewrite E in H. apply H.
+  - destruct a. simpl.
+    rewrite app_length. simpl.
+    case_eq (beq_nat x0 (length GH0 + S (length GH1))); intros E'.
+    simpl in H. rewrite app_length in H. simpl in H. rewrite E' in H.
+    rewrite H. reflexivity.
+    simpl in H. rewrite app_length in H. simpl in H. rewrite E' in H.
+    rewrite IHGH0. reflexivity. assumption.
+Qed.
+
+Inductive venv_ext : venv -> venv -> Prop :=
+| venv_ext_refl : forall G, venv_ext G G
+| venv_ext_cons : forall x T G1 G2, fresh G1 <= x -> venv_ext G1 G2 -> venv_ext ((x,T)::G1) G2.
+
+Inductive aenv_ext : aenv -> aenv -> Prop :=
+| aenv_ext_nil : aenv_ext nil nil
+| aenv_ext_cons : forall x T G' G A A', aenv_ext A' A -> venv_ext G' G -> aenv_ext ((x,(G',T))::A') ((x,(G,T))::A).
+
+Lemma aenv_ext_refl: forall GH, aenv_ext GH GH.
+Proof.
+  intros. induction GH.
+  - apply aenv_ext_nil.
+  - destruct a. destruct p. apply aenv_ext_cons.
+    assumption.
+    apply venv_ext_refl.
+Qed.
+
+Lemma index_extend_mult : forall G G' x T,
+                       index x G = Some T ->
+                       venv_ext G' G ->
+                       index x G' = Some T.
+Proof.
+  intros G G' x T H HV.
+  induction HV.
+  - assumption.
+  - apply index_extend. apply IHHV. apply H. assumption.
+Qed.
+
+Lemma aenv_ext__same_length:
+  forall GH GH',
+    aenv_ext GH' GH ->
+    length GH = length GH'.
+Proof.
+  intros. induction H.
+  - simpl. reflexivity.
+  - simpl. rewrite IHaenv_ext. reflexivity.
+Qed.
+
+Lemma indexr_at_ext :
+  forall GH GH' x T G,
+    aenv_ext GH' GH ->
+    indexr x GH = Some (G, T) ->
+    exists G', indexr x GH' = Some (G', T) /\ venv_ext G' G.
+Proof.
+  intros GH GH' x T G Hext Hindex. induction Hext.
+  - simpl in Hindex. inversion Hindex.
+  - simpl. simpl in Hindex.
+    case_eq (beq_nat x (length A)); intros E.
+    rewrite E in Hindex.  inversion Hindex. subst.
+    rewrite <- (@aenv_ext__same_length A A'). rewrite E.
+    exists G'. split. reflexivity. assumption. assumption.
+    rewrite E in Hindex.
+    rewrite <- (@aenv_ext__same_length A A'). rewrite E.
+    apply IHHext. assumption. assumption.
+Qed.
+
+
+Lemma stp2_closure_extend_rec :
+  forall G1 G2 T1 T2 GH s m n1,
+    stp2 s m G1 T1 G2 T2 GH n1 ->
+    (forall G1' G2' GH',
+       aenv_ext GH' GH ->
+       venv_ext G1' G1 ->
+       venv_ext G2' G2 ->
+       stp2 s m G1' T1 G2' T2 GH' n1).
+Proof.
+  intros G1 G2 T1 T2 GH s m n1 H.
+  induction H; intros; eauto;
+  try solve [inversion IHstp2_1; inversion IHstp2_2; eauto];
+  try solve [inversion IHstp2; eauto].
+  - Case "strong_sel1".
+    eapply stp2_strong_sel1. eapply index_extend_mult. apply H.
+    assumption. assumption. (* assumption. *)
+    apply IHstp2. assumption. apply venv_ext_refl. assumption.
+  - Case "strong_sel2".
+    eapply stp2_strong_sel2. eapply index_extend_mult. apply H.
+    assumption. assumption. (* assumption. *)
+    apply IHstp2. assumption. assumption. apply venv_ext_refl.
+  - Case "strong_selx".
+    eapply stp2_strong_selx.
+    eapply index_extend_mult. apply H. assumption.
+    eapply index_extend_mult. apply H0. assumption.
+  - Case "sel1".
+    eapply stp2_sel1. eapply index_extend_mult. apply H.
+    assumption. eassumption. assumption.
+    apply IHstp2_1. assumption. apply venv_ext_refl. assumption.
+    apply IHstp2_2. assumption. assumption. assumption.
+  - Case "selb1".
+    eapply stp2_selb1. eapply index_extend_mult. apply H.
+    assumption. eassumption. assumption.
+    apply IHstp2_1. apply aenv_ext_refl. apply venv_ext_refl. assumption.
+    apply IHstp2_2. assumption. assumption. assumption.
+  - Case "sel2".
+    eapply stp2_sel2. eapply index_extend_mult. apply H.
+    assumption. eassumption. assumption.
+    apply IHstp2_1. assumption. apply venv_ext_refl. assumption.
+    apply IHstp2_2. assumption. assumption. assumption.
+  - Case "selx".
+    eapply stp2_selx.
+    eapply index_extend_mult. apply H. assumption.
+    eapply index_extend_mult. apply H0. assumption.
+  - Case "sela1".
+    assert (exists GX', indexr x GH' = Some (GX', TX) /\ venv_ext GX' GX) as A. {
+      apply indexr_at_ext with (GH:=GH); assumption.
+    }
+    inversion A as [GX' [H' HX]].
+    apply stp2_sela1 with (GX:=GX') (TX:=TX).
+    assumption. assumption.
+    apply IHstp2_1; assumption.
+    apply IHstp2_2; assumption.
+  - Case "selab1".
+    assert (exists GX', indexr x GH' = Some (GX', TX) /\ venv_ext GX' GX) as A. {
+      apply indexr_at_ext with (GH:=GH); assumption.
+    }
+    inversion A as [GX' [H' HX]].
+    eapply stp2_selab1 with (GX:=GX') (TX:=TX).
+    assumption.
+    apply IHstp2_1; eauto. apply aenv_ext_refl.
+    assumption.
+    apply IHstp2_2; eauto.
+  - Case "sela2".
+    assert (exists GX', indexr x GH' = Some (GX', TX) /\ venv_ext GX' GX) as A. {
+      apply indexr_at_ext with (GH:=GH); assumption.
+    }
+    inversion A as [GX' [H' HX]].
+    apply stp2_sela2 with (GX:=GX') (TX:=TX).
+    assumption. assumption.
+    apply IHstp2_1; assumption.
+    apply IHstp2_2; assumption.
+  - Case "selax".
+    assert (exists GX', indexr x GH' = Some (GX', TX) /\ venv_ext GX' GX) as A. {
+      apply indexr_at_ext with (GH:=GH); assumption.
+    }
+    inversion A as [GX' [H' HX]].
+    apply stp2_selax with (GX:=GX') (TX:=TX).
+    assumption.
+  - Case "all".
+    assert (length GH = length GH') as A. {
+      apply aenv_ext__same_length. assumption.
+    }
+    apply stp2_all.
+    apply IHstp2_1; assumption.
+    subst. rewrite <- A. assumption.
+    subst. rewrite <- A. assumption.
+    subst. rewrite <- A.
+    apply IHstp2_2. apply aenv_ext_cons. assumption. assumption. assumption. assumption.
+    subst. rewrite <- A.
+    apply IHstp2_3. apply aenv_ext_cons. assumption. assumption. assumption. assumption.
+  - Case "bind".
+    assert (length GH = length GH') as A. {
+      apply aenv_ext__same_length. assumption.
+    }
+    apply stp2_bind.
+    subst. rewrite A in H. assumption.
+    subst. rewrite A in H0. assumption.
+    rewrite A in IHstp2_1. apply IHstp2_1. apply aenv_ext_cons. assumption. assumption. assumption. assumption.
+    subst.
+    rewrite A in IHstp2_2. apply IHstp2_2. apply aenv_ext_cons. assumption. assumption. assumption. assumption.
+  - Case "bindb".
+    assert (length GH = length GH') as A. {
+      apply aenv_ext__same_length. assumption.
+    }
+    apply stp2_bindb.
+    subst. rewrite A in H. assumption.
+    subst. rewrite A in H0. assumption.
+    rewrite A in IHstp2_1. apply IHstp2_1. apply aenv_ext_cons. assumption. assumption. assumption. assumption.
+    subst.
+    rewrite A in IHstp2_2. apply IHstp2_2. apply aenv_ext_cons. assumption. assumption. assumption. assumption.
+  - Case "trans".
+    eapply stp2_transf.
+    eapply IHstp2_1.
+    assumption. assumption. apply venv_ext_refl.
+    eapply IHstp2_2.
+    assumption. apply venv_ext_refl. assumption.
+Qed.
+
+
+Lemma stp2_closure_extend : forall G1 T1 G2 T2 GH GX T x v s m n1,
+                              stp2 s m G1 T1 G2 T2 ((0,(GX,T))::GH) n1 ->
+                              fresh GX <= x ->
+                              stp2 s m G1 T1 G2 T2 ((0,((x,v)::GX,T))::GH) n1.
+Proof.
+  intros. eapply stp2_closure_extend_rec. apply H.
+  apply aenv_ext_cons. apply aenv_ext_refl. apply venv_ext_cons.
+  assumption. apply venv_ext_refl. apply venv_ext_refl. apply venv_ext_refl.
+Qed.
+
+
+Lemma stp2_extend : forall x v1 G1 G2 T1 T2 H s m n1,
+                      stp2 s m G1 T1 G2 T2 H n1 ->
+                      (fresh G1 <= x ->
+                       stp2 s m ((x,v1)::G1) T1 G2 T2 H n1) /\
+                      (fresh G2 <= x ->
+                       stp2 s m G1 T1 ((x,v1)::G2) T2 H n1) /\
+                      (fresh G1 <= x -> fresh G2 <= x ->
+                       stp2 s m ((x,v1)::G1) T1 ((x,v1)::G2) T2 H n1).
+Proof.
+  intros. induction H0;
+    try solve [split; try split; repeat ev; intros; eauto using index_extend];
+    try solve [split; try split; intros; inversion IHstp2_1 as [? [? ?]]; inversion IHstp2_2 as [? [? ?]]; inversion IHstp2_3 as [? [? ?]]; constructor; eauto; apply stp2_closure_extend; eauto];
+    try solve [split; try split; intros; inversion IHstp2_1 as [? [? ?]]; inversion IHstp2_2 as [? [? ?]]; eapply stp2_bind; eauto; apply stp2_closure_extend; eauto];
+    try solve [split; try split; intros; inversion IHstp2_1 as [? [? ?]]; inversion IHstp2_2 as [? [? ?]]; eapply stp2_bindb; eauto; apply stp2_closure_extend; eauto].
+Qed.
 
 Lemma stp2_extend2 : forall x v1 G1 G2 T1 T2 H s m n1,
                        stp2 s m G1 T1 G2 T2 H n1 ->
                        fresh G2 <= x ->
                        stp2 s m G1 T1 ((x,v1)::G2) T2 H n1.
-Proof. admit. Qed.
+Proof.
+  intros. apply (proj2 (stp2_extend x v1 G1 G2 T1 T2 H s m n1 H0)). assumption.
+Qed.
 
 Lemma stp2_extend1 : forall x v1 G1 G2 T1 T2 H s m n1,
                        stp2 s m G1 T1 G2 T2 H n1 ->
                        fresh G1 <= x ->
                        stp2 s m ((x,v1)::G1) T1 G2 T2 H n1.
-Proof. admit. Qed.
-
-Lemma stp2_extendH : forall x v1 G1 G2 T1 T2 H s m n1,
-                       stp2 s m G1 T1 G2 T2 H n1 ->
-                       stp2 s m G1 T1 G2 T2 ((x,v1)::H) n1.
 Proof.
-  admit. (* (NOT) TODO (NOW): use splice *)
+  intros. apply (proj1 (stp2_extend x v1 G1 G2 T1 T2 H s m n1 H0)). assumption.
+Qed.
+
+Lemma stp2_extendH : forall x v1 G1 G2 T1 T2 GH s m n1,
+                       stp2 s m G1 T1 G2 T2 GH n1 ->
+                       stp2 s m G1 T1 G2 T2 ((x,v1)::GH) n1.
+Proof.
+  intros. induction H; eauto using indexr_extend.
+  - Case "all".
+  assert (splice (length GH) T2 = T2) as A2. {
+    eapply closed_splice_idem. apply H0. omega.
+  }
+  assert (splice (length GH) T4 = T4) as A4. {
+    eapply closed_splice_idem. apply H1. omega.
+  }
+  assert (TSelH (S (length GH)) = splice (length GH) (TSelH (length GH))) as AH. {
+    simpl. case_eq (le_lt_dec (length GH) (length GH)); intros E LE.
+    simpl. rewrite NPeano.Nat.add_1_r. reflexivity.
+    clear LE. apply lt_irrefl in E. inversion E.
+  }
+  assert (closed 0 (length GH) T1). eapply stp2_closed2. eauto.
+  assert (splice (length GH) T1 = T1) as A1. {
+    eapply closed_splice_idem. eauto. omega.
+  }
+  assert (map (spliceat (length GH)) [(0,(G1, T1))] ++(x,v1)::GH =((0, (G1, T1))::(x,v1)::GH)) as HGX1. {
+    simpl. rewrite A1. eauto.
+  }
+  assert (closed 0 (length GH) T3). eapply stp2_closed1. eauto.
+  assert (splice (length GH) T3 = T3) as A3. {
+    eapply closed_splice_idem. eauto. omega.
+  }
+  assert (map (spliceat (length GH)) [(0,(G2, T3))] ++(x,v1)::GH =((0, (G2, T3))::(x,v1)::GH)) as HGX3. {
+    simpl. rewrite A3. eauto.
+  }
+  eapply stp2_all.
+  apply IHstp2_1.
+  apply closed_inc. apply H0.
+  apply closed_inc. apply H1.
+  simpl.
+  unfold open.
+  rewrite <- A2.
+  unfold open.
+  change (TSelH (S (length GH))) with (TSelH (0 + (S (length GH)))).
+  rewrite -> splice_open_permute.
+  rewrite <- HGX1.
+  apply stp2_splice.
+  simpl. unfold open in H2. apply H2.
+  simpl. omega.
+  rewrite <- A2. rewrite <- A4.
+  unfold open. simpl.
+  change (TSelH (S (length GH))) with (TSelH (0 + (S (length GH)))).
+  rewrite -> splice_open_permute.
+  rewrite -> splice_open_permute.
+  rewrite <- HGX3.
+  apply stp2_splice.
+  simpl. unfold open in H3. apply H3.
+  omega. omega.
+
+  - Case "bind".
+  assert (splice (length GH) T2 = T2) as A2. {
+    eapply closed_splice_idem. eauto. omega.
+  }
+  assert (splice (length GH) T1 = T1) as A1. {
+    eapply closed_splice_idem. eauto. omega.
+  }
+  eapply stp2_bind.
+  apply closed_inc. eauto.
+  apply closed_inc. eauto.
+  simpl.
+  unfold open.
+  rewrite <- A2.
+  change (TSelH (S (length GH))) with (TSelH (0 + (S (length GH)))).
+  rewrite -> splice_open_permute. simpl.
+  assert (
+   stp2 1 false G2 (splice (length GH) (open_rec 0 (TSelH (length GH)) T2))
+     G2 (splice (length GH) (open_rec 0 (TSelH (length GH)) T2))
+     ((map (spliceat (length GH)) [(0, (G2, open_rec 0 (TSelH (length GH)) T2))])++((x, v1)::GH))
+      n2
+   ->
+   stp2 1 false G2 (splice (length GH) (open_rec 0 (TSelH (length GH)) T2))
+     G2 (splice (length GH) (open_rec 0 (TSelH (length GH)) T2))
+     ((0, (G2, splice (length GH) (open_rec 0 (TSelH (length GH)) T2)))
+      :: (x, v1) :: GH) n2
+    ) as HGX1. {
+    simpl. intros A. apply A.
+  }
+  apply HGX1.
+  apply stp2_splice.
+  simpl. unfold open in H1. apply H1.
+  simpl. apply le_refl.
+  rewrite <- A1. rewrite <- A2.
+  unfold open. simpl.
+  change (TSelH (S (length GH))) with (TSelH (0 + (S (length GH)))).
+  rewrite -> splice_open_permute. rewrite -> splice_open_permute.
+  assert (
+   stp2 1 false G1
+     (splice (length GH) (open_rec 0 (TSelH (0 + length GH)) T1)) G2
+     (splice (length GH) (open_rec 0 (TSelH (0 + length GH)) T2))
+     ((map (spliceat (length GH)) [(0, (G1, (open_rec 0 (TSelH (0 + length GH)) T1)))])++((x, v1) :: GH)) n1
+      ->
+   stp2 1 false G1
+     (splice (length GH) (open_rec 0 (TSelH (0 + length GH)) T1)) G2
+     (splice (length GH) (open_rec 0 (TSelH (0 + length GH)) T2))
+     ((0, (G1, splice (length GH) (open_rec 0 (TSelH (0 + length GH)) T1)))
+        :: (x, v1) :: GH) n1
+   ) as HGX2. {
+    simpl. intros A. apply A.
+  }
+  apply HGX2.
+  apply stp2_splice.
+  simpl. unfold open in H2. apply H2.
+  simpl. apply le_refl. simpl. apply le_refl.
+
+  - Case "bindb".
+  assert (splice (length GH) T2 = T2) as A2. {
+    eapply closed_splice_idem. eauto. omega.
+  }
+  assert (splice (length GH) T1 = T1) as A1. {
+    eapply closed_splice_idem. eauto. omega.
+  }
+  eapply stp2_bindb.
+  apply closed_inc. eauto.
+  apply closed_inc. eauto.
+  simpl.
+  unfold open.
+  rewrite <- A2.
+  change (TSelH (S (length GH))) with (TSelH (0 + (S (length GH)))).
+  rewrite -> splice_open_permute. simpl.
+  assert (
+   stp2 (S m) false G2 (splice (length GH) (open_rec 0 (TSelH (length GH)) T2))
+     G2 (splice (length GH) (open_rec 0 (TSelH (length GH)) T2))
+     ((map (spliceat (length GH)) [(0, (G2, open_rec 0 (TSelH (length GH)) T2))])++((x, v1)::GH))
+      n2
+   ->
+   stp2 (S m) false G2 (splice (length GH) (open_rec 0 (TSelH (length GH)) T2))
+     G2 (splice (length GH) (open_rec 0 (TSelH (length GH)) T2))
+     ((0, (G2, splice (length GH) (open_rec 0 (TSelH (length GH)) T2)))
+      :: (x, v1) :: GH) n2
+    ) as HGX1. {
+    simpl. intros A. apply A.
+  }
+  apply HGX1.
+  apply stp2_splice.
+  simpl. unfold open in H1. apply H1.
+  simpl. apply le_refl.
+  rewrite <- A1. rewrite <- A2.
+  unfold open. simpl.
+  change (TSelH (S (length GH))) with (TSelH (0 + (S (length GH)))).
+  rewrite -> splice_open_permute. rewrite -> splice_open_permute.
+  assert (
+   stp2 (S m) false G1
+     (splice (length GH) (open_rec 0 (TSelH (0 + length GH)) T1)) G2
+     (splice (length GH) (open_rec 0 (TSelH (0 + length GH)) T2))
+     ((map (spliceat (length GH)) [(0, (G1, (open_rec 0 (TSelH (0 + length GH)) T1)))])++((x, v1) :: GH)) n1
+      ->
+   stp2 (S m) false G1
+     (splice (length GH) (open_rec 0 (TSelH (0 + length GH)) T1)) G2
+     (splice (length GH) (open_rec 0 (TSelH (0 + length GH)) T2))
+     ((0, (G1, splice (length GH) (open_rec 0 (TSelH (0 + length GH)) T1)))
+        :: (x, v1) :: GH) n1
+   ) as HGX2. {
+    simpl. intros A. apply A.
+  }
+  apply HGX2.
+  apply stp2_splice.
+  simpl. unfold open in H2. apply H2.
+  simpl. apply le_refl. simpl. apply le_refl.
 Qed.
 
 Lemma stp2_extendH_mult : forall G1 G2 T1 T2 H H2 s m n1,
@@ -1203,78 +2292,134 @@ Lemma stp2_extendH_mult0 : forall G1 G2 T1 T2 H2 s m n1,
                        stp2 s m G1 T1 G2 T2 H2 n1.
 Proof. intros. eapply stp2_extendH_mult with (H2:=H2) in H; eauto. rewrite app_nil_r in H. eauto. Qed.
 
+Lemma stp2_reg  : forall G1 G2 T1 T2 GH s m n1,
+                    stp2 s m G1 T1 G2 T2 GH n1 ->
+                    (exists n0, stp2 s true G1 T1 G1 T1 GH n0) /\
+                    (exists n0, stp2 s true G2 T2 G2 T2 GH n0).
+Proof.
+  intros. induction H;
+    try solve [repeat ev; split; eexists; eauto].
+  - Case "and11".
+    repeat ev; split; eexists.
+    eapply stp2_and2.
+    eapply stp2_wrapf. eapply stp2_and11; eassumption.
+    eapply stp2_wrapf. eapply stp2_and12; eassumption.
+    eassumption.
+  - Case "and12".
+    repeat ev; split; eexists.
+    eapply stp2_and2.
+    eapply stp2_wrapf. eapply stp2_and11; eassumption.
+    eapply stp2_wrapf. eapply stp2_and12; eassumption.
+    eassumption.
+  - Case "and2".
+    repeat ev; split; eexists.
+    eassumption.
+    eapply stp2_and2.
+    eapply stp2_wrapf. eapply stp2_and11; eassumption.
+    eapply stp2_wrapf. eapply stp2_and12; eassumption.
+  Grab Existential Variables.
+  apply 0. apply 0. apply 0. apply 0. apply 0. apply 0. apply 0. apply 0. apply 0. apply 0.
+  apply 0. apply 0. apply 0. apply 0. apply 0. apply 0. apply 0. apply 0. apply 0. apply 0.
+  apply 0. apply 0.
+Qed.
 
-Lemma stp2_reg2 : forall G1 G2 T1 T2 H s m n1,
-                       stp2 s m G1 T1 G2 T2 H n1 ->
-                       stp2 s m G2 T2 G2 T2 H n1.
-Proof. admit. Qed.
+Lemma stp2_reg2 : forall G1 G2 T1 T2 GH s m n1,
+                       stp2 s m G1 T1 G2 T2 GH n1 ->
+                       (exists n0, stp2 s true G2 T2 G2 T2 GH n0).
+Proof.
+  intros. apply (proj2 (stp2_reg G1 G2 T1 T2 GH s m n1 H)).
+Qed.
 
-Lemma stp2_reg1 : forall G1 G2 T1 T2 H s m n1,
-                       stp2 s m G1 T1 G2 T2 H n1 ->
-                       stp2 s m G1 T1 G1 T1 H n1.
-Proof. admit. Qed.
+Lemma stp2_reg1 : forall G1 G2 T1 T2 GH s m n1,
+                       stp2 s m G1 T1 G2 T2 GH n1 ->
+                       (exists n0, stp2 s true G1 T1 G1 T1 GH n0).
+Proof.
+  intros. apply (proj1 (stp2_reg G1 G2 T1 T2 GH s m n1 H)).
+Qed.
 
-
-Lemma stp2_closed2 : forall G1 G2 T1 T2 H s m n1,
-                       stp2 s m G1 T1 G2 T2 H n1 ->
-                       closed 0 (length H) T2.
-Proof. admit. Qed.
-
-Lemma stp2_closed1 : forall G1 G2 T1 T2 H s m n1,
-                       stp2 s m G1 T1 G2 T2 H n1 ->
-                       closed 0 (length H) T1.
-Proof. admit. Qed.
-
-(* stpd2 variants below *)
+Lemma stp_reg  : forall G GH T1 T2,
+                    stp G GH T1 T2 ->
+                    stp G GH T1 T1 /\ stp G GH T2 T2.
+Proof.
+  intros. induction H;
+    try solve [repeat ev; split; eauto].
+Qed.
 
 Lemma stpd2_extend2 : forall x v1 G1 G2 T1 T2 H m,
                        stpd2 m G1 T1 G2 T2 H ->
                        fresh G2 <= x ->
                        stpd2 m G1 T1 ((x,v1)::G2) T2 H.
-Proof. admit. Qed.
+Proof.
+  intros. inversion H0 as [n1 Hsub]. exists n1.
+  apply stp2_extend2; assumption.
+Qed.
 
 Lemma stpd2_extend1 : forall x v1 G1 G2 T1 T2 H m,
                        stpd2 m G1 T1 G2 T2 H ->
                        fresh G1 <= x ->
                        stpd2 m ((x,v1)::G1) T1 G2 T2 H.
-Proof. admit. Qed.
+Proof.
+  intros. inversion H0 as [n1 Hsub]. exists n1.
+  apply stp2_extend1; assumption.
+Qed.
 
 Lemma stpd2_extendH : forall x v1 G1 G2 T1 T2 H m,
                        stpd2 m G1 T1 G2 T2 H ->
                        stpd2 m G1 T1 G2 T2 ((x,v1)::H).
-Proof. admit. Qed.
+Proof.
+  intros. inversion H0 as [n1 Hsub]. exists n1.
+  apply stp2_extendH; assumption.
+Qed.
 
 Lemma stpd2_extendH_mult : forall G1 G2 T1 T2 H H2 m,
                        stpd2 m G1 T1 G2 T2 H->
                        stpd2 m G1 T1 G2 T2 (H2++H).
-Proof. admit. Qed.
+Proof.
+  intros. inversion H0 as [n1 Hsub]. exists n1.
+  apply stp2_extendH_mult; assumption.
+Qed.
 
 Lemma stpd2_extendH_mult0 : forall G1 G2 T1 T2 H2 m,
                        stpd2 m G1 T1 G2 T2 [] ->
                        stpd2 m G1 T1 G2 T2 H2.
-Proof. admit. Qed.
+Proof.
+  intros. inversion H as [n1 Hsub]. exists n1.
+  apply stp2_extendH_mult0; assumption.
+Qed.
 
 
 Lemma stpd2_reg2 : forall G1 G2 T1 T2 H m,
                        stpd2 m G1 T1 G2 T2 H ->
-                       stpd2 m G2 T2 G2 T2 H.
-Proof. admit. Qed.
+                       stpd2 true G2 T2 G2 T2 H.
+Proof.
+  intros. inversion H0 as [n1 Hsub].
+  eapply stp2_reg2; eassumption.
+Qed.
 
 Lemma stpd2_reg1 : forall G1 G2 T1 T2 H m,
                        stpd2 m G1 T1 G2 T2 H ->
-                       stpd2 m G1 T1 G1 T1 H.
-Proof. admit. Qed.
+                       stpd2 true G1 T1 G1 T1 H.
+Proof.
+  intros. inversion H0 as [n1 Hsub].
+  eapply stp2_reg1; eassumption.
+Qed.
 
 
 Lemma stpd2_closed2 : forall G1 G2 T1 T2 H m,
                        stpd2 m G1 T1 G2 T2 H ->
                        closed 0 (length H) T2.
-Proof. admit. Qed.
+Proof.
+  intros. inversion H0 as [n1 Hsub].
+  eapply stp2_closed2; eassumption.
+Qed.
 
 Lemma stpd2_closed1 : forall G1 G2 T1 T2 H m,
                        stpd2 m G1 T1 G2 T2 H ->
                        closed 0 (length H) T1.
-Proof. admit. Qed.
+Proof.
+  intros. inversion H0 as [n1 Hsub].
+  eapply stp2_closed1; eassumption.
+Qed.
 
 
 (* sstpd2 variants below *)
@@ -1283,51 +2428,75 @@ Lemma sstpd2_extend2 : forall x v1 G1 G2 T1 T2 H m,
                        sstpd2 m G1 T1 G2 T2 H ->
                        fresh G2 <= x ->
                        sstpd2 m G1 T1 ((x,v1)::G2) T2 H.
-Proof. admit. Qed.
+Proof.
+  intros. inversion H0 as [n1 Hsub]. exists n1.
+  apply stp2_extend2; assumption.
+Qed.
 
 Lemma sstpd2_extend1 : forall x v1 G1 G2 T1 T2 H m,
                        sstpd2 m G1 T1 G2 T2 H ->
                        fresh G1 <= x ->
                        sstpd2 m ((x,v1)::G1) T1 G2 T2 H.
-Proof. admit. Qed.
+Proof.
+  intros. inversion H0 as [n1 Hsub]. exists n1.
+  apply stp2_extend1; assumption.
+Qed.
 
 Lemma sstpd2_extendH : forall x v1 G1 G2 T1 T2 H m,
                        sstpd2 m G1 T1 G2 T2 H ->
                        sstpd2 m G1 T1 G2 T2 ((x,v1)::H).
-Proof. admit. Qed.
+Proof.
+  intros. inversion H0 as [n1 Hsub]. exists n1.
+  apply stp2_extendH; assumption.
+Qed.
 
 Lemma sstpd2_extendH_mult : forall G1 G2 T1 T2 H H2 m,
                        sstpd2 m G1 T1 G2 T2 H->
                        sstpd2 m G1 T1 G2 T2 (H2++H).
-Proof. admit. Qed.
+Proof.
+  intros. inversion H0 as [n1 Hsub]. exists n1.
+  apply stp2_extendH_mult; assumption.
+Qed.
 
 Lemma sstpd2_extendH_mult0 : forall G1 G2 T1 T2 H2 m,
                        sstpd2 m G1 T1 G2 T2 [] ->
                        sstpd2 m G1 T1 G2 T2 H2.
-Proof. admit. Qed.
+Proof.
+  intros. inversion H as [n1 Hsub]. exists n1.
+  apply stp2_extendH_mult0; assumption.
+Qed.
 
 Lemma sstpd2_reg2 : forall G1 G2 T1 T2 H m,
                        sstpd2 m G1 T1 G2 T2 H ->
-                       sstpd2 m G2 T2 G2 T2 H.
-Proof. admit. Qed.
+                       sstpd2 true G2 T2 G2 T2 H.
+Proof.
+  intros. inversion H0 as [n1 Hsub].
+  eapply stp2_reg2; eassumption.
+Qed.
 
 Lemma sstpd2_reg1 : forall G1 G2 T1 T2 H m,
                        sstpd2 m G1 T1 G2 T2 H ->
-                       sstpd2 m G1 T1 G1 T1 H.
-Proof. admit. Qed.
+                       sstpd2 true G1 T1 G1 T1 H.
+Proof.
+  intros. inversion H0 as [n1 Hsub].
+  eapply stp2_reg1; eassumption.
+Qed.
 
 Lemma sstpd2_closed2 : forall G1 G2 T1 T2 H m,
                        sstpd2 m G1 T1 G2 T2 H ->
                        closed 0 (length H) T2.
-Proof. admit. Qed.
+Proof.
+  intros. inversion H0 as [n1 Hsub].
+  eapply stp2_closed2; eassumption.
+Qed.
 
 Lemma sstpd2_closed1 : forall G1 G2 T1 T2 H m,
                        sstpd2 m G1 T1 G2 T2 H ->
                        closed 0 (length H) T1.
-Proof. admit. Qed.
-
-
-
+Proof.
+  intros. inversion H0 as [n1 Hsub].
+  eapply stp2_closed1; eassumption.
+Qed.
 
 Lemma valtp_extend : forall vs v x v1 T,
                        val_type vs v T ->
@@ -1352,7 +2521,7 @@ Proof. intros. induction H.
        elim (le_xx (fresh vs) n QF). intros ? EX.
 
        case_eq (beq_nat i n); intros E2.
-       * SSCase "hit".         
+       * SSCase "hit".
          assert (index i ((n, v) :: vs) = Some v). eauto. unfold index. rewrite EX. rewrite E2. eauto.
          assert (t = TF).
          unfold index in H0. rewrite E1 in H0. rewrite E2 in H0. inversion H0. eauto.
@@ -1390,7 +2559,7 @@ Proof. intros. induction H0.
        eapply v_tya. (* aenv is not constrained -- bit of a cheat?*)
 Qed.
 
-  
+
 Inductive res_type: venv -> option vl -> ty -> Prop :=
 | not_stuck: forall venv v T,
       val_type venv v T ->
@@ -1411,47 +2580,276 @@ Proof.
   - Case "transf". eapply stpd2_transf. eauto. eapply IHn. eauto. omega. eauto.
 Qed.
 
+Lemma sstpd2_trans_axiom_aux: forall n, forall G1 G2 G3 T1 T2 T3 H n1,
+  stp2 0 false G1 T1 G2 T2 H n1 -> n1 < n ->
+  sstpd2 false G2 T2 G3 T3 H ->
+  sstpd2 false G1 T1 G3 T3 H.
+Proof.
+  intros n. induction n; intros; try omega; repeat eu; subst; inversion H0.
+  - Case "wrapf". eapply sstpd2_transf. eexists. eauto. eexists. eauto.
+  - Case "transf". eapply sstpd2_transf. eexists. eauto. eapply IHn. eauto. omega. eexists. eauto.
+Qed.
+
+Lemma atpd2_trans_axiom_aux: forall n, forall G1 G2 G3 T1 T2 T3 H n1,
+  stp2 1 false G1 T1 G2 T2 H n1 -> n1 < n ->
+  atpd2 false G2 T2 G3 T3 H ->
+  atpd2 false G1 T1 G3 T3 H.
+Proof.
+  intros n. induction n; intros; try omega; repeat eu; subst; inversion H0.
+  - Case "wrapf". eapply atpd2_transf. eexists. eauto. eexists. eauto.
+  - Case "transf". eapply atpd2_transf. eexists. eauto. eapply IHn. eauto. omega. eexists. eauto.
+Qed.
+
 Lemma stpd2_trans: forall G1 G2 G3 T1 T2 T3 H,
   stpd2 false G1 T1 G2 T2 H ->
   stpd2 false G2 T2 G3 T3 H ->
   stpd2 false G1 T1 G3 T3 H.
 Proof. intros. repeat eu. eapply stpd2_trans_aux; eauto. Qed.
 
+Lemma sstpd2_trans_axiom: forall G1 G2 G3 T1 T2 T3 H,
+  sstpd2 false G1 T1 G2 T2 H ->
+  sstpd2 false G2 T2 G3 T3 H ->
+  sstpd2 false G1 T1 G3 T3 H.
+Proof. intros. repeat eu.
+       eapply sstpd2_trans_axiom_aux; eauto.
+       eexists. eauto.
+Qed.
+
 Lemma atpd2_trans_axiom: forall G1 G2 G3 T1 T2 T3 H,
   atpd2 false G1 T1 G2 T2 H ->
   atpd2 false G2 T2 G3 T3 H ->
   atpd2 false G1 T1 G3 T3 H.
-Proof. admit. Qed.
-
-
-(*
-Lemma sstpd2_trans_axiom: forall n, forall G1 G2 G3 T1 T2 T3 H n1,
-  stp2 true false G1 T1 G2 T2 H n1 -> n1 < n ->
-  sstpd2 false G2 T2 G3 T3 H ->
-  sstpd2 false G1 T1 G3 T3 H.
 Proof.
-  intros n. induction n; intros; try omega; repeat eu; subst; inversion H0.
-  - Case "wrapf". eexists. eapply stp2_transf; eauto.
-  - Case "transf". admit. (*eexists. eapply stp2_transf. eauto. ep. eapply IHn. eauto. omega. eauto. eauto. *)
+  intros. repeat eu. eapply atpd2_trans_axiom_aux; eauto. eexists. eauto.
 Qed.
-*)
+
+Lemma stp2_narrow_aux: forall n, forall m G1 T1 G2 T2 GH n0,
+  stp2 MAX m G1 T1 G2 T2 GH n0 ->
+  n0 <= n ->
+  forall x GH1 GH0 GH' GX1 TX1 GX2 TX2,
+    GH=GH1++[(x,(GX2,TX2))]++GH0 ->
+    GH'=GH1++[(x,(GX1,TX1))]++GH0 ->
+    stpd2 false GX1 TX1 GX2 TX2 [] ->
+    stpd2 m G1 T1 G2 T2 GH'.
+Proof.
+  intros n.
+  induction n.
+  - Case "z". intros. inversion H0. subst. inversion H; eauto.
+  - Case "s n". intros m G1 T1 G2 T2 GH n0 H NE. inversion H; subst;
+      intros x0 GH1 GH0 GH' GX1 TX1 GX2 TX2 EGH EGH' HX; eauto.
+    + SCase "top". eapply stpd2_top. eapply IHn; try eassumption. omega.
+    + SCase "bot". eapply stpd2_bot. eapply IHn; try eassumption. omega.
+    + SCase "fun". eapply stpd2_fun.
+      eapply IHn; try eassumption. omega.
+      eapply IHn; try eassumption. omega.
+    + SCase "mem". eapply stpd2_mem.
+      eapply IHn; try eassumption. omega.
+      eapply IHn; try eassumption. omega.
+    + SCase "sel1". eapply stpd2_sel1; try eassumption.
+      eapply IHn; try eassumption. omega.
+      eapply IHn; try eassumption. omega.
+    + SCase "selb1". eapply stpd2_selb1; try eassumption.
+      eexists; eassumption.
+      eapply IHn; try eassumption. omega.
+    + SCase "sel2". eapply stpd2_sel2; try eassumption.
+      eapply IHn; try eassumption. omega.
+      eapply IHn; try eassumption. omega.
+    + SCase "selx". eapply stpd2_selx; try eassumption.
+    + SCase "sela1".
+      case_eq (beq_nat x (length GH0)); intros E.
+      * assert (indexr x ([(x0, (GX2, TX2))]++GH0) = Some (GX2, TX2)) as A2. {
+          simpl. rewrite E. reflexivity.
+        }
+        assert (indexr x GH = Some (GX2, TX2)) as A2'. {
+          rewrite EGH. eapply indexr_extend_mult. apply A2.
+        }
+        rewrite A2' in H1. inversion H1. subst.
+        inversion HX as [nx HX'].
+        eapply stpd2_sela1.
+        eapply indexr_extend_mult. simpl. rewrite E. reflexivity.
+        apply beq_nat_true in E. rewrite E. eapply stp2_closed1. eapply stp2_extendH_mult0. eassumption.
+        eapply stpd2_trans.
+        eexists. eapply stp2_extendH_mult0. eassumption.
+        eapply IHn; try eassumption. omega.
+        reflexivity. reflexivity.
+        eapply IHn; try eassumption. omega.
+        reflexivity. reflexivity.
+      * assert (indexr x GH' = Some (GX, TX)) as A. {
+          subst.
+          eapply indexr_same. apply E. eassumption.
+        }
+        eapply stpd2_sela1. eapply A. assumption.
+        eapply IHn; try eassumption. omega.
+        eapply IHn; try eassumption. omega.
+    + SCase "selab1".
+      case_eq (beq_nat x (length GH0)); intros E.
+      * assert (indexr x ([(x0, (GX2, TX2))]++GH0) = Some (GX2, TX2)) as A2. {
+          simpl. rewrite E. reflexivity.
+        }
+        assert (indexr x GH = Some (GX2, TX2)) as A2'. {
+          rewrite EGH. eapply indexr_extend_mult. apply A2.
+        }
+        assert (Some (GX2,TX2) = Some (GX, TX)) as E2. {
+          rewrite A2' in H1. apply H1.
+        }
+        inversion E2. subst.
+        eapply stpd2_selab1.
+        eapply indexr_extend_mult. simpl. rewrite E. reflexivity.
+        eapply stpd2_trans. eassumption. eexists. eassumption.
+        eapply IHn; try eassumption. omega.
+        reflexivity. reflexivity.
+      * assert (indexr x GH' = Some (GX, TX)) as A. {
+          subst.
+          eapply indexr_same. apply E. eassumption.
+        }
+        eapply stpd2_selab1. eapply A.
+        eexists. eassumption.
+        eapply IHn; try eassumption. omega.
+    + SCase "sela2".
+      case_eq (beq_nat x (length GH0)); intros E.
+      * assert (indexr x ([(x0, (GX2, TX2))]++GH0) = Some (GX2, TX2)) as A2. {
+          simpl. rewrite E. reflexivity.
+        }
+        assert (indexr x GH = Some (GX2, TX2)) as A2'. {
+          rewrite EGH. eapply indexr_extend_mult. apply A2.
+        }
+        rewrite A2' in H1. inversion H1. subst.
+        inversion HX as [nx HX'].
+        eapply stpd2_sela2.
+        eapply indexr_extend_mult. simpl. rewrite E. reflexivity.
+        apply beq_nat_true in E. rewrite E. eapply stp2_closed1. eapply stp2_extendH_mult0. eassumption.
+        eapply stpd2_trans.
+        eexists. eapply stp2_extendH_mult0. eassumption.
+        eapply IHn; try eassumption. omega.
+        reflexivity. reflexivity.
+        eapply IHn; try eassumption. omega.
+        reflexivity. reflexivity.
+      * assert (indexr x GH' = Some (GX, TX)) as A. {
+          subst.
+          eapply indexr_same. apply E. eassumption.
+        }
+        eapply stpd2_sela2. eapply A. assumption.
+        eapply IHn; try eassumption. omega.
+        eapply IHn; try eassumption. omega.
+    + SCase "selax".
+      case_eq (beq_nat x (length GH0)); intros E.
+      * assert (indexr x ([(x0, (GX2, TX2))]++GH0) = Some (GX2, TX2)) as A2. {
+          simpl. rewrite E. reflexivity.
+        }
+        assert (indexr x GH = Some (GX2, TX2)) as A2'. {
+          rewrite EGH. eapply indexr_extend_mult. apply A2.
+        }
+        rewrite A2' in H1. inversion H1. subst.
+        inversion HX as [nx HX'].
+        eapply stpd2_selax.
+        eapply indexr_extend_mult. simpl. rewrite E. reflexivity.
+      * assert (indexr x GH' = Some (GX, TX)) as A. {
+          subst.
+          eapply indexr_same. apply E. eassumption.
+        }
+        eapply stpd2_selax. eapply A.
+    + SCase "all".
+      assert (length GH = length GH') as A. {
+        subst. clear.
+        induction GH1.
+        - simpl. reflexivity.
+        - simpl. simpl in IHGH1. rewrite IHGH1. reflexivity.
+      }
+      eapply stpd2_all.
+      eapply IHn; try eassumption. omega.
+      rewrite <- A. assumption. rewrite <- A. assumption.
+      rewrite <- A. subst.
+      eapply IHn with (GH1:=(0, (G1, T0)) :: GH1); try eassumption. omega.
+      simpl. reflexivity. simpl. reflexivity.
+      rewrite <- A. subst.
+      eapply IHn with (GH1:=(0, (G2, T4)) :: GH1); try eassumption. omega.
+      simpl. reflexivity. simpl. reflexivity.
+    + SCase "bind".
+      assert (length GH = length GH') as A. {
+        subst. clear.
+        induction GH1.
+        - simpl. reflexivity.
+        - simpl. simpl in IHGH1. rewrite IHGH1. reflexivity.
+      }
+      eapply stpd2_bind.
+      assert (closed 1 (length GH) T0 -> closed 1 (length GH') T0) as C0. {
+        rewrite A. intros P. apply P.
+      }
+      apply C0; assumption.
+      assert (closed 1 (length GH) T3 -> closed 1 (length GH') T3) as C3. {
+        rewrite A. intros P. apply P.
+      }
+      apply C3; assumption.
+      assert (
+          stpd2 false G2 (open (TSelH (length GH)) T3) G2
+                (open (TSelH (length GH)) T3)
+                ((0, (G2, open (TSelH (length GH)) T3)) :: GH')
+                ->
+          stpd2 false G2 (open (TSelH (length GH')) T3) G2
+                (open (TSelH (length GH')) T3)
+                ((0, (G2, open (TSelH (length GH')) T3)) :: GH')) as CS1. {
+        rewrite A. intros P. apply P.
+      }
+      apply CS1. eapply IHn. eassumption. omega.
+      instantiate (5:=(0, (G2, open (TSelH (length GH)) T3)) :: GH1).
+      subst. simpl. reflexivity. subst. simpl. reflexivity.
+      assumption.
+      assert (
+          stpd2 false G1 (open (TSelH (length GH)) T0) G2
+                (open (TSelH (length GH)) T3)
+                ((0, (G1, open (TSelH (length GH)) T0)) :: GH')
+                ->
+          stpd2 false G1 (open (TSelH (length GH')) T0) G2
+                (open (TSelH (length GH')) T3)
+                ((0, (G1, open (TSelH (length GH')) T0)) :: GH')
+        ) as CS2. {
+        rewrite A. intros P. apply P.
+      }
+      apply CS2. eapply IHn. eassumption. omega.
+      instantiate (5:=(0, (G1, open (TSelH (length GH)) T0)) :: GH1).
+      subst. simpl. reflexivity. subst. simpl. reflexivity.
+      assumption.
+    + SCase "and11".
+      eapply stpd2_and11.
+      eapply IHn; try eassumption. omega.
+      eapply IHn; try eassumption. omega.
+    + SCase "and12".
+      eapply stpd2_and12.
+      eapply IHn; try eassumption. omega.
+      eapply IHn; try eassumption. omega.
+    + SCase "and2".
+      eapply stpd2_and2.
+      eapply IHn; try eassumption. omega.
+      eapply IHn; try eassumption. omega.
+    + SCase "wrapf".
+      eapply stpd2_wrapf.
+      eapply IHn; try eassumption. omega.
+    + SCase "transf".
+      eapply stpd2_transf.
+      eapply IHn; try eassumption. omega.
+      eapply IHn; try eassumption. omega.
+Grab Existential Variables.
+apply 0. apply 0. apply 0.
+Qed.
+
+Lemma stpd2_narrow: forall x G1 G2 G3 G4 T1 T2 T3 T4,
+  stpd2 false G1 T1 G2 T2 [] -> (* careful about H! *)
+  stpd2 false G3 T3 G4 T4 ((x,(G2,T2))::[]) ->
+  stpd2 false G3 T3 G4 T4 ((x,(G1,T1))::[]).
+Proof.
+  intros. inversion H0 as [n H'].
+  eapply (stp2_narrow_aux n) with (GH1:=[]) (GH0:=[]). eapply H'. omega.
+  simpl. reflexivity. reflexivity.
+  assumption.
+Qed.
 
 
-
-(* used in trans -- need to generalize interface for induction *)
-
-Lemma stpd2_narrow: forall x G1 G2 G3 G4 T1 T2 T3 T4 H,
-  stpd2 false G1 T1 G2 T2 ((x,(G1,T1))::H) -> (* careful about H! *)
-  stpd2 false G3 T3 G4 T4 ((x,(G2,T2))::H) ->
-  stpd2 false G3 T3 G4 T4 ((x,(G1,T1))::H).
-Proof. admit. Qed.
 
 Lemma atpd2_narrow: forall x G1 G2 G3 G4 T1 T2 T3 T4 H,
   atpd2 false G1 T1 G2 T2 ((x,(G1,T1))::H) -> (* careful about H! *)
   atpd2 false G3 T3 G4 T4 ((x,(G2,T2))::H) ->
   atpd2 false G3 T3 G4 T4 ((x,(G1,T1))::H).
 Proof. admit. Qed.
-
 
 
 Lemma sstpd2_trans_aux: forall n, forall m G1 G2 G3 T1 T2 T3 n1,
@@ -1464,107 +2862,139 @@ Proof.
   - Case "topx". subst. inversion H1.
     + SCase "topx". eexists. eauto.
     + SCase "top". eexists. eauto.
-    + SCase "sel2". eexists. eapply stp2_strong_sel2. eauto. eauto. eapply stp2_transf. eauto. eauto.
-    + SCase "and2". subst. eexists. eauto.
+    + SCase "sel2". eexists. eapply stp2_strong_sel2; eauto.
+    + SCase "and2". subst. eexists. eapply stp2_and2; eauto.
   - Case "botx". subst. inversion H1.
     + SCase "botx". eexists. eauto.
     + SCase "top". eexists. eauto.
     + SCase "?". eexists. eauto.
-    + SCase "sel2". eexists. eapply stp2_strong_sel2. eauto. eauto. eapply stp2_transf. eauto. eauto.
-    + SCase "and2". subst. eexists. eauto.
+    + SCase "sel2". eexists. eapply stp2_strong_sel2; eauto.
+    + SCase "and2". subst. eexists. eapply stp2_and2; eauto.
   - Case "top". subst. inversion H1.
     + SCase "topx". eexists. eauto.
     + SCase "top". eexists. eauto.
-    + SCase "sel2". eexists. eapply stp2_strong_sel2. eauto. eauto. eapply stp2_transf. eauto. eauto.
-    + SCase "and2". subst. eexists. eapply stp2_and2. ep. eapply stpd2_trans. eexists. eapply stp2_wrapf. eauto. eauto. eauto. eauto.
-  - Case "bot". admit. 
+    + SCase "sel2". eexists. eapply stp2_strong_sel2; eauto.
+    + SCase "and2". subst. eexists. eapply stp2_and2; eauto.
+  - Case "bot". subst.
+    apply stp2_reg2 in H1. inversion H1 as [n1' H1'].
+    exists (S n1'). apply stp2_bot. apply H1'.
   - Case "bool". subst. inversion H1.
     + SCase "top". eexists. eauto.
     + SCase "bool". eexists. eauto.
-    + SCase "sel2". eexists. eapply stp2_strong_sel2. eauto. eauto. eapply stp2_transf. eauto. eauto.
-    + SCase "and2". subst. eexists. eauto.
+    + SCase "sel2". eexists. eapply stp2_strong_sel2; eauto.
+    + SCase "and2". subst. eexists. eapply stp2_and2; eauto.
   - Case "fun". subst. inversion H1.
-    + SCase "top". eexists. eapply stp2_top. subst. eapply stp2_wrapf. eapply stp2_fun. eapply stp2_reg2. eauto. eapply stp2_reg1. eauto.
-    + SCase "fun".
-      admit.
-      (* eexists. eapply stp2_fun. ep. eapply stpd2_trans. eauto. eauto. destruct EEX. eauto. *)
-    + SCase "sel2". eexists. eapply stp2_strong_sel2. eauto. eauto. eapply stp2_transf. eauto. eauto.
-    + SCase "and2". subst. eexists. eapply stp2_and2. ep. eapply stpd2_trans. eexists. eapply stp2_wrapf. eauto. eauto. eauto. eauto.
+    + SCase "top".
+      assert (stpd2 false G1 T0 G1 T0 []) as A0 by solve [eapply stpd2_wrapf; eapply stp2_reg2; eassumption].
+      inversion A0 as [na0 HA0].
+      assert (stpd2 false G1 T4 G1 T4 []) as A4 by solve [eapply stpd2_wrapf; eapply stp2_reg1; eassumption].
+      inversion A4 as [na4 HA4].
+      eexists. eapply stp2_top. subst. eapply stp2_fun.
+      eassumption. eassumption.
+    + SCase "fun". subst.
+      assert (stpd2 false G3 T7 G1 T0 []) as A by solve [eapply stpd2_trans; eauto].
+      inversion A as [na A'].
+      assert (stpd2 false G1 T4 G3 T8 []) as B by solve [eapply stpd2_trans; eauto].
+      inversion B as [nb B'].
+      eexists. eapply stp2_fun. apply A'. apply B'.
+    + SCase "sel2". eexists. eapply stp2_strong_sel2; eauto.
+    + SCase "and2". subst. eexists. eapply stp2_and2; eauto.
   - Case "mem". subst. inversion H1.
-    + SCase "top". admit.
-    + SCase "mem". admit.
-    + SCase "sel2". eexists. eapply stp2_strong_sel2. eauto. eauto. eapply stp2_transf. eauto. eauto.
-    + SCase "and2". admit.
+    + SCase "top".
+      apply stp2_reg1 in H. inversion H. eexists. eapply stp2_top. eassumption.
+    + SCase "mem". subst.
+      assert (sstpd2 false G3 T7 G1 T0 []) as A. {
+        eapply sstpd2_trans_axiom; eexists; eauto.
+      }
+      inversion A as [na A'].
+      assert (sstpd2 true G1 T4 G3 T8 []) as B. {
+        eapply IHn. eassumption. omega. eexists. eassumption.
+      }
+      inversion B as [nb B'].
+      eexists. eapply stp2_mem. apply A'. apply B'.
+    + SCase "sel2". eexists. eapply stp2_strong_sel2; eauto.
+    + SCase "and2". subst. eexists. eapply stp2_and2; eauto.
   - Case "ssel1".
-    assert (sstpd2 true GX TX G3 T3 []). eapply IHn. eauto. omega. eexists. eapply H1. 
-    eu. eexists. eapply stp2_strong_sel1. eauto. eauto. eauto.
+    assert (sstpd2 true GX TX G3 T3 []). eapply IHn. eauto. omega. eexists. eapply H1.
+    eu. eexists. eapply stp2_strong_sel1; eauto.
   - Case "ssel2". subst. inversion H1.
-    + SCase "top". admit.
+    + SCase "top". subst.
+      apply stp2_reg1 in H4. inversion H4.
+      eexists. eapply stp2_top. eassumption.
     + SCase "ssel1".  (* interesting one *)
       subst. rewrite H6 in H2. inversion H2. subst.
       eapply IHn. eapply H4. omega. eexists. eauto.
     + SCase "ssel2".
-      eexists. eapply stp2_strong_sel2. eauto. eauto. eapply stp2_transf. eauto. eauto.
+      eexists. eapply stp2_strong_sel2; eauto.
     + SCase "sselx".
       subst. rewrite H2 in H6. inversion H6. subst.
-      eexists. eapply stp2_strong_sel2. eauto. eauto. eauto.
-    + SCase "and2". admit.
+      eexists. eapply stp2_strong_sel2; eauto.
+    + SCase "and2". subst. eexists. eapply stp2_and2; eauto.
   - Case "sselx". subst. inversion H1.
-    + SCase "top". admit.
+    + SCase "top". subst.
+      apply stp2_reg1 in H. inversion H.
+      eexists. eapply stp2_top. eassumption.
     + SCase "ssel1".
       subst. rewrite H5 in H3. inversion H3. subst.
-      eexists. eapply stp2_strong_sel1. eauto. eauto. eauto.
-    + SCase "ssel2". eexists. eapply stp2_strong_sel2. eauto. eauto. eapply stp2_transf. eauto. eauto.
+      eexists. eapply stp2_strong_sel1; eauto.
+    + SCase "ssel2". eexists. eapply stp2_strong_sel2; eauto.
     + SCase "sselx".
       subst. rewrite H5 in H3. inversion H3. subst.
       eexists. eapply stp2_strong_selx. eauto. eauto.
-    + SCase "and2". admit.
+    + SCase "and2". subst. eexists. eapply stp2_and2; eauto.
   - Case "all". subst. inversion H1.
-    + SCase "top". admit.
+    + SCase "top".
+      apply stp2_reg1 in H. inversion H.
+      eexists. eapply stp2_top. eassumption.
     + SCase "ssel2".
-      eexists. eapply stp2_strong_sel2. eauto. eauto. eapply stp2_transf. eauto. eauto.
+      eexists. eapply stp2_strong_sel2; eauto.
     + SCase "all".
       subst.
       assert (stpd2 false G3 T7 G1 T0 []). eapply stpd2_trans. eauto. eauto.
       assert (stpd2 false G1 (open (TSelH (length ([]:aenv))) T4)
                           G3 (open (TSelH (length ([]:aenv))) T8)
                           [(0, (G3, T7))]).
-        eapply stpd2_trans. eapply stpd2_narrow. eapply stpd2_extendH. eexists. eapply H8. eauto. eauto. 
-      repeat eu. eexists. eapply stp2_all. eauto. eauto. eauto. eauto.
-    + SCase "and2". admit.
-  - Case "bind". subst. inversion H1.
-    + SCase "top". admit.
+        eapply stpd2_trans. eapply stpd2_narrow. eexists. eapply H9. eauto. eauto.
+        repeat eu. eexists. eapply stp2_all. eauto. eauto. eauto. eauto. eapply H8.
+    + SCase "and2". subst. eexists. eapply stp2_and2; eauto.
+  - Case "bind". subst. inversion H1; subst.
+    + SCase "top".
+      apply stp2_reg1 in H. inversion H.
+      eexists. eapply stp2_top. eassumption.
     + SCase "ssel2".
-      eexists. eapply stp2_strong_sel2. eauto. eauto. eapply stp2_transf. eauto. eauto.
+      eexists. eapply stp2_strong_sel2; eauto.
     + SCase "bind".
       subst.
-      assert (atpd2 false G1 (open (TSelH (length ([]:aenv))) T0)
-                          G3 (open (TSelH (length ([]:aenv))) T2)
-                          [(0, (G1, open (TSelH (length ([]:aenv))) T0))]).
-        eapply atpd2_trans_axiom. unfold atpd2. eauto. eapply atpd2_narrow. eexists. eapply H4. unfold atpd2. eauto. 
-      unfold atpd2 in H5. destruct H5. repeat eu. eexists. eapply stp2_bind. eauto. eauto. eauto. 
-    + SCase "and2". admit.
-  - Case "and11". subst.
-    assert (sstpd2 true G1 T0 G3 T3 []) as Hn. {
-      eapply IHn. eauto. omega. eexists. eauto.
-    }
-    inversion Hn.
-    eexists. eapply stp2_and11. eassumption. eassumption.
-  - Case "and12". subst.
-    assert (sstpd2 true G1 T4 G3 T3 []) as Hn. {
-      eapply IHn. eauto. omega. eexists. eauto.
-    }
-    inversion Hn.
-    eexists. eapply stp2_and12. eassumption. eassumption.
-  - Case "and2". admit.
-    (*subst. inversion H1.
-    + SCase "top". subst. eexists. eapply stp2_top. eapply stp2_reg1. eauto.
-    + SCase "ssel2".
-      eexists. eapply stp2_strong_sel2. eauto. eauto. eapply stp2_transf. eauto. eauto.*)
+      assert (atpd2 false G1 (open (TSelH 0) T0) G3 (open (TSelH 0) T2)
+                    [(0, (G1, open (TSelH 0) T0))]) as A. {
+        simpl in H5. simpl in H10.
+        eapply atpd2_trans_axiom.
+        eexists; eauto.
+        change ([(0, (G1, open (TSelH 0) T0))]) with ((0, (G1, open (TSelH 0) T0))::[]).
+        eapply atpd2_narrow. eexists. eassumption. eexists. eassumption.
+      }
+      inversion A.
+      eexists. eapply stp2_bind; try eassumption.
+    + SCase "and2". subst. eexists. eapply stp2_and2; eauto.
+  - Case "and11". subst. inversion H1; subst;
+                         try solve [eapply IHn in H2;
+                         [inversion H2; eexists; eapply stp2_and11; eassumption
+                         | omega | eexists; eassumption]].
+  - Case "and12". subst. inversion H1; subst;
+                         try solve [eapply IHn in H2;
+                         [inversion H2; eexists; eapply stp2_and12; eassumption
+                         | omega | eexists; eassumption]].
+  - Case "and2". subst. inversion H1; subst.
+    + SCase "top". eapply stp2_reg1 in H. inversion H. eexists. eapply stp2_top; eassumption.
+    + SCase "sel2". eexists. eapply stp2_strong_sel2; eauto.
+    + SCase "and11". subst. eapply IHn. apply H2. omega. eexists. eassumption.
+    + SCase "and12". subst. eapply IHn. apply H3. omega. eexists. eassumption.
+    + SCase "and2". subst. eexists. eapply stp2_and2; eauto.
   - Case "wrapf". subst. eapply IHn. eapply H2. omega. eexists. eauto.
   - Case "transf". subst. eapply IHn. eapply H2. omega. eapply IHn. eapply H3. omega. eexists. eauto.
+
 Grab Existential Variables.
-apply 0. apply 0. apply 0. apply 0. apply 0. apply 0. apply 0. apply 0. apply 0. apply 0. apply 0. apply 0. apply 0.
+apply 0. apply 0. apply 0. apply 0. apply 0. apply 0. apply 0.
 Qed.
 
 Lemma sstpd2_trans: forall G1 G2 G3 T1 T2 T3,
@@ -1607,11 +3037,6 @@ Proof.
   intros. inversion H. eapply not_stuck. eapply valtp_widen; eauto.
 Qed.
 
-Ltac ev := repeat match goal with
-                    | H: exists _, _ |- _ => destruct H
-                    | H: _ /\  _ |- _ => destruct H
-           end.
-
 Lemma invert_typ: forall venv vx T1 T2,
   val_type venv vx (TMem T1 T2) ->
   exists GX TX,
@@ -1621,10 +3046,15 @@ Lemma invert_typ: forall venv vx T1 T2,
 Proof.
   intros. inversion H; ev; try solve by inversion. inversion H1.
   subst.
-  assert (sstpd2 false venv0 T1 venv1 T0 []) as E1. admit. (* FIXME: def of stp_mem *)
-  assert (sstpd2 true venv1 T0 venv0 T2 []) as E2. admit.
-  repeat eu. repeat eexists; eauto. 
+  assert (sstpd2 false venv0 T1 venv1 T0 []) as E1. {
+    eexists. eassumption.
+  }
+  assert (sstpd2 true venv1 T0 venv0 T2 []) as E2. {
+    eexists. eassumption.
+  }
+  repeat eu. repeat eexists; eauto.
 Qed.
+
 
 
 Lemma stpd2_to_sstpd2_aux1: forall n, forall G1 G2 T1 T2 m n1,
@@ -1633,15 +3063,18 @@ Lemma stpd2_to_sstpd2_aux1: forall n, forall G1 G2 T1 T2 m n1,
 Proof.
   intros n. induction n; intros; try omega.
   inversion H.
-  - Case "botx". eexists. eauto.
   - Case "topx". eexists. eauto.
-  - Case "bot". eexists. eauto.
-  - Case "top". eexists. eauto.
+  - Case "botx". eexists. eauto.
+  - Case "top". subst.
+    eapply IHn in H1. inversion H1. eexists. eauto. omega.
+  - Case "bot". subst.
+    eapply IHn in H1. inversion H1. eexists. eauto. omega.
   - Case "bool". eexists. eauto.
   - Case "fun". eexists. eapply stp2_fun. eauto. eauto.
   - Case "mem".
+    eapply IHn in H2. eapply sstpd2_untrans in H2. eu.
     eapply IHn in H3. eapply sstpd2_untrans in H3. eu.
-    eexists. eapply stp2_mem. eauto. eauto. omega.
+    eexists. eapply stp2_mem. eauto. eauto. omega. omega.
   - Case "sel1".
     eapply IHn in H5. eapply sstpd2_untrans in H5. eapply valtp_widen with (2:=H5) in H3.
     eapply invert_typ in H3. ev. repeat eu. subst.
@@ -1653,16 +3086,19 @@ Proof.
     assert (closed 0 (length ([]:aenv)) x1). eapply stp2_closed2; eauto.
     eexists. eapply stp2_strong_sel2. eauto. eauto. eauto. omega.
   - Case "selx".
-    eexists. eapply stp2_strong_selx. eauto. eauto. 
+    eexists. eapply stp2_strong_selx. eauto. eauto.
   - Case "sela1". inversion H2.
-  - Case "selab1". inversion H2. 
-  - Case "sela2". inversion H2. 
+  - Case "selab1". inversion H2.
+  - Case "sela2". inversion H2.
   - Case "selax". inversion H2.
-  - Case "all". eexists. eapply stp2_all. eauto. eauto. eauto. eauto.
-  - Case "bind". eexists. eapply stp2_bind. eauto. eauto. eauto.
-  - Case "and11". admit.
-  - Case "and12". admit.
-  - Case "and2". admit.
+  - Case "all". eexists. eapply stp2_all. eauto. eauto. eauto. eauto. eauto.
+  - Case "bind". eexists. eapply stp2_bind. eauto. eauto. eauto. eauto.
+  - Case "and11". subst. eapply IHn in H1. inversion H1. eapply IHn in H2. inversion H2.
+    eexists. eapply stp2_and11; eauto. omega. omega.
+  - Case "and12". subst. eapply IHn in H1. inversion H1. eapply IHn in H2. inversion H2.
+    eexists. eapply stp2_and12; eauto. omega. omega.
+  - Case "and2". subst. eapply IHn in H1. inversion H1. eapply IHn in H2. inversion H2.
+    eexists. eapply stp2_and2; eauto. omega. omega.
   - Case "wrapf". eapply IHn in H1. eu. eexists. eapply stp2_wrapf. eauto. omega.
   - Case "transf". eapply IHn in H1. eapply IHn in H2. eu. eu. eexists.
     eapply stp2_transf. eauto. eauto. omega. omega.
@@ -1676,24 +3112,30 @@ Lemma stpd2_to_sstpd2_aux2: forall n, forall G1 G2 GH T1 T2 m n1,
 Proof.
   intros n. induction n; intros; try omega.
   inversion H.
-  - Case "botx". eexists. eauto.
   - Case "topx". eexists. eauto.
-  - Case "bot". eexists. eauto.
-  - Case "top". eexists. eauto.
+  - Case "botx". eexists. eauto.
+  - Case "top". subst.
+    eapply IHn in H1. inversion H1. eexists. eauto. omega.
+  - Case "bot". subst.
+    eapply IHn in H1. inversion H1. eexists. eauto. omega.
   - Case "bool". eexists. eauto.
   - Case "fun". eexists. eapply stp2_fun. eauto. eauto.
   - Case "mem".
     eapply IHn in H2. ev. eapply IHn in H3. ev.
     eexists. eapply stp2_mem2; eauto. omega. omega.
-  - Case "sel1".
-    eapply IHn in H5. ev.
-    eexists. eapply stp2_sel1; eauto. omega.
-  - Case "sel1b".
-    eapply IHn in H5. ev. eapply stpd2_to_sstpd2_aux1 in H5. eapply sstpd2_untrans in H5. eapply valtp_widen with (2:=H5) in H3.
+  - Case "sel1". subst.
+    eapply IHn in H5. eapply IHn in H6. ev. ev.
+    eexists. eapply stp2_sel1; eauto. omega. omega.
+  - Case "selb1". subst.
+    eapply IHn in H5. eapply IHn in H6. ev. ev. eapply stpd2_to_sstpd2_aux1 in H5. eapply sstpd2_untrans in H5. eapply valtp_widen with (2:=H5) in H3.
     (* now invert base on TBind knowledge -- TODO: helper lemma*)
-    inversion H3; ev. inversion H14. inversion H13. inversion H17. inversion H16. (* 1 case left *)
-    subst. inversion H16. subst.
-    assert (stp2 1 false venv0 (open (TSel x1) T3)
+    inversion H3; ev. subst.
+    inversion H7. subst.
+    inversion H6. subst.
+    inversion H10.
+    inversion H9. (* 1 case left *)
+    subst. inversion H9. subst.
+    assert (stp2 1 false venv0 (open (TSel x2) T2)
                  G2 (open (TSel x) (TMem TBot T0)) [] n1) as ST.
     admit. (* get this from substitute *)
 
@@ -1707,7 +3149,7 @@ Proof.
          So we cannot change the bind's body elsewhere, before inverting here.
 
          (UPDATE: actually that's what we're doing now. We get away with it
-         because GH = [], which means that we may not be able to  unfold nontrivial 
+         because GH = [], which means that we may not be able to  unfold nontrivial
          binds for selections on hypothetical vars)
 
        - Doing induction on ST here would be difficult, because the size is wrong.
@@ -1720,33 +3162,38 @@ Proof.
          That makes it seem unlikely that we'd be able to use IHn on the result.
 
          We know the size of what we're putting into ST. But we have the same problem
-         as previously in narrowing: we do not know how many times the added term 
+         as previously in narrowing: we do not know how many times the added term
          is used, so we cannot bound the result size.
     *)
-    
-    assert (closed 0 (length (nil:aenv)) (open (TSel x1) T3)). eapply stp2_closed1. eauto.
-    eexists. eapply stp2_sel1. eauto. eapply H14. eauto.
-    eapply stp2_extendH_mult0. eauto. eauto. omega.
-  - Case "sel2".
-    eapply IHn in H5. ev.
-    eexists. eapply stp2_sel2; eauto. omega.
-  - Case "selx".
-    eexists. eapply stp2_selx. eauto. eauto. 
-  - Case "sela1". eapply IHn in H3. ev. eexists. eapply stp2_sela1; eauto. omega.
+    assert (closed 0 (length (nil:aenv)) (open (TSel x2) T2)) as C. eapply stp2_closed1. eauto. simpl in C.
+    eexists. eapply stp2_sel1. eauto. eapply H7. eauto.
+    eapply stp2_extendH_mult0. eauto. eauto. eauto. omega. omega.
+  - Case "sel2". subst.
+    eapply IHn in H5. eapply IHn in H6. ev. ev.
+    eexists. eapply stp2_sel2; eauto. omega. omega.
+  - Case "selx". subst.
+    eexists. eapply stp2_selx. eauto. eauto.
+  - Case "sela1". subst. eapply IHn in H4. eapply IHn in H5. ev. ev.
+    eexists. eapply stp2_sela1; eauto. omega. omega.
   - Case "selab1".
     (* THIS ONE WILL NOT WORK AT LEVEL 2 (no way to remove *)
     (* so we use it at level 1, and translate during subst *)
     (* restriction GH = [] ensures that level 2 terms are already removed *)
-    eapply IHn in H3. ev. eexists. eapply stp2_selab1; eauto. omega.
-  - Case "sela2". eapply IHn in H3. ev. eexists. eapply stp2_sela2; eauto. omega.
-  - Case "selhx". eexists. eapply stp2_selax. eauto. eauto.
-  - Case "all". eexists. eapply stp2_all. eauto. eauto. eauto. eauto.
+    eapply IHn in H3. eapply IHn in H5. ev. ev.
+    eexists. eapply stp2_selab1; eauto. omega. omega.
+  - Case "sela2". eapply IHn in H4. eapply IHn in H5. ev. ev.
+    eexists. eapply stp2_sela2; eauto. omega. omega.
+  - Case "selhx". eexists. eapply stp2_selax. eauto.
+  - Case "all". eexists. eapply stp2_all. eauto. eauto. eauto. eapply H4. eapply H5.
   - Case "bind".
-    eapply IHn in H4. ev. 
-    eexists. eapply stp2_bindb. eauto. eauto. eauto. omega.
-  - Case "and11". admit.
-  - Case "and12". admit.
-  - Case "and2". admit.
+    eapply IHn in H4. eapply IHn in H5. ev. ev.
+    eexists. eapply stp2_bindb. eauto. eauto. eauto. eauto. omega. omega.
+  - Case "and11". subst. eapply IHn in H1. inversion H1. eapply IHn in H2. inversion H2.
+    eexists. eapply stp2_and11; eauto. omega. omega.
+  - Case "and12". subst. eapply IHn in H1. inversion H1. eapply IHn in H2. inversion H2.
+    eexists. eapply stp2_and12; eauto. omega. omega.
+  - Case "and2". subst. eapply IHn in H1. inversion H1. eapply IHn in H2. inversion H2.
+    eexists. eapply stp2_and2; eauto. omega. omega.
   - Case "wrapf". eapply IHn in H1. ev. eexists. eapply stp2_wrapf. eauto. omega.
   - Case "transf". eapply IHn in H1. eapply IHn in H2. ev. ev. eexists.
     eapply stp2_transf. eauto. eauto. omega. omega.
@@ -1782,12 +3229,9 @@ Proof.
   admit.
 Qed.
 
-
-
-
 Lemma index_miss {X}: forall x x1 (B:X) A G,
   index x ((x1,B)::G) = A ->
-  fresh G <= x1 ->                      
+  fresh G <= x1 ->
   x <> x1 ->
   index x G = A.
 Proof.
@@ -1801,7 +3245,7 @@ Qed.
 
 Lemma index_hit {X}: forall x x1 (B:X) A G,
   index x ((x1,B)::G) = Some A ->
-  fresh G <= x1 ->                      
+  fresh G <= x1 ->
   x = x1 ->
   B = A.
 Proof.
@@ -1814,7 +3258,7 @@ Proof.
 Qed.
 
 Lemma index_hit2 {X}: forall x x1 (B:X) A G,
-  fresh G <= x1 ->                      
+  fresh G <= x1 ->
   x = x1 ->
   B = A ->
   index x ((x1,B)::G) = Some A.
@@ -1856,7 +3300,7 @@ Lemma indexr_hit0: forall GH (GX0:venv) (TX0:ty),
       Some (GX0, TX0).
 Proof.
   intros GH. induction GH.
-  - intros. simpl. eauto. 
+  - intros. simpl. eauto.
   - intros. simpl. destruct a. simpl. rewrite app_length. simpl.
     assert (length GH + 1 = S (length GH)). omega. rewrite H.
     eauto.
@@ -1879,33 +3323,10 @@ Proof.
   try solve [compute; compute in IHclosed_rec1; compute in IHclosed_rec2; rewrite <-IHclosed_rec1; rewrite <-IHclosed_rec2; auto].
 
   Case "TSelB".
-    unfold open_rec. assert (k <> i). omega. 
+    unfold open_rec. assert (k <> i). omega.
     apply beq_nat_false_iff in H0.
     rewrite H0. auto.
 Qed.
-
-
-
-Lemma closed_upgrade: forall i j l T,
- closed_rec i l T ->
- j >= i ->
- closed_rec j l T.
-Proof.
- intros. generalize dependent j. induction H; intros; eauto.
- Case "TAll". econstructor. eapply IHclosed_rec1. omega. eapply IHclosed_rec2. omega.
- Case "TBind". econstructor. eapply IHclosed_rec. omega. 
- Case "TSelB". econstructor. omega.
-Qed.
-
-Lemma closed_upgrade_free: forall i l k T,
- closed_rec i l T ->
- k >= l ->
- closed_rec i k T.
-Proof.
- intros. generalize dependent k. induction H; intros; eauto.
- Case "TSelH". econstructor. omega. 
-Qed.
-
 
 
 Lemma open_subst_commute: forall T2 TX (n:nat) x j,
@@ -1916,7 +3337,7 @@ Proof.
   intros T2 TX n. induction T2; intros; eauto.
   -  simpl. rewrite IHT2_1. rewrite IHT2_2. eauto. eauto. eauto.
   -  simpl. rewrite IHT2_1. rewrite IHT2_2. eauto. eauto. eauto.
-  -  simpl. case_eq (beq_nat i 0); intros E. symmetry. eapply closed_no_open. eauto. simpl. eauto.  
+  -  simpl. case_eq (beq_nat i 0); intros E. symmetry. eapply closed_no_open. eauto. simpl. eauto.
   - simpl. case_eq (beq_nat j i); intros E. simpl.
     assert (x+1<>0). omega. eapply beq_nat_false_iff in H0.
     assert (x=x+1-1). unfold id. omega.
@@ -1924,7 +3345,7 @@ Proof.
     simpl. eauto.
   -  simpl. rewrite IHT2_1. rewrite IHT2_2. eauto. eapply closed_upgrade. eauto. eauto. eauto.
   -  simpl. rewrite IHT2. eauto. eapply closed_upgrade. eauto. eauto.
-  - simpl. rewrite IHT2_1. rewrite IHT2_2. eauto. assumption. assumption.
+  - simpl. rewrite IHT2_1. rewrite IHT2_2. eauto. eauto. eauto.
 Qed.
 
 
@@ -1940,27 +3361,12 @@ Proof.
     try rewrite (IHT j TX); eauto;
     try rewrite (IHT1 j TX); eauto;
     try rewrite (IHT2 j TX); eauto.
-            
+
   eapply closed_upgrade. eauto. eauto.
   eapply closed_upgrade. eauto. eauto.
   subst. omega.
-  eapply closed_upgrade. eauto. eauto.
+  subst. eapply closed_upgrade. eassumption. omega.
 Qed.
-
-Lemma closed_open: forall j n TX T, closed (j+1) n T -> closed j n TX -> closed j n (open_rec j TX T).
-Proof.
-  intros. generalize dependent j. induction T; intros; inversion H; unfold closed; try econstructor; try eapply IHT1; eauto; try eapply IHT2; eauto; try eapply IHT; eauto. eapply closed_upgrade. eauto. eauto.
-
-  - Case "TSelB". simpl.
-    case_eq (beq_nat j i); intros E. eauto. 
-    
-    econstructor. eapply beq_nat_false_iff in E. omega.
-
-  - eauto.
-  - eapply closed_upgrade; eauto.
-  - eapply closed_upgrade; eauto.
-Qed.
-
 
 Lemma closed_subst: forall j n TX T, closed j (n+1) T -> closed 0 n TX -> closed j (n) (subst TX T).
 Proof.
@@ -1971,7 +3377,7 @@ Proof.
     econstructor. assert (i > 0). eapply beq_nat_false_iff in E. omega. omega.
 Qed.
 
-    
+
 Lemma subst_open_commute_m: forall j n m TX T2, closed (j+1) (n+1) T2 -> closed 0 m TX ->
     subst TX (open_rec j (TSelH (n+1)) T2) = open_rec j (TSelH n) (subst TX T2).
 Proof.
@@ -2019,7 +3425,7 @@ Proof.
   simpl. eauto.
 Qed.
 
-    
+
 Lemma nosubst_intro: forall j T, closed j 0 T -> nosubst T.
 Proof.
   intros. generalize dependent j. induction T; intros; inversion H; simpl; eauto.
@@ -2070,86 +3476,25 @@ Proof.
       left. split. eapply beq_nat_true_iff. eauto. eauto.
     + rewrite E in H. inversion H.
   -  destruct a. unfold id in H. remember ((length (GH0 ++ [(0, TX)]))) as L.
-     case_eq (beq_nat x L); intros E. 
+     case_eq (beq_nat x L); intros E.
      + assert (x = L). eapply beq_nat_true_iff. eauto.
        eapply indexr_hit in H.
        right. split. rewrite app_length in HeqL. simpl in HeqL. omega.
        assert ((x - 1) = (length (map (substt TX) GH0))).
        rewrite map_length. rewrite app_length in HeqL. simpl in HeqL. unfold id. omega.
        simpl.
-       eapply beq_nat_true_iff in H1. unfold id in H1. unfold id. rewrite H1. subst. eauto. eauto. subst. eauto. 
+       eapply beq_nat_true_iff in H1. unfold id in H1. unfold id. rewrite H1. subst. eauto. eauto. subst. eauto.
      + assert (x <> L). eapply beq_nat_false_iff. eauto.
        eapply indexr_miss in H. eapply IHGH0 in H.
        inversion H. left. eapply H1.
        right. inversion H1. split. eauto.
        simpl.
        assert ((x - 1) <> (length (map (substt TX) GH0))).
-       rewrite app_length in HeqL. simpl in HeqL. rewrite map_length.       
+       rewrite app_length in HeqL. simpl in HeqL. rewrite map_length.
        unfold not. intros. subst L. unfold id in H0. unfold id in H2. unfold not in H0. eapply H0. unfold id in H4. rewrite <-H4. omega.
        eapply beq_nat_false_iff in H4. unfold id in H4. unfold id. rewrite H4.
        eauto. subst. eauto.
 Qed.
-
-(*
-Lemma stp_substitute: forall T1 T2 GX GH,
-   stp GX GH T1 T2 ->
-   forall GH0 TX0,
-     GH = (GH0 ++ [(0,TMem TBot TX0)]) ->
-     closed 0 0 TX0 ->
-     stp GX (map (substt TX0) GH0) TX0 TX0 ->
-     stp GX (map (substt TX0) GH0)
-         (subst TX0 T1)
-         (subst TX0 T2).
-Proof.
-  intros T1 T2 GX GH H.
-  induction H.
-  - Case "top". eauto.
-  - Case "bot". eauto.
-  - Case "bool". eauto.
-  - Case "fun". intros. simpl. eapply stp_fun. eauto. eauto.
-  - Case "mem". intros. simpl. eapply stp_mem. eauto. eauto.
-  - Case "sel1". admit.
-  - Case "sel2". admit.
-  - Case "selx". admit.
-  - Case "sela1". intros GH0 TX1 ? ? ?. simpl.
-    subst GH. specialize (indexr_subst _ x (TMem TBot TX1) _ H). intros. 
-    destruct H1; destruct H1.
-    + subst. simpl.
-      specialize (IHstp GH0 TX1). 
-      assert (subst TX1 TX1 = TX1). eapply closed_no_subst; eauto.
-      (* rewrite H1 in IHstp. *)
-      eapply IHstp. eauto. eauto. eauto.
-    + subst. simpl.
-      assert (beq_nat x 0 = false). eapply beq_nat_false_iff; omega. rewrite H5. simpl.
-      eapply stp_sela1. eapply H4. eapply IHstp. eauto. eauto. eauto.
-  - Case "sela2". admit. 
-  - Case "selax". intros GH0 TX ? ? ?. simpl.
-    subst GH. specialize (indexr_subst _ x TX TL TU H). intros.
-    destruct H0; destruct H0.
-    + subst. simpl. eauto.
-    + subst. simpl. assert (beq_nat x 0 = false). eapply beq_nat_false_iff. omega. rewrite H4. eapply stp_selax. eauto.
-  - Case "all".
-    intros GH0 TX ? ? ?.
-    simpl. eapply stp_all.
-    + eapply IHstp1; eauto.
-    + rewrite map_length. eauto.
-    + rewrite map_length. eapply closed_subst. subst GH.
-      rewrite app_length in H1. simpl in H1. eauto.
-      eapply closed_upgrade_free; eauto. omega.
-    + rewrite map_length. eapply closed_subst. subst GH.
-      rewrite app_length in H2. simpl in H2. eauto.
-      eapply closed_upgrade_free; eauto. omega.
-    + specialize IHstp2 with (GH0:=(0, T3)::GH0) (TX:=TX).
-      subst GH. simpl in IHstp2.
-      unfold open. unfold open in IHstp2.
-      subst x.
-      rewrite open_subst_commute with (n:=0).
-      rewrite open_subst_commute with (n:=0).
-      rewrite app_length in IHstp2. simpl in IHstp2.
-      eapply IHstp2; eauto. eapply stp_extend; eauto.
-      eauto. eauto.
-Qed.
-*)
 
 (*
 when and how we can replace with multiple environments:
@@ -2197,6 +3542,21 @@ Definition compat2 (GX:venv) (TX: ty) (V: option vl) (p1:id*(venv*ty)) (p2:id*(v
   end.
 
 
+Lemma closed_compat: forall GX TX V GXX TXX TXX' j k,
+  compat GX TX V GXX TXX TXX' ->
+  closed 0 k TX ->
+  closed j (k+1) TXX ->
+  closed j k TXX'.
+Proof.
+  intros. inversion H;[|destruct H2;[|destruct H2]].
+  - destruct H2. destruct H2. destruct H2. destruct H2. destruct H3.
+    destruct H3. destruct H3. destruct H4. rewrite H4.
+    eapply closed_subst. eauto. eauto.
+  - destruct H2. rewrite H3.
+    eapply closed_upgrade. eapply closed_upgrade_free. eauto. omega. omega.
+  - rewrite H3.
+    eapply closed_subst. eauto. eauto.
+Qed.
 
 Lemma indexr_compat_miss0: forall GH GH' GX TX V (GXX:venv) (TXX:ty) n,
       Forall2 (compat2 GX TX V) GH GH' ->
@@ -2228,7 +3588,7 @@ Qed.
 Lemma compat_top: forall GX TX V G1 T1',
   compat GX TX V G1 TTop T1' -> closed 0 0 TX -> T1' = TTop.
 Proof.
-  intros ? ? ? ? ? CC CLX. repeat destruct CC as [|CC]; ev; eauto. 
+  intros ? ? ? ? ? CC CLX. repeat destruct CC as [|CC]; ev; eauto.
 Qed.
 
 Lemma compat_bot: forall GX TX V G1 T1',
@@ -2246,7 +3606,7 @@ Qed.
 
 Lemma compat_mem: forall GX TX V G1 T1 T2 T1',
     compat GX TX V G1 (TMem T1 T2) T1' ->
-    closed 0 0 TX -> 
+    closed 0 0 TX ->
     exists TA TB, T1' = TMem TA TB /\
                   compat GX TX V G1 T1 TA /\
                   compat GX TX V G1 T2 TB.
@@ -2264,7 +3624,7 @@ Lemma compat_mem_fwd2: forall GX TX V G1 T2 T2',
 Proof.
   intros. repeat destruct H as [|H].
   - ev. repeat eexists; eauto. + left. repeat eexists; eauto. rewrite H3. eauto.
-  - ev. repeat eexists; eauto. + right. left. subst. eauto. 
+  - ev. repeat eexists; eauto. + right. left. subst. eauto.
   - ev. repeat eexists; eauto. + right. right. subst. simpl. eauto.
 Qed.
 
@@ -2274,7 +3634,7 @@ Lemma compat_mem_fwd1: forall GX TX V G1 T2 T2',
 Proof.
   intros. repeat destruct H as [|H].
   - ev. repeat eexists; eauto. + left. repeat eexists; eauto. rewrite H3. eauto.
-  - ev. repeat eexists; eauto. + right. left. subst. eauto. 
+  - ev. repeat eexists; eauto. + right. left. subst. eauto.
   - ev. repeat eexists; eauto. + right. right. subst. simpl. eauto.
 Qed.
 
@@ -2284,15 +3644,28 @@ Lemma compat_mem_fwdx: forall GX TX V G1 T2 T2',
 Proof.
   intros. repeat destruct H as [|H].
   - ev. repeat eexists; eauto. + left. repeat eexists; eauto. rewrite H3. eauto.
-  - ev. repeat eexists; eauto. + right. left. subst. eauto. 
+  - ev. repeat eexists; eauto. + right. left. subst. eauto.
   - ev. repeat eexists; eauto. + right. right. subst. simpl. eauto.
 Qed.
 
 
 Lemma compat_fun: forall GX TX V G1 T1 T2 T1',
     compat GX TX V G1 (TFun T1 T2) T1' ->
-    closed_rec 0 0 TX -> 
+    closed_rec 0 0 TX ->
     exists TA TB, T1' = TFun TA TB /\
+                  compat GX TX V G1 T1 TA /\
+                  compat GX TX V G1 T2 TB.
+Proof.
+  intros ? ? ? ? ? ? ? CC CLX. repeat destruct CC as [|CC].
+  - ev. repeat eexists; eauto. + left. repeat eexists; eauto. + left. repeat eexists; eauto.
+  - ev. repeat eexists; eauto. + right. left. inversion H. eauto. + right. left. inversion H. eauto.
+  - ev. repeat eexists; eauto. + right. right. inversion H. eauto. + right. right. inversion H. eauto.
+Qed.
+
+Lemma compat_and: forall GX TX V G1 T1 T2 T1',
+    compat GX TX V G1 (TAnd T1 T2) T1' ->
+    closed_rec 0 0 TX ->
+    exists TA TB, T1' = TAnd TA TB /\
                   compat GX TX V G1 T1 TA /\
                   compat GX TX V G1 T2 TB.
 Proof.
@@ -2332,7 +3705,7 @@ Lemma compat_selh: forall GX TX V G1 T1' GH0 GH0' (GXX:venv) (TXX:ty) x,
       compat GX TX V GXX TXX TXX'
 .
 Proof.
-  intros ? ? ? ? ? ? ? ? ? ? CC CL IX FA. 
+  intros ? ? ? ? ? ? ? ? ? ? CC CL IX FA.
   unfold id in x.
   case_eq (beq_nat x 0); intros E.
   - left. assert (x = 0). eapply beq_nat_true_iff. eauto. subst x. rewrite indexr_hit0 in IX. inversion IX. eauto.
@@ -2341,7 +3714,7 @@ Proof.
     eapply (indexr_compat_miss0 GH0 GH0' _ _ _ _ _ _ FA) in IX.
     repeat destruct CC as [|CC].
     + ev. simpl in H7. rewrite E in H7. rewrite <-Heqy in H7. eexists. eauto.
-    + ev. inversion H1. omega. 
+    + ev. inversion H1. omega.
     + ev. simpl in H4. rewrite E in H4. rewrite <-Heqy in H4. eexists. eauto.
 Qed.
 
@@ -2366,7 +3739,7 @@ Proof.
     + unfold compat. right. right. split.
       * eapply nosubst_open. simpl. omega. eapply nosubst_intro. eauto.
       * rewrite subst_open_commute.  assert (T2 = subst TTop T2) as E. symmetry. eapply closed_no_subst; eauto. rewrite <-E. eauto. eauto. eauto.
-      
+
   - ev. simpl in H0. destruct H. repeat eexists; eauto. eapply closed_subst; eauto. eauto.
     + unfold compat. right. right. eauto.
     + unfold compat. right. right. split.
@@ -2392,7 +3765,7 @@ Proof.
     + unfold compat. right. right. split.
       * eapply nosubst_open. simpl. omega. eapply nosubst_intro. eauto.
       * rewrite subst_open_commute.  assert (T2 = subst TTop T2) as E. symmetry. eapply closed_no_subst; eauto. rewrite <-E. eauto. eauto. eauto.
-      
+
   - ev. simpl in H0. simpl in H. repeat eexists; eauto. eapply closed_subst; eauto. eauto.
     + unfold compat. right. right. split.
       * eapply nosubst_open. simpl. omega. eauto.
@@ -2419,32 +3792,32 @@ Proof.
     eapply compat_top in IX1.
     eapply compat_top in IX2.
     subst. eapply stp2_topx. eauto. eauto.
-    
+
   - Case "botx".
     intros GH0 GH0' GXX TXX T1' T2' V ? CX IX1 IX2 FA.
     eapply compat_bot in IX1.
     eapply compat_bot in IX2.
     subst. eapply stp2_botx. eauto. eauto.
-    
+
   - Case "top".
     intros GH0 GH0' GXX TXX T1' T2' V ? CX IX1 IX2 FA.
     eapply compat_top in IX2.
     subst. eapply stp2_top. eapply IHn; eauto. omega.
-    eauto. 
-    
+    eauto.
+
   - Case "bot".
     intros GH0 GH0' GXX TXX T1' T2' V ? CX IX1 IX2 FA.
     eapply compat_bot in IX1.
     subst. eapply stp2_bot. eapply IHn; eauto. omega.
     eauto.
-    
+
   - Case "bool".
     intros GH0 GH0' GXX TXX T1' T2' V ? CX IX1 IX2 FA.
     eapply compat_bool in IX1.
     eapply compat_bool in IX2.
     subst. eapply stp2_bool; eauto.
-    eauto. eauto. 
-    
+    eauto. eauto.
+
   - Case "fun".
     intros GH0 GH0' GXX TXX T1' T2' V ? CX IX1 IX2 FA.
     eapply compat_fun in IX1. repeat destruct IX1 as [? IX1].
@@ -2458,10 +3831,10 @@ Proof.
     eapply compat_mem in IX2. repeat destruct IX2 as [? IX2].
     subst. eapply stp2_mem2. eapply IHn; eauto. omega. eapply IHn; eauto. omega.
     eauto. eauto.
-                                
-  - Case "sel1". 
+
+  - Case "sel1".
     intros GH0 GH0' GXX TXX T1' T2' V ? CX IX1 IX2 FA.
-    
+
     assert (length GH = length GH0 + 1). subst GH. eapply app_length.
     assert (length GH0 = length GH0') as EL. eapply Forall2_length. eauto.
 
@@ -2473,19 +3846,20 @@ Proof.
     eapply stp2_sel1. eauto. eauto. eauto.
     eapply IHn. eauto. omega. eauto. eauto. eauto.
     eapply compat_mem_fwd2. eauto. eauto.
+    eapply IHn; eauto; try omega.
     eauto. eauto. eauto. eauto.
 
-  - Case "sel1b".
+  - Case "selb1".
     intros GH0 GH0' GXX TXX T1' T2' V ? CX IX1 IX2 FA.
 
     assert (closed 0 (length ([]:aenv)) (TBind (TMem TBot T0))). eapply stp2_closed2; eauto.
-    simpl in  H6. unfold closed in H6. inversion H6. subst. inversion H10. subst. 
+    simpl in  H6. unfold closed in H7. inversion H7. subst. inversion H11. subst.
 
-    admit. (* eapply stp2_sel1b. arg has GH = [] so nothing to be done (inversion IX2 and then a couple simplifications *)
-    
-  - Case "sel2". 
+    admit. (* eapply stp2_selb1. arg has GH = [] so nothing to be done (inversion IX2 and then a couple simplifications *)
+
+  - Case "sel2".
     intros GH0 GH0' GXX TXX T1' T2' V ? CX IX1 IX2 FA.
-    
+
     assert (length GH = length GH0 + 1). subst GH. eapply app_length.
     assert (length GH0 = length GH0') as EL. eapply Forall2_length. eauto.
 
@@ -2497,32 +3871,33 @@ Proof.
     eapply stp2_sel2. eauto. eauto. eauto.
     eapply IHn. eauto. omega. eauto. eauto. eauto.
     eapply compat_mem_fwd1. eauto. eauto.
+    eapply IHn; eauto; try omega.
     eauto. eauto. eauto. eauto.
 
-  - Case "selx". 
+  - Case "selx".
 
     intros GH0 GH0' GXX TXX T1' T2' V ? CX IX1 IX2 FA.
-    
+
     assert (length GH = length GH0 + 1). subst GH. eapply app_length.
     assert (length GH0 = length GH0') as EL. eapply Forall2_length. eauto.
 
     assert (T1' = TSel x1). destruct IX1. ev. eauto. destruct H5. ev. auto. ev. eauto.
     assert (T2' = TSel x2). destruct IX2. ev. eauto. destruct H6. ev. auto. ev. eauto.
-    
+
     subst.
-    eapply stp2_selx. eauto. eauto. 
+    eapply stp2_selx. eauto. eauto.
 
   - Case "sela1".
     intros GH0 GH0' GXX TXX T1' T2' V ? CX IX1 IX2 FA.
-    
+
     assert (length GH = length GH0 + 1). subst GH. eapply app_length.
     assert (length GH0 = length GH0') as EL. eapply Forall2_length. eauto.
 
     assert (compat GXX TXX V G1 (TSelH x) T1') as IXX. eauto.
-    
+
     eapply (compat_selh GXX TXX V G1 T1' GH0 GH0' GX TX) in IX1. repeat destruct IX1 as [? IX1].
-    
-    destruct IX1. 
+
+    destruct IX1.
     + SCase "x = 0".
       repeat destruct IXX as [|IXX]; ev.
       * subst. simpl.
@@ -2530,30 +3905,38 @@ Proof.
         eapply IHn. eauto. omega. eauto. eauto. right. left. eauto.
         eapply compat_mem_fwd2. eauto.
         eauto.
-      * subst. inversion H6. omega.
-      * subst. destruct H6. eauto.
+        eapply IHn; eauto; try omega.
+      * subst. inversion H8. omega.
+      * subst. destruct H8. eauto.
     + SCase "x > 0".
       ev. subst.
-      eapply stp2_sela1. eauto. eapply IHn; eauto. omega. eauto. eapply compat_mem_fwd2. eauto.
+      eapply stp2_sela1. eauto.
+
+      assert (x-1+1=x) as A by omega.
+      remember (x-1) as x1. rewrite <- A in H3.
+      eapply closed_compat. eauto. eapply closed_upgrade_free. eauto. omega. eauto.
+
+      eapply IHn; eauto. omega. eauto. eapply compat_mem_fwd2. eauto.
+      eapply IHn; eauto; try omega.
     (* remaining obligations *)
     + eauto. + subst GH. eauto. + eauto.
-      
+
 
   - Case "selab1".
     intros GH0 GH0' GXX TXX T1' T2' V ? CX IX1 IX2 FA.
-    
+
     assert (length GH = length GH0 + 1). subst GH. eapply app_length.
     assert (length GH0 = length GH0') as EL. eapply Forall2_length. eauto.
 
     assert (compat GXX TXX V G1 (TSelH x) T1') as IXX. eauto.
-    
+
     eapply (compat_selh GXX TXX V G1 T1' GH0 GH0' GX TX) in IX1. repeat destruct IX1 as [? IX1].
-    
+
     destruct IX1.
     + SCase "x = 0".
       assert (d = 0). admit. (* either we are called with m = 1 (from 2->1) or with m = 2, in which case we can call 2->1 *)
-      subst d. 
-      admit. (* TODO! *)        
+      subst d.
+      admit. (* TODO! *)
         (*
           Do basically what 2->1 does. Create a sel1 node.
          *)
@@ -2564,50 +3947,59 @@ Proof.
     + eauto. + subst GH. eauto. + eauto.
 
   - Case "sela2". admit. (* just like sela1 *)
-    
+
   - Case "selax".
 
     intros GH0 GH0' GXX TXX T1' T2' V ? CX IX1 IX2 FA.
-    
+
     assert (length GH = length GH0 + 1). subst GH. eapply app_length.
     assert (length GH0 = length GH0') as EL. eapply Forall2_length. eauto.
 
     assert (compat GXX TXX V G1 (TSelH x) T1') as IXX1. eauto.
     assert (compat GXX TXX V G2 (TSelH x) T2') as IXX2. eauto.
-    
+
     eapply (compat_selh GXX TXX V G1 T1' GH0 GH0' GX TX) in IX1. repeat destruct IX1 as [? IX1].
     eapply (compat_selh GXX TXX V G2 T2' GH0 GH0' GX TX) in IX2. repeat destruct IX2 as [? IX2].
     assert (not (nosubst (TSelH 0))). unfold not. intros. simpl in H1. eauto.
-    assert (not (closed 0 0 (TSelH 0))). unfold not. intros. inversion H6. omega.
+    assert (not (closed 0 0 (TSelH 0))). unfold not. intros. inversion H5. omega.
 
     destruct x; destruct IX1; ev; try omega; destruct IX2; ev; try omega; subst.
     + SCase "x = 0".
       repeat destruct IXX1 as [IXX1|IXX1]; ev; try contradiction.
-      repeat destruct IXX2 as [IXX2|IXX2]; ev; try contradiction. 
+      repeat destruct IXX2 as [IXX2|IXX2]; ev; try contradiction.
       * SSCase "sel-sel".
-        subst. inversion H16. subst.
+        subst. inversion H15. subst.
         simpl. eapply stp2_selx. eauto. eauto.
     + SCase "x > 0".
       destruct IXX1; destruct IXX2; ev; subst; eapply stp2_selax; eauto.
     (* leftovers *)
-    + eauto. + subst. eauto. + eauto. + eauto. + subst. eauto. + eauto. 
+    + eauto. + subst. eauto. + eauto. + eauto. + subst. eauto. + eauto.
 
   - Case "all".
     intros GH0 GH0' GX TX T1' T2' V ? CX IX1 IX2 FA.
-    
+
     assert (length GH = length GH0 + 1). subst GH. eapply app_length.
     assert (length GH0 = length GH0') as EL. eapply Forall2_length. eauto.
-    
+
     eapply compat_all in IX1. repeat destruct IX1 as [? IX1].
     eapply compat_all in IX2. repeat destruct IX2 as [? IX2].
 
     subst.
-    
-    eapply stp2_all. 
-    + eapply IHn. eauto. omega. eauto. eauto. eauto. eauto. eauto. 
+
+    eapply stp2_all.
+    + eapply IHn. eauto. omega. eauto. eauto. eauto. eauto. eauto.
     + eauto.
     + eauto.
-    + subst. 
+    + subst.
+      eapply IHn. eauto. omega.
+      change ((0, (G1, T0)) :: GH0 ++ [(0, (GX, TX))]) with
+      (((0, (G1, T0)) :: GH0) ++ [(0, (GX, TX))]).
+      reflexivity.
+      eauto.
+      rewrite app_length. simpl. rewrite EL. eauto.
+      rewrite app_length. simpl. rewrite EL. eauto.
+      eapply Forall2_cons. simpl. eauto. eauto.
+    + subst.
       (* specialize (IHn) with (GH0 := (0, (G2, T4))::GH0). *)
       eapply IHn. eauto. omega.
       instantiate (3:= (0, (G2, T4))::GH0).
@@ -2623,19 +4015,31 @@ Proof.
 
   - Case "bind".
     intros GH0 GH0' GX TX T1' T2' V ? CX IX1 IX2 FA.
-    
+
     assert (length GH = length GH0 + 1). subst GH. eapply app_length.
     assert (length GH0 = length GH0') as EL. eapply Forall2_length. eauto.
-    
+
     eapply compat_bind in IX1. repeat destruct IX1 as [? IX1].
     eapply compat_bind in IX2. repeat destruct IX2 as [? IX2].
 
-    subst. 
-    
-    eapply stp2_bindb. 
+    subst.
+
+    eapply stp2_bindb.
     + eauto.
     + eauto.
-    + subst. 
+    + subst.
+      eapply IHn. eauto. omega.
+      change
+        ((0, (G2, open (TSelH (length (GH0 ++ [(0, (GX, TX))]))) T3))
+           :: GH0 ++ [(0, (GX, TX))]) with
+      (((0, (G2, open (TSelH (length (GH0 ++ [(0, (GX, TX))]))) T3))
+          :: GH0) ++ [(0, (GX, TX))]).
+      reflexivity.
+      eauto.
+      rewrite app_length. simpl. rewrite EL. eauto.
+      rewrite app_length. simpl. rewrite EL. eauto.
+      eapply Forall2_cons. simpl. eauto. eauto. repeat split. rewrite app_length. simpl. rewrite EL. eapply IX2. eauto.
+    + subst.
 (*
       specialize (IHstp2 H2) with (GH1 := (0, (G1,  open (TSelH (length (GH0 ++ [(0, (GX, TX))]))) T1))::GH0). *)
       eapply IHn. eauto. omega.
@@ -2647,15 +4051,31 @@ Proof.
       eapply Forall2_cons. simpl. eauto. eauto. repeat split. rewrite app_length. simpl. rewrite EL. eapply IX1. eauto.
     + eauto.
     + eauto. subst GH. fold id. rewrite <- EL.
-      eapply closed_upgrade_free. eauto. unfold id in H5. omega.
+      eapply closed_upgrade_free. eauto. unfold id in H5.
+      rewrite app_length. simpl. omega.
     + eauto.
     + eauto. subst GH. fold id. rewrite <-EL.
-      eapply closed_upgrade_free. eauto. unfold id in H5. omega.
+      eapply closed_upgrade_free. eauto. unfold id in H5.
+      rewrite app_length. simpl. omega.
 
-  - Case "and11". admit.
-  - Case "and12". admit.
-  - Case "and2". admit.
+  - Case "and11".
+    intros GH0 GH0' GXX TXX T1' T2' V ? CX IX1 IX2 FA.
+    subst. apply compat_and in IX1. repeat destruct IX1 as [? IX1].
+    subst. eapply stp2_and11; eapply IHn; eauto; try omega.
+    eauto.
 
+  - Case "and12".
+    intros GH0 GH0' GXX TXX T1' T2' V ? CX IX1 IX2 FA.
+    subst. apply compat_and in IX1. repeat destruct IX1 as [? IX1].
+    subst. eapply stp2_and12; eapply IHn; eauto; try omega.
+    eauto.
+
+  - Case "and2".
+    intros GH0 GH0' GXX TXX T1' T2' V ? CX IX1 IX2 FA.
+    subst. apply compat_and in IX2. repeat destruct IX2 as [? IX2].
+    subst. eapply stp2_and2; eapply IHn; eauto; try omega.
+    eauto.
+    
   - Case "wrapf".
     intros. subst. eapply stp2_wrapf. eapply IHn; eauto. omega.
   - Case "transf".
@@ -2667,18 +4087,18 @@ Proof.
               compat GX TX (Some vx) ((fresh G3,vx)::G3) T3 T3' /\
               Forall2 (compat2 GX TX (Some vx)) GH0 GH0').
     {
-      (* TODO: If V is None, use vx = vty GX TX. (may need to pass in val_type evidence 
+      (* TODO: If V is None, use vx = vty GX TX. (may need to pass in val_type evidence
                If V is Some v, use v. However v might never actually be used.
                In that case, process as with V = None. *)
       admit.
     }
     ev.
-    
+
     assert (stp2 (S d) true G1 T1 ((fresh G3,x)::G3) T3 (GH0 ++ [(0, (GX, TX))]) n0) as S1.
     eapply stp2_extend2; eauto.
     assert (stp2 (S d) false ((fresh G3,x)::G3) T3 G2 T2 (GH0 ++ [(0, (GX, TX))]) n2) as S2.
     eapply stp2_extend1; eauto.
-      
+
     eapply stp2_transf.
     eapply IHn. eauto. omega. eauto. eauto. eauto. eauto. eauto.
     eapply IHn. eauto. omega. eauto. eauto. eauto. eauto. eauto.
@@ -2697,134 +4117,145 @@ Lemma stpd2_substitute: forall m G1 G2 T1 T2 GH,
 Proof. intros. repeat eu. eexists. eapply stp2_substitute_aux; eauto. Qed.
 
 
-
-
-(*
-(* not used right now, but could be a useful helper *)
-Lemma stp2_concretize: forall G1 G2 T1X T2X TX,
-   stp2 G1 (open (TSelH 0) T1X) G2 (open (TSelH 0) T2X) [(0,(G2, TX))] ->
-   stp2 ((fresh G1, vty G2 TX)::G1) (open (TSel (fresh G1)) T1X)
-     G2 (open TX T2X) [].
-Proof.
-  admit. (* call aux version above *)
-Qed.
-*)
-
-
 (* --------------------------------- *)
-
-(*
-Lemma stp_wf_subst: forall G1 GH T11 T12 x,
-  stp G1 GH T11 T11 ->
-  stp G1 ((x, TMem T11) :: GH) (open (TSelH x) T12) (open (TSelH x) T12) ->
-  stp G1 GH (open T11 T12) (open T11 T12).
-Proof.
-  admit.
-Qed.
-
-
-Lemma has_type_wf: forall G1 t T,
-  has_type G1 t T ->
-  stp G1 [] T T.
-Proof.
-  intros. induction H.
-  - Case "true". eauto.
-  - Case "false". eauto.
-  - Case "var". eauto.
-  - Case "app".
-    assert (stp env [] (TFun T1 T2) (TFun T1 T2)) as WF. eauto.
-    inversion WF. eauto.
-  - Case "abs".
-    eauto.
-  - Case "tapp".
-    assert (stp env [] (TAll T11 T12) (TAll T11 T12)) as WF. eauto.
-    inversion WF. subst. eapply stp_wf_subst; eauto.
-  - Case "tabs".
-    eauto.
-Qed.
-*)
-
-
 
 Lemma valtp_closed: forall G v T,
   val_type G v T -> closed 0 0 T.
-Proof. admit. Qed. (* from embedded stp2 *)
+Proof.
+  intros. inversion H; subst; repeat ev;
+  match goal with
+      [ H : stp2 ?s ?m ?G1 ?T1 G T [] ?n |- _ ] =>
+      eapply stp2_closed2 in H; simpl in H; apply H
+  end.
+Qed.
 
 Hint Constructors wf_envh.
 
-Lemma stp_to_stp2: forall G1 GH S T1 T2,
-  stp G1 GH S T1 T2 ->
+Lemma stp_to_stp2_aux: forall G1 GH T1 T2,
+  stp G1 GH T1 T2 ->
   forall GX GY, wf_env GX G1 -> wf_envh GX GY GH ->
-  stpd2 false GX T1 GX T2 GY.
-Proof with stpd2_wrapf.
-  intros G1 G2 S T1 T2 ST. induction ST; intros GX GY WX WY; eapply stpd2_wrapf.
+  stpd2 true GX T1 GX T2 GY.
+Proof.
+  intros G1 G2 T1 T2 ST. induction ST; intros GX GY WX WY.
   - Case "topx". eapply stpd2_topx.
   - Case "botx". eapply stpd2_botx.
-  - Case "top". eapply stpd2_top; eauto.
-  - Case "bot". eapply stpd2_bot; eauto.
+  - Case "top".
+    eapply stpd2_top.
+    specialize (IHST GX GY WX WY).
+    apply stpd2_reg2 in IHST.
+    apply IHST.
+  - Case "bot".
+    eapply stpd2_bot.
+    specialize (IHST GX GY WX WY).
+    apply stpd2_reg2 in IHST.
+    apply IHST.
   - Case "bool". eapply stpd2_bool; eauto.
-  - Case "fun". eapply stpd2_fun; eauto.
-  - Case "mem". eapply stpd2_mem; eauto. 
-  - Case "sel1". 
+  - Case "fun". eapply stpd2_fun; eapply stpd2_wrapf; eauto.
+  - Case "mem". eapply stpd2_mem; eapply stpd2_wrapf; eauto.
+  - Case "sel1".
     assert (exists v : vl, index x GX = Some v /\ val_type GX v TX) as A.
     eapply index_safe_ex. eauto. eauto.
     destruct A as [? [? VT]].
-    eapply stpd2_sel1. eauto. eauto. eapply valtp_closed; eauto. eauto.
+    eapply stpd2_sel1. eauto. eauto. eapply valtp_closed; eauto.
+    eapply stpd2_wrapf. eauto.
+    specialize (IHST2 GX GY WX WY).
+    apply stpd2_reg2 in IHST2.
+    apply IHST2.
   - Case "sel2".
     assert (exists v : vl, index x GX = Some v /\ val_type GX v TX) as A.
     eapply index_safe_ex. eauto. eauto.
     destruct A as [? [? VT]].
-    eapply stpd2_sel2. eauto. eauto. eapply valtp_closed; eauto. eauto.
+    eapply stpd2_sel2. eauto. eauto. eapply valtp_closed; eauto.
+    eapply stpd2_wrapf. eauto.
+    specialize (IHST2 GX GY WX WY).
+    apply stpd2_reg2 in IHST2.
+    apply IHST2.
   - Case "selb1".
     assert (exists v : vl, index x GX = Some v /\ val_type GX v TX) as A.
     eapply index_safe_ex. eauto. eauto.
     destruct A as [? [? VT]].
-    eapply stpd2_sel1b. eauto. eauto. eapply valtp_closed; eauto. eauto.
+    eapply stpd2_selb1. eauto. eauto. eapply valtp_closed; eauto.
+    eapply stpd2_wrapf. eauto.
+    specialize (IHST2 GX GY WX WY).
+    apply stpd2_reg2 in IHST2.
+    apply IHST2.
   - Case "selb2". admit.
-  - Case "selx". 
+  - Case "selx".
     assert (exists v : vl, index x GX = Some v /\ val_type GX v TX) as A.
     eapply index_safe_ex. eauto. eauto. ev.
-    eapply stpd2_selx. eauto. eauto. 
-  - Case "sela1". eauto.
+    eapply stpd2_selx. eauto. eauto.
+  - Case "sela1".
     assert (exists v, indexr x GY = Some v /\ valh_type GX GY v TX) as A.
     eapply index_safeh_ex. eauto. eauto. eauto.
     destruct A as [? [? VT]]. destruct x0.
-    inversion VT. subst. 
-    eapply stpd2_sela1. eauto. eapply IHST. eauto. eauto.
+    inversion VT. subst.
+    eapply stpd2_sela1. eauto. eauto.
+    eapply stpd2_wrapf. eapply IHST1. eauto. eauto.
+    specialize (IHST2 _ _ WX WY).
+    apply stpd2_reg2 in IHST2.
+    apply IHST2.
   - Case "sela2".
     assert (exists v, indexr x GY = Some v /\ valh_type GX GY v TX) as A.
     eapply index_safeh_ex. eauto. eauto. eauto.
     destruct A as [? [? VT]]. destruct x0.
-    inversion VT. subst. 
-    eapply stpd2_sela2. eauto. eapply IHST. eauto. eauto.
+    inversion VT. subst.
+    eapply stpd2_sela2. eauto. eauto.
+    eapply stpd2_wrapf. eapply IHST1. eauto. eauto.
+    specialize (IHST2 _ _ WX WY).
+    apply stpd2_reg2 in IHST2.
+    apply IHST2.
   - Case "selab1".
     assert (exists v, indexr x GY = Some v /\ valh_type GX GY v TX) as A.
     eapply index_safeh_ex. eauto. eauto. eauto.
     destruct A as [? [? VT]].
-    inversion VT. subst. 
-    eapply stpd2_selab1. eauto. eapply IHST. eauto. econstructor.
+    inversion VT. subst.
+    eapply stpd2_selab1. eauto.
+    eapply stpd2_wrapf. eapply IHST1. eauto. econstructor.
+    specialize (IHST2 _ _ WX WY).
+    apply stpd2_reg2 in IHST2.
+    apply IHST2.
   - Case "selab2". admit.
-  - Case "selax". eauto.
+  - Case "selax".
     assert (exists v, indexr x GY = Some v /\ valh_type GX GY v TX) as A.
     eapply index_safeh_ex. eauto. eauto. eauto. ev. destruct x0.
-    eapply stpd2_selax. eauto. eauto. 
+    eapply stpd2_selax. eauto.
   - Case "all".
     subst x. assert (length GY = length GH). eapply wfh_length; eauto.
-    eapply stpd2_all. eauto. rewrite H. eauto. rewrite H.  eauto.
+    eapply stpd2_all.
+    eapply stpd2_wrapf. eauto.
+    rewrite H. eauto. rewrite H.  eauto.
     rewrite H.
-    eapply IHST2. eauto. eapply wfeh_cons. eauto.
+    eapply stpd2_wrapf. eapply IHST2. eauto. eapply wfeh_cons. eauto.
+    rewrite H.
+    eapply stpd2_wrapf. apply IHST3; eauto.
   - Case "bind".
     subst x. assert (length GY = length GH). eapply wfh_length; eauto. unfold id in H.
     eapply stpd2_bind. rewrite H. eauto. rewrite H. eauto.
     rewrite H.
-    eapply IHST. eauto. eapply wfeh_cons. eauto.
-  - Case "and11". admit.
-  - Case "and12". admit.
-  - Case "and2". admit.
+    eapply stpd2_wrapf. eapply IHST1. eauto. eapply wfeh_cons. eauto.
+    rewrite H.
+    eapply stpd2_wrapf. eapply IHST2; eauto.
+  - Case "and11".
+    eapply stpd2_and11.
+    eapply IHST1; eauto.
+    eapply IHST2; eauto.
+  - Case "and12".
+    eapply stpd2_and12.
+    eapply IHST1; eauto.
+    eapply IHST2; eauto.
+  - Case "and2".
+    eapply stpd2_and2.
+    eapply stpd2_wrapf. eapply IHST1; eauto.
+    eapply stpd2_wrapf. eapply IHST2; eauto.
 Qed.
 
-
-
+Lemma stp_to_stp2: forall G1 GH T1 T2,
+  stp G1 GH T1 T2 ->
+  forall GX GY, wf_env GX G1 -> wf_envh GX GY GH ->
+  stpd2 false GX T1 GX T2 GY.
+Proof.
+  intros. eapply stpd2_wrapf. eapply stp_to_stp2_aux; eauto.
+Qed.
 
 Lemma invert_abs: forall venv vf T1 T2,
   val_type venv vf (TFun T1 T2) ->
@@ -2841,16 +4272,38 @@ Proof.
   assert (stpd2 false venv0 T1 venv1 T0 []) as E1. eauto.
   assert (stpd2 false venv1 T3 venv0 T2 []) as E2. eauto.
   eapply stpd2_upgrade in E1. eapply stpd2_upgrade in E2.
-  repeat eu. repeat eexists; eauto. 
+  repeat eu. repeat eexists; eauto.
 Qed.
-
-
 
 
 Lemma inv_vtp_half: forall G v T GH,
   val_type G v T ->
   exists T0, val_type (base v) v T0 /\ closed 0 0 T0 /\ stpd2 false (base v) T0 G T GH.
-Proof. admit. Qed.
+Proof.
+  intros. induction H.
+  - eexists. split; try split.
+    + simpl. econstructor. eassumption. ev. eapply stp2_reg1 in H0. apply H0.
+    + ev. eapply stp2_closed1 in H0. simpl in H0. apply H0.
+    + eapply sstpd2_downgrade. ev. eexists. simpl.
+      eapply stp2_extendH_mult0. eassumption.
+  - eexists. split; try split.
+    + simpl. econstructor. ev. eapply stp2_reg1 in H. apply H.
+    + ev. eapply stp2_closed1 in H. simpl in H. apply H.
+    + eapply sstpd2_downgrade. ev. eexists. simpl.
+      eapply stp2_extendH_mult0. eassumption.
+  - eexists. split; try split.
+    + simpl. econstructor; try eassumption. ev. eapply stp2_reg1 in H3. apply H3.
+    + ev. eapply stp2_closed1 in H3. simpl in H3. apply H3.
+    + eapply sstpd2_downgrade. ev. eexists. simpl.
+      eapply stp2_extendH_mult0. eassumption.
+  - eexists. split; try split.
+    + simpl. subst. econstructor; try eassumption. reflexivity. ev. eapply stp2_reg1 in H1. apply H1.
+    + ev. eapply stp2_closed1 in H2. simpl in H2. apply H2.
+    + eapply sstpd2_downgrade. ev. eexists. simpl.
+      eapply stp2_extendH_mult0. eassumption.
+  - repeat ev. eexists. split; try split; try eassumption.
+    + admit.
+Qed.
 
 Lemma invert_tabs: forall venv vf vx T1 T2,
   val_type venv vf (TAll T1 T2) ->
@@ -2866,50 +4319,50 @@ Lemma invert_tabs: forall venv vf vx T1 T2,
 Proof.
   intros venv0 vf vx T1 T2 VF VX STY. inversion VF; ev; try solve by inversion. inversion H2. subst.
   eexists. eexists. eexists. eexists. eexists. eexists.
-  repeat split; eauto. 
+  repeat split; eauto.
   remember (fresh venv1) as x.
   remember (x + fresh venv0) as xx.
 
   eapply stpd2_upgrade; eauto.
 
   (* -- new goal: result -- *)
-  
+
   (* inversion of TAll < TAll *)
   assert (stpd2 false venv0 T1 venv1 T0 []) as ARG. eauto.
   assert (stpd2 false venv1 (open (TSelH 0) T3) venv0 (open (TSelH 0) T2) [(0,(venv0, T1))]) as KEY. {
     eauto.
   }
-  eapply stpd2_upgrade in ARG.                                                                                                     
-  
+  eapply stpd2_upgrade in ARG.
+
   (* need reflexivity *)
-  assert (stpd2 false venv0 T1 venv0 T1 []). eapply stpd2_reg1. eauto.
+  assert (stpd2 false venv0 T1 venv0 T1 []). eapply stpd2_wrapf. eapply stpd2_reg1. eauto.
   assert (closed 0 0 T1). eapply stpd2_closed1 in H1. simpl in H1. eauto.
-  
+
   (* now rename *)
-  
+
   assert (stpd2 false ((fresh venv1,vx) :: venv1) (open_rec 0 (TSel (fresh venv1)) T3) venv0 (T2) []). { (* T2 was open T1 T2 *)
 
     (* now that sela1/sela2 can use subtyping, it is better to dispatch on the
        valtp evidence (instead of the type, as before) *)
 
     eapply inv_vtp_half in VX. ev.
-    
+
     assert (closed 0 (length ([]:aenv)) T2). eapply sstpd2_closed1; eauto.
     assert (open (TSelH 0) T2 = T2) as OP2. symmetry. eapply closed_no_open; eauto.
 
-    
-    eapply stpd2_substitute with (GH0:=nil). 
-    eapply stpd2_extend1. eapply stpd2_narrow. eapply stpd2_extendH. eapply H6. eapply KEY.
-    eauto. simpl. eauto. eauto. 
+
+    eapply stpd2_substitute with (GH0:=nil).
+    eapply stpd2_extend1. eapply stpd2_narrow. eapply H6. eapply KEY.
+    eauto. simpl. eauto. eauto.
     left. repeat eexists. eapply index_hit2. eauto. eauto. eauto. eauto.
     rewrite (subst_open_zero 0 1). eauto. eauto.
-    right. left. split. rewrite OP2. eauto. eauto. eauto. 
+    right. left. split. rewrite OP2. eauto. eauto. eauto.
   }
   eapply stpd2_upgrade in H4.
 
   (* done *)
   subst. eauto.
-Qed. 
+Qed.
 
 
 
@@ -2923,44 +4376,44 @@ Proof.
   intros n. induction n.
   (* 0 *)   intros. inversion H.
   (* S n *) intros. destruct e; inversion H.
-  
+
   - Case "True".
     remember (ttrue) as e. induction H0; inversion Heqe; subst.
-    + eapply not_stuck. eapply v_bool; eauto. 
+    + eapply not_stuck. eapply v_bool; eauto.
     + eapply restp_widen. eapply IHhas_type; eauto. eapply stpd2_upgrade. eapply stp_to_stp2; eauto.
 
   - Case "False".
     remember (tfalse) as e. induction H0; inversion Heqe; subst.
-    + eapply not_stuck. eapply v_bool; eauto. 
+    + eapply not_stuck. eapply v_bool; eauto.
     + eapply restp_widen. eapply IHhas_type; eauto. eapply stpd2_upgrade. eapply stp_to_stp2; eauto.
-      
+
   - Case "Var".
     remember (tvar i) as e. induction H0; inversion Heqe; subst.
-    + destruct (index_safe_ex venv0 env T1 i) as [v [I V]]; eauto. 
+    + destruct (index_safe_ex venv0 env T1 i) as [v [I V]]; eauto.
       rewrite I. eapply not_stuck. eapply V.
 
     + SCase "pack". admit.
     + SCase "unpack". admit.
-      
+
     + eapply restp_widen. eapply IHhas_type; eauto. eapply stpd2_upgrade. eapply stp_to_stp2; eauto.
 
   - Case "Typ".
     remember (ttyp t) as e. induction H0; inversion Heqe; subst.
     + admit. (* TODO: insert v_pack! *) (*eapply not_stuck. eapply v_pack. eapply v_ty; eauto. eapply stpd2_upgrade. eapply stp_to_stp2; eauto. econstructor. *)
     + eapply restp_widen. eapply IHhas_type; eauto. eapply stpd2_upgrade. eapply stp_to_stp2; eauto.
-      
+
   - Case "App".
     remember (tapp e1 e2) as e. induction H0; inversion Heqe; subst.
     +
       remember (teval n venv0 e1) as tf.
-      remember (teval n venv0 e2) as tx. 
-    
-    
+      remember (teval n venv0 e2) as tx.
+
+
       destruct tx as [rx|]; try solve by inversion.
       assert (res_type venv0 rx T1) as HRX. SCase "HRX". subst. eapply IHn; eauto.
-      inversion HRX as [? vx]. 
+      inversion HRX as [? vx].
 
-      destruct tf as [rf|]; subst rx; try solve by inversion.  
+      destruct tf as [rf|]; subst rx; try solve by inversion.
       assert (res_type venv0 rf (TFun T1 T2)) as HRF. SCase "HRF". subst. eapply IHn; eauto.
       inversion HRF as [? vf].
 
@@ -2971,19 +4424,25 @@ Proof.
       assert (res_type ((x0,vx)::(f0,vf)::env1) res T4) as HRY.
         SCase "HRY".
           subst. eapply IHn. eauto. eauto.
-          (* wf_env f x *) econstructor. eapply valtp_widen; eauto. eapply sstpd2_extend2. eapply sstpd2_extend2. eauto. eauto. eauto. 
+          (* wf_env f x *) econstructor. eapply valtp_widen; eauto. eapply sstpd2_extend2. eapply sstpd2_extend2. eauto. eauto. eauto.
           (* wf_env f   *) econstructor. eapply v_abs; eauto. eapply sstpd2_extend2.
           eapply sstpd2_downgrade in STX. eapply sstpd2_downgrade in STY. repeat eu.
-          eexists. eapply stp2_fun. eapply stp2_reg2. eapply STX. eapply stp2_reg1. eauto. eauto.
-          eauto. (* TODO: sstpd2_fun constructor *)
+          assert (stpd2 false env1 T3 env1 T3 []) as A3. {
+            eapply stpd2_wrapf. eapply stpd2_reg2. eauto.
+          }
+          inversion A3 as [na3 HA3].
+          assert (stpd2 false env1 T4 env1 T4 []) as A4 by solve [eapply stpd2_wrapf; eapply stpd2_reg1; eauto].
+          inversion A4 as [na4 HA4].
+          eexists. eapply stp2_fun. eassumption. eassumption. eauto. eauto.
+          (* TODO: sstpd2_fun constructor *)
 
       inversion HRY as [? vy].
 
       eapply not_stuck. eapply valtp_widen; eauto. eapply sstpd2_extend1. eapply sstpd2_extend1. eauto. eauto. eauto.
 
     + eapply restp_widen. eapply IHhas_type; eauto. eapply stpd2_upgrade. eapply stp_to_stp2; eauto.
-      
-    
+
+
   - Case "Abs".
     remember (tabs i i0 e) as xe. induction H0; inversion Heqxe; subst.
     + eapply not_stuck. eapply v_abs; eauto. rewrite (wf_fresh venv0 env H1). eauto. eapply stpd2_upgrade. eapply stp_to_stp2. eauto. eauto. econstructor.
@@ -2994,14 +4453,14 @@ Proof.
     +
       remember (teval n venv0 e1) as tf.
       remember (teval n venv0 e2) as tx.
-      
+
       destruct tx as [rx|]; try solve by inversion.
       assert (res_type venv0 rx T11) as HRX. SCase "HRX". subst. eapply IHn; eauto.
       inversion HRX as [? vx].
 
       subst rx.
 
-      destruct tf as [rf|]; try solve by inversion.  
+      destruct tf as [rf|]; try solve by inversion.
       assert (res_type venv0 rf (TAll T11 T12)) as HRF. SCase "HRF". subst. eapply IHn; eauto.
       inversion HRF as [? vf].
 
